<?xml version="1.0"  encoding="UTF-8"?>
<rdf:RDF
    xmlns       ="http://rdf.muninn-project.org/ontologies/documents#"
    xmlns:documents="http://rdf.muninn-project.org/ontologies/documents#"
    xmlns:rdf="http://www.w3.org/1999/02/22-rdf-syntax-ns#"
    xmlns:owl="http://www.w3.org/2002/07/owl#"
    xmlns:xsd="http://www.w3.org/2001/XMLSchema#"
    xmlns:dc="http://purl.org/dc/elements/1.1/"
    xmlns:dcterms="http://purl.org/dc/terms/"
    xmlns:time="http://www.w3.org/2006/time#"
    xmlns:foaf="http://xmlns.com/foaf/spec"
    xmlns:cc="http://creativecommons.org/ns#"
    xmlns:rdfs="http://www.w3.org/2000/01/rdf-schema#"
    xml:base="http://rdf.muninn-project.org/ontologies/documents">

  <owl:Ontology rdf:about="">
   <dc:title>The Muninn Documents Ontology</dc:title> 
   <dc:description>The Muninn Documents Ontology models documents, forms and rights.</dc:description>
   <rdfs:label xml:lang="en">The Muninn Documents Ontology</rdfs:label>
   <dc:creator rdf:resource="http://rdf.muninn-project.org/ww1/2011/11/11/Person/Warren"/>
   <cc:attributionName>The Muninn Project</cc:attributionName>
   <cc:attributionURL rdf:resource="http://www.muninn-project.org/"/>
   <rdfs:comment xml:lang="en">The Muninn Documents Ontology models documents, forms and rights.</rdfs:comment>
   <owl:versionInfo rdf:datatype="http://www.w3.org/2001/XMLSchema#decimal">1.0</owl:versionInfo>
  </owl:Ontology>

  <owl:Class rdf:ID="Document">
   <rdfs:label xml:lang="en">A Digital Document</rdfs:label>
   <rdfs:comment xml:lang="en">A digital document made up of 1 or more pages.</rdfs:comment>
   <rdfs:subClassOf rdf:resource="http://xmlns.com/foaf/spec/Document" />
  </owl:Class>

  <owl:DatatypeProperty rdf:ID="filled_out_form">
   <rdfs:label xml:lang="en">Form</rdfs:label>
   <rdfs:comment xml:lang="en">This document is a filled out form.</rdfs:comment>
   <rdfs:domain rdf:resource="#Document"/>
   <rdfs:domain rdf:resource="owl:Thing"/>
  </owl:DatatypeProperty>

  <owl:DatatypeProperty rdf:ID="pages">
   <rdfs:label xml:lang="en">Pages</rdfs:label>
   <rdfs:comment xml:lang="en">Total number of pages (single or double sided) in the document. This count may or might not match the number of content properties if one-sided and double-sided documents are present.</rdfs:comment>
   <rdfs:domain rdf:resource="#Document"/>
   <rdfs:domain rdf:resource="http://www.w3.org/2001/XMLSchema#decimal"/>
  </owl:DatatypeProperty>

  <owl:DatatypeProperty rdf:ID="title">
   <rdfs:label xml:lang="en">Title</rdfs:label>
   <rdfs:domain rdf:resource="#Document"/>
   <rdfs:domain rdf:resource="http://www.w3.org/2001/XMLSchema#string"/>
   <!-- Let's see how the reasoners like this. -->
   <rdfs:subPropertyOf rdf:resource="http://purl.org/dc/elements/1.1/title"/>
  </owl:DatatypeProperty>

  <owl:ObjectProperty rdf:ID="date_published">
   <rdfs:label xml:lang="en">Publication Date</rdfs:label>
   <rdfs:comment xml:lang="en">Date of publication of the document being modeled.</rdfs:comment>
   <rdfs:domain rdf:resource="#Document"/>
   <rdfs:range rdf:resource="time:TemporalEntity"/>
  </owl:ObjectProperty>

  <owl:ObjectProperty rdf:ID="date_retrieved">
   <rdfs:label xml:lang="en">Date Retrieved</rdfs:label>
   <rdfs:comment xml:lang="en">Date that the modeled document was retrieved from another source (eg: downloaded from a web server).</rdfs:comment>
   <rdfs:domain rdf:resource="#Document"/>
   <rdfs:range rdf:resource="time:TemporalEntity"/>
  </owl:ObjectProperty>

  <owl:ObjectProperty rdf:ID="date_digitized">
   <rdfs:label xml:lang="en">Digitization Date</rdfs:label>
   <rdfs:comment xml:lang="en">Date that this document was digitized from a physical representation.</rdfs:comment>
   <rdfs:domain rdf:resource="#Document"/>
   <rdfs:range rdf:resource="time:TemporalEntity"/>
  </owl:ObjectProperty>

  <owl:ObjectProperty rdf:ID="date_created">
   <rdfs:label xml:lang="en">Creation Date</rdfs:label>
  <rdfs:comment xml:lang="en">Date of this *record* created. (unstable / non-standard)</rdfs:comment>
   <rdfs:domain rdf:resource="#Document"/>
   <rdfs:subPropertyOf rdf:resource="http://purl.org/dc/terms/created"/>
   <rdfs:range rdf:resource="time:TemporalEntity"/>
  </owl:ObjectProperty>

  <owl:ObjectProperty rdf:ID="date_copyrighted">
   <rdfs:label xml:lang="en">Copyrighted Date</rdfs:label>
   <rdfs:comment xml:lang="en">Copyright date is synonymous with creation date in most cases. Used primarily to support copyright status and distribution permissions.</rdfs:comment>
   <rdfs:domain rdf:resource="#Document"/>
   <rdfs:subPropertyOf rdf:resource="http://purl.org/dc/terms/dateCopyrighted"/>
   <rdfs:range rdf:resource="time:TemporalEntity"/>
  </owl:ObjectProperty>


  <owl:ObjectProperty rdf:ID="publisher">
   <rdfs:label xml:lang="en">Original publisher of modeled document, may be different than the publisher of the digital copy of the documents images.</rdfs:label>
   <rdfs:domain rdf:resource="#Document"/>
   <rdfs:range rdf:resource="#owl:Thing"/>
   <rdfs:subPropertyOf rdf:resource="http://purl.org/dc/elements/1.1/publisher" />
  </owl:ObjectProperty>

  <owl:ObjectProperty rdf:ID="description">
   <rdfs:label xml:lang="en">Description</rdfs:label>
   <rdfs:domain rdf:resource="#Document"/>
   <rdfs:range rdf:resource="#owl:Thing"/>
   <rdfs:subPropertyOf rdf:resource="http://purl.org/dc/elements/1.1/description" />
  </owl:ObjectProperty>


  <owl:ObjectProperty rdf:ID="author">
   <rdfs:label xml:lang="en">Original author(s) of Document. Might have more than one.</rdfs:label>
   <rdfs:domain rdf:resource="#Document"/>
   <rdfs:range rdf:resource="#owl:Thing"/>
   <rdfs:subPropertyOf rdf:resource="http://purl.org/dc/elements/1.1/creator" />
  </owl:ObjectProperty>

  <owl:ObjectProperty rdf:ID="editor">
   <rdfs:label xml:lang="en">Editor</rdfs:label>
   <rdfs:comment xml:lang="en">Original editor(s) of Document. Might have more than one.</rdfs:comment>
   <rdfs:domain rdf:resource="#Document"/>
   <rdfs:range rdf:resource="#owl:Thing"/>
   <rdfs:subPropertyOf rdf:resource="http://purl.org/dc/elements/1.1/contributor" />
  </owl:ObjectProperty>


  <owl:ObjectProperty rdf:ID="source">
   <rdfs:label xml:lang="en">Editor</rdfs:label>
   <rdfs:comment xml:lang="en">Original Source of Document. Most likely a url or organization.</rdfs:comment>
   <rdfs:domain rdf:resource="#Document"/>
   <rdfs:range rdf:resource="#Document"/>
   <rdfs:subPropertyOf rdf:resource="http://purl.org/dc/elements/1.1/source" />
  </owl:ObjectProperty>

  <owl:ObjectProperty rdf:ID="content">
   <rdfs:label xml:lang="en">A page of the document - no ordering on property.</rdfs:label>
   <rdfs:domain rdf:resource="#Document"/>
   <rdfs:range rdf:resource="#Page"/>
  </owl:ObjectProperty>

  <owl:ObjectProperty rdf:ID="accessRights">
   <rdfs:label xml:lang="en">Access Rights</rdfs:label>
  <rdfs:comment xml:lang="en">Meant as a side support to the rights property</rdfs:comment>
   <rdfs:domain rdf:resource="#Document"/>
   <rdfs:subPropertyOf rdf:resource="http://purl.org/dc/terms/accessRights"/>
   <rdfs:range rdf:resource="cc:Permission"/>
  </owl:ObjectProperty>
  <!-- Distribution - http://creativecommons.org/ns#Distribution -->

  <cc:Permission rdf:about="http://rdf.muninn-project.org/ww1/2011/11/11/Permission/Restricted">
   <rdfs:label xml:lang="en">Restricted Access</rdfs:label>
   <rdfs:comment xml:lang="en">Webserver will not share content.</rdfs:comment> 
  </cc:Permission>
  <cc:Permission rdf:about="http://rdf.muninn-project.org/ww1/2011/11/11/Permission/ForwardToPublisher">
   <rdfs:label xml:lang="en">Forward To Publisher</rdfs:label> 
   <rdfs:comment xml:lang="en">Webserver will forward request to content to the publisher or source organization.</rdfs:comment>     
  </cc:Permission>
  <cc:Permission rdf:about="http://rdf.muninn-project.org/ww1/2011/11/11/Permission/ForwardToOriginal">
   <rdfs:label xml:lang="en">Forward to original copy</rdfs:label> 
   <rdfs:comment xml:lang="en">Forward to source URL</rdfs:comment>
  </cc:Permission>
  <cc:license rdf:about="http://rdf.muninn-project.org/ww1/2011/11/11/Permission/PublicDomain">
   <rdfs:label xml:lang="en">Public Domain</rdfs:label>
  </cc:license>
  <cc:license rdf:about="http://rdf.muninn-project.org/ww1/2011/11/11/Permission/GFDL">
   <rdfs:label xml:lang="en">GNU Free Documentation License</rdfs:label>
   <foaf:logo rdf:resource="http://upload.wikimedia.org/wikipedia/en/thumb/2/22/Heckert_GNU_white.svg/200px-Heckert_GNU_white.svg.png"/>
  </cc:license>
  <cc:license rdf:about="http://rdf.muninn-project.org/ww1/2011/11/11/Permission/FreeArtLicense">
   <rdfs:label xml:lang="en">Free Art License</rdfs:label>
   <foaf:logo rdf:resource="http://upload.wikimedia.org/wikipedia/commons/thumb/2/28/Licence_Art_Libre.svg/200px-Licence_Art_Libre.svg.png"/>
  </cc:license>
  <cc:Jurisdiction rdf:about="http://rdf.muninn-project.org/ww1/2011/11/11/Permission/US_Copyright_Act_of_1909">
   <rdfs:label xml:lang="en">The US Copyright Act of 1909</rdfs:label>
   <rdfs:comment xml:lang="en">Copyright lasts for 28 years, renewable once.</rdfs:comment>
   <owl:sameAs>http://dbpedia.org/resource/Copyright_Act_of_1909</owl:sameAs>   
  </cc:Jurisdiction>
  <cc:Jurisdiction rdf:about="http://rdf.muninn-project.org/ww1/2011/11/11/Permission/German_Empire_Copyright_Act">
   <rdfs:label xml:lang="en">Copyright Act under the German Empire</rdfs:label>
  </cc:Jurisdiction>

  <cc:Jurisdiction rdf:about="http://rdf.muninn-project.org/ww1/2011/11/11/Permission/Australia_Copyright_Act_1912">
   <rdfs:label xml:lang="en">Australian Copyright Act, 1912</rdfs:label>
   <rdfs:comment xml:lang="en">Essentially the British Copyright Act (1911), but under Australian Dominion.</rdfs:comment>
   <!-- Damm you dublin core -->
   <dcterms:dateAccepted>
    <time:DateTimeInterval>
     <time:hasDateTimeDescription>
      <time:DateTimeDescription>   
       <time:year rdf:datatype="http://www.w3.org/2001/XMLSchema#gYear">1912</time:year>
      </time:DateTimeDescription>
     </time:hasDateTimeDescription>
    </time:DateTimeInterval>
   </dcterms:dateAccepted>
   <dc:date>1912</dc:date>
   <!-- http://en.wikipedia.org/wiki/Copyright_law_of_Australia -->
  </cc:Jurisdiction>

  <cc:Jurisdiction rdf:about="http://rdf.muninn-project.org/ww1/2011/11/11/Permission/British_Copyright_Act_1911">
   <rdfs:label xml:lang="en">British Copyright Act, 1911</rdfs:label>
   <dcterms:dateAccepted>
    <time:DateTimeInterval>
     <time:hasDateTimeDescription>
      <time:DateTimeDescription>
       <time:year rdf:datatype="http://www.w3.org/2001/XMLSchema#gYear">1911</time:year>
      </time:DateTimeDescription>
     </time:hasDateTimeDescription>
    </time:DateTimeInterval>
   </dcterms:dateAccepted>
   <dc:date>1911</dc:date>
   <!-- http://en.wikipedia.org/wiki/Copyright_Act_1911 -->
  </cc:Jurisdiction>

  <cc:Jurisdiction rdf:about="http://rdf.muninn-project.org/ww1/2011/11/11/Permission/Australian_Crown_Copyright">
   <rdfs:label xml:lang="en">Australian Crown Copyright</rdfs:label>
   <rdfs:comment xml:lang="en">Copyright is owned by the crown, in the context of the state of Australia.</rdfs:comment>
   <!-- http://en.wikipedia.org/wiki/Copyright_law_of_Australia -->
  </cc:Jurisdiction>

  <cc:Jurisdiction rdf:about="http://rdf.muninn-project.org/ww1/2011/11/11/Permission/British_Crown_Copyright">
   <rdfs:label xml:lang="en">Crown Copyright (Britain)</rdfs:label>
   <rdfs:comment xml:lang="en">Copyright is owned by the crown, in the context of the state of Great Britain (or the British Empire).</rdfs:comment>
   <!-- http://en.wikipedia.org/wiki/Crown_copyright -->
  </cc:Jurisdiction>

  <cc:Jurisdiction rdf:about="http://rdf.muninn-project.org/ww1/2011/11/11/Permission/Canadian_Crown_Copyright">
   <rdfs:label xml:lang="en">Crown Copyright (Canada)</rdfs:label>
   <rdfs:comment xml:lang="en">Copyright is owned by the crown, in the context of the state of Canada.</rdfs:comment>
   <!-- http://en.wikipedia.org/wiki/Crown_copyright -->
  </cc:Jurisdiction>

  <cc:Jurisdiction rdf:about="http://rdf.muninn-project.org/ww1/2011/11/11/Permission/Newfoundland_Crown_Copyright">
   <rdfs:label xml:lang="en">Crown Copyright (Newfoundland and Labrador)</rdfs:label>
   <rdfs:comment xml:lang="en">Copyright is owned by the crown, in the context of the state of Newfoundland and Labrador.</rdfs:comment>
   <!-- http://en.wikipedia.org/wiki/Crown_copyright -->
  </cc:Jurisdiction>


<!-- Page in Documet -->
  <owl:Class rdf:ID="Page">
   <rdfs:label xml:lang="en">Page</rdfs:label>
   <rdfs:comment xml:lang="en">A page of a document, may be double-sided.</rdfs:comment>
   <rdfs:subClassOf rdf:resource="#Document" />
  </owl:Class>

<owl:DataTypeProperty rdf:ID="page_number">
 <rdfs:label xml:lang="en">Page Number</rdfs:label>  
 <rdfs:domain rdf:resource="#Page"/>
 <rdfs:comment xml:lang="en">The page number, as numbered in the actual document. This means that the number of page objects isn't related to number of physical pages.</rdfs:comment>
 <rdfs:range rdf:resource="http://www.w3.org/2001/XMLSchema#integer"/>
</owl:DataTypeProperty>

 <owl:ObjectProperty rdf:ID="depiction">
  <rdfs:label xml:lang="en">Imaged copy of the page.</rdfs:label>
  <rdfs:domain rdf:resource="#Page"/>
  <rdfs:range rdf:resource="#Image"/> 
  <rdfs:subPropertyOf rdf:resource="foaf:depiction" />
 </owl:ObjectProperty>

 <owl:ObjectProperty rdf:ID="back_page">
  <rdfs:label xml:lang="en">Back Page</rdfs:label>
  <rdfs:comment xml:lang="en">The side of the physical piece of paper that should be read last.</rdfs:comment>
  <rdfs:domain rdf:resource="#Page"/>
  <rdfs:range rdf:resource="#Page"/> 
 </owl:ObjectProperty>

 <owl:ObjectProperty rdf:ID="front_page">
  <rdfs:label xml:lang="en">Front Page</rdfs:label>
  <rdfs:comment xml:lang="en">The side of the physical piece of paper that should be read first.</rdfs:comment>
  <rdfs:domain rdf:resource="#Page"/>
  <rdfs:range rdf:resource="#Page"/> 
  <owl:inverseOf rdf:resource="#back_page" />
 </owl:ObjectProperty>

 <owl:ObjectProperty rdf:ID="next_page">
  <rdfs:label xml:lang="en">Next Page</rdfs:label>
   <rdfs:comment xml:lang="en">The next physical page that a human reader would read, even if blank. This implies that this property is pointing to a page that has no front_page property.</rdfs:comment>
   <rdfs:domain rdf:resource="#Page"/>
   <rdfs:range rdf:resource="#Page"/> 
 </owl:ObjectProperty>

 <owl:ObjectProperty rdf:ID="previous_page">
  <rdfs:label xml:lang="en">Previous Page</rdfs:label>
   <rdfs:comment xml:lang="en">The previous physical page that a human reader would have just read.</rdfs:comment>
  <rdfs:domain rdf:resource="#Page"/>
  <rdfs:range rdf:resource="#Page"/> 
 </owl:ObjectProperty>

 <!-- Add the constraints for a back page or front page. -->

 <!-- http://www.w3.org/2003/12/exif/http://www.w3.org/2003/12/exif/ -->

  <owl:Class rdf:ID="Image">
   <rdfs:label xml:lang="en">A Digital Image</rdfs:label>
   <rdfs:comment xml:lang="en">A digital image</rdfs:comment>
   <rdfs:subClassOf rdf:resource="http://xmlns.com/foaf/spec/Image" />
   <dc:type rdf:resource="http://purl.org/dc/dcmitype/StillImage"/>
  </owl:Class>

  <owl:DatatypeProperty rdf:ID="format">
   <rdfs:label xml:lang="en">Mime-Type</rdfs:label>
   <rdfs:domain rdf:resource="#Image"/>
   <rdfs:subPropertyOf rdf:resource="http://purl.org/dc/terms/MediaType" />
   <rdfs:range rdf:resource="http://www.w3.org/2001/XMLSchema#string"/>
  </owl:DatatypeProperty>

  <owl:DatatypeProperty rdf:ID="x_pixels">
   <rdfs:label xml:lang="en">Width of image in Pixels.</rdfs:label>
   <rdfs:domain rdf:resource="#Image"/>
   <rdfs:range rdf:resource="http://www.w3.org/2001/XMLSchema#integer"/>
  </owl:DatatypeProperty>

  <owl:DatatypeProperty rdf:ID="y_pixels">
   <rdfs:label xml:lang="en">Height of image in Pixels.</rdfs:label>
   <rdfs:domain rdf:resource="#Image"/>
   <rdfs:range rdf:resource="http://www.w3.org/2001/XMLSchema#integer"/>
  </owl:DatatypeProperty>

  <owl:DatatypeProperty rdf:ID="size_bytes" >
   <rdfs:label xml:lang="en">Size of image in 8-bit bytes.</rdfs:label>
   <rdfs:domain rdf:resource="#Image"/>
   <rdfs:range rdf:resource="http://www.w3.org/2001/XMLSchema#integer"/>
  </owl:DatatypeProperty>

  <owl:DatatypeProperty rdf:ID="url" >
   <rdfs:label xml:lang="en">Image URL</rdfs:label>
   <rdfs:comment xml:lang="en">Shortcut to the full url to the image ressource.</rdfs:comment>
   <rdfs:domain rdf:resource="#Image"/>
   <rdfs:range rdf:resource="http://www.w3.org/2001/XMLSchema#anyURI"/>
  </owl:DatatypeProperty>

  <owl:ObjectProperty rdf:ID="location" >
   <rdfs:label xml:lang="en">Location</rdfs:label>
   <rdfs:domain rdf:resource="#Image"/>
   <rdfs:range rdf:resource="#location"/>
  </owl:ObjectProperty>

</rdf:RDF>


