<?xml version="1.0"?>
<rdf:RDF
    xmlns       ="http://rdf.muninn-project.org/ontologies/mugshots#"
    xmlns:mugshots="http://rdf.muninn-project.org/ontologies/mugshots#"
    xmlns:rdf="http://www.w3.org/1999/02/22-rdf-syntax-ns#"
    xmlns:owl="http://www.w3.org/2002/07/owl#"
    xmlns:xsd="http://www.w3.org/2001/XMLSchema#"
    xmlns:vs="http://www.w3.org/2003/06/sw-vocab-status/ns#"
    xmlns:swrl="http://www.w3.org/2003/11/swrl#"
    xmlns:dc="http://purl.org/dc/elements/1.1/"
    xmlns:swrlb="http://www.w3.org/2003/11/swrlb#"
    xmlns:rdfs="http://www.w3.org/2000/01/rdf-schema#"
    xml:base="http://rdf.muninn-project.org/ontologies/mugshots">

  <owl:Ontology rdf:about="">
   <dc:title>The Muninn Mugshots Facial Recognition Ontology</dc:title> 
   <dc:description>The Muninn Mugshot Ontology is an experiment to markup facial recognition models in a manner that is portable and referenceable across research projects.</dc:description>
   <rdfs:label xml:lang="en">The Muninn Mugshots Facial Recognition Ontology</rdfs:label>
   <rdfs:comment xml:lang="en">The Muninn Mugshot Ontology is an experiment to markup facial recognition models in a manner that is portable and referenceable across research projects.</rdfs:comment>
   <dc:creator rdf:resource="http://rdf.muninn-project.org/ww1/2011/11/11/Person/Warren"/>
   <owl:versionInfo rdf:datatype="xsd:decimal">0.01</owl:versionInfo>
  </owl:Ontology>

  <owl:Class rdf:ID="Mugshot">
   <rdfs:label xml:lang="en">Mugshot</rdfs:label>
   <rdfs:comment xml:lang="en">A mugshot is a generic representation of a person appearance.</rdfs:comment>
   <rdfs:subClassOf rdf:resource="http://xmlns.com/foaf/spec/Document" />
  </owl:Class>


  <owl:Class rdf:ID="ProofImage">
   <rdfs:label xml:lang="en">ProofImage</rdfs:label>
   <rdfs:comment xml:lang="en">An image with the relevant features shown.</rdfs:comment>
   <rdfs:subClassOf rdf:resource="http://xmlns.com/foaf/spec/Document" />
  </owl:Class>

  <owl:Class rdf:ID="Profile">
   <rdfs:label xml:lang="en">Mugshot (Profile)</rdfs:label>
   <rdfs:comment xml:lang="en"></rdfs:comment>
   <rdfs:subClassOf rdf:resource="#Mugshot" />
   <owl:disjointWith rdf:resource="#Frontal_Mugshot"/>
  </owl:Class>

  <owl:Class rdf:ID="Face">
   <rdfs:label xml:lang="en">Mugshot (Front)</rdfs:label>
   <rdfs:comment xml:lang="en"></rdfs:comment>
   <rdfs:subClassOf rdf:resource="#Mugshot" />
  </owl:Class>

  <owl:ObjectProperty rdf:ID="depiction">
   <rdfs:label xml:lang="en">Proof Image</rdfs:label>
   <rdfs:comment xml:lang="en">A proof is a image of the person in whatever view the model is meant to represent.</rdfs:comment>
   <rdfs:domain rdf:resource="#Mugshot"/>
   <rdfs:range rdf:resource="http://xmlns.com/foaf/spec/Image"/>
  </owl:ObjectProperty>

  <owl:ObjectProperty rdf:ID="source">
   <rdfs:label xml:lang="en">Source Image</rdfs:label>
   <rdfs:comment xml:lang="en">The image(s) this mugshot was derived from.</rdfs:comment>
   <rdfs:domain rdf:resource="#Mugshot"/>
   <rdfs:range rdf:resource="http://xmlns.com/foaf/spec/Image"/>
  </owl:ObjectProperty>

<owl:DatatypeProperty rdf:ID="source_left_x">
 <rdfs:label xml:lang="en">Left X Coordinate</rdfs:label>  
 <rdfs:comment xml:lang="en">Provides the left most x coordinate in the source picture where the mugshot was extracted from.</rdfs:comment>
 <rdfs:domain rdf:resource="#Mugshot"/>
 <rdfs:range rdf:resource="xsd:int" />
</owl:DatatypeProperty>

<owl:DatatypeProperty rdf:ID="source_right_x">
 <rdfs:label xml:lang="en">Right X Coordinate</rdfs:label>  
 <rdfs:comment xml:lang="en">Provides the right most x coordinate in the source picture where the mugshot was extracted from.</rdfs:comment>
 <rdfs:domain rdf:resource="#Mugshot"/>
 <rdfs:range rdf:resource="xsd:int"/>
</owl:DatatypeProperty>

<owl:DatatypeProperty rdf:ID="source_top_y">
 <rdfs:label xml:lang="en">Top Y Coordinate</rdfs:label>  
 <rdfs:comment xml:lang="en">Provides the top most (count starting from north) y coordinate in the source picture where the mugshot was extracted from.</rdfs:comment>
 <rdfs:domain rdf:resource="#Mugshot"/>
 <rdfs:range rdf:resource="xsd:int"/>
</owl:DatatypeProperty>

<owl:DatatypeProperty rdf:ID="source_bottom_y">
 <rdfs:label xml:lang="en">Bottom Y Coordinate</rdfs:label>  
 <rdfs:comment xml:lang="en">Provides the bottom most (count starting from north) y coordinate in the source picture where the mugshot was extracted from.</rdfs:comment>
 <rdfs:domain rdf:resource="#Mugshot"/>
 <rdfs:range rdf:resource="xsd:int"/>
</owl:DatatypeProperty>

  <owl:ObjectProperty rdf:ID="identity">
   <rdfs:label xml:lang="en">Indentity</rdfs:label>
   <rdfs:comment xml:lang="en">Links the mugshot to an identity instance.</rdfs:comment>
   <rdfs:domain rdf:resource="#Mugshot"/>
   <rdfs:range rdf:resource="owl:Thing"/>
  </owl:ObjectProperty>

  <owl:ObjectProperty rdf:ID="recognition_model">
   <rdfs:label xml:lang="en">Recognition Model</rdfs:label>
   <rdfs:comment xml:lang="en">Generic pointer to a recognition model used to locate this mugshot.</rdfs:comment>
   <rdfs:domain rdf:resource="#Mugshot"/>
   <rdfs:range rdf:resource="owl:Thing"/>
  </owl:ObjectProperty>
</rdf:RDF>

