<?xml version="1.0"  encoding="UTF-8"?>
<rdf:RDF
    xmlns="http://rdf.muninn-project.org/ontologies/ott#"
    xmlns:person="http://rdf.muninn-project.org/ontologies/person#"
    xmlns:vann="http://purl.org/vocab/vann/"
    xmlns:rdf="http://www.w3.org/1999/02/22-rdf-syntax-ns#"
    xmlns:org="http://rdf.muninn-project.org/ontologies/organization#"
    xmlns:mil="http://rdf.muninn-project.org/ontologies/military#"
    xmlns:muninn="http://rdf.muninn-project.org/ontologies/muninn#"
    xmlns:foaf="http://xmlns.com/foaf/0.1/"
    xmlns:dbpedia="http://dbpedia.org/resource/"
    xmlns:time = "http://www.w3.org/2006/time#"   
    xmlns:cc = "http://creativecommons.org/ns#"
    xmlns:skos="http://www.w3.org/2004/02/skos/core#"
    xmlns:prov="http://www.w3.org/ns/prov#"
    xmlns:owl="http://www.w3.org/2002/07/owl#"
    xmlns:xsd="http://www.w3.org/2001/XMLSchema#"
    xmlns:vs="http://www.w3.org/2003/06/sw-vocab-status/ns#"
    xmlns:swrl="http://www.w3.org/2003/11/swrl#"
    xmlns:dc="http://purl.org/dc/elements/1.1/"
    xmlns:swrlb="http://www.w3.org/2003/11/swrlb#"
    xmlns:rdfs="http://www.w3.org/2000/01/rdf-schema#"
    xmlns:ott="http://rdf.muninn-project.org/ontologies/ott#"
    xml:base="http://rdf.muninn-project.org/ontologies/ott">

  <owl:Ontology rdf:about="">
   <dc:title>Tommy's Dictionary of the Trenches</dc:title> 
   <dc:description>In this so-called dictionary I have tried to list most of the pet terms and slangy definitions, which Tommy Atkins uses a thousand times a day as he is serving in France. I have gathered them as I lived with him in the trenches and rest billets, and later in the hospitals in England where I met men from all parts of the line. The definitions are not official, of course. Tommy is not a sentimental sort of animal so some of his definitions are not exactly complimentary, but he is not cynical and does not mean to offend anyone higher up. It is just a sort of &quot;ragging&quot; or &quot;kidding,&quot; as the American would say, that helps him pass the time away.</dc:description>
   <rdfs:label xml:lang="en">Tommy's Dictionary of the Trenches</rdfs:label>
   <rdfs:comment xml:lang="en">As extracted and converted into OWL / RDF by the Muninn Project.</rdfs:comment>
   <dc:date rdf:datatype="http://www.w3.org/2001/XMLSchema#date">2013-09-04</dc:date>
   <vs:term_status>Stable</vs:term_status>
   <dc:creator rdf:resource="http://rdf.muninn-project.org/ww1/2011/11/11/Person/Warren"/> 
   <dc:publisher rdf:resource="http://rdf.muninn-project.org/ww1/2011/11/11/Organization/Muninn"/>
   <dc:rights rdf:resource="http://creativecommons.org/licenses/by/3.0/"/>
   <cc:attributionName>The Muninn Project</cc:attributionName>
   <cc:attributionURL rdf:resource="http://www.muninn-project.org/"/>
   <vann:preferredNamespacePrefix>ott</vann:preferredNamespacePrefix>
   <owl:versionInfo rdf:datatype="http://www.w3.org/2001/XMLSchema#decimal">1.0</owl:versionInfo>
   <prov:wasGeneratedBy>
    <prov:Activity rdf:ID="scriptExtractedOntology">
     <rdfs:label>Extracted from Over the Top, by Arthur Guy Empey by Rob Warren, Muninn Project.</rdfs:label>
     <prov:startedAtTime>2013-09-4T01:01:01Z</prov:startedAtTime>
     <prov:endedAtTime>2013-09-4T01:01:01Z</prov:endedAtTime>
     <prov:wasAssociatedWith rdf:resource="http://rdf.muninn-project.org/ww1/2011/11/11/Organization/Muninn"/>
     <prov:wasAssociatedWith rdf:resource="http://rdf.muninn-project.org/ww1/2011/11/11/Person/Warren"/>
     <prov:hadPrimarySource rdf:resource="http://www.gutenberg.org/ebooks/7962/about.rdf"/>
    </prov:Activity>
   </prov:wasGeneratedBy>
  </owl:Ontology>

 <skos:ConceptScheme rdf:ID="OverTheTopDictionary">
  <foaf:name>Tommy's Dictionary of the Trenches</foaf:name>
  <rdfs:label xml:lang="en">Tommy's Dictionary of the Trenches</rdfs:label>
  <rdfs:comment xml:lang="en">As extracted and converted into OWL / RDF by the Muninn Project. Shallow dictionary of terms in SKOS format.</rdfs:comment>   
  <dc:creator rdf:resource="http://rdf.muninn-project.org/ww1/2011/11/11/Person/d5a8872da7e01842a246cef1fdcafdc7"/>
  <rdfs:isDefinedBy rdf:resource="http://rdf.muninn-project.org/ontologies/ott"/>
 </skos:ConceptScheme>

<skos:Concept rdf:ID="Allemand">
<rdfs:label xml:lang="fr">Allemand</rdfs:label>
<foaf:name>Allemand</foaf:name>
<skos:prefLabel xml:lang="fr">Allemand</skos:prefLabel>
<skos:definition xml:lang="fr">A French term meaning &quot;German.&quot; Tommy uses it because he thinks it is a swear word.</skos:definition>
<skos:inScheme rdf:resource="#OverTheTopDictionary"/>
<rdfs:isDefinedBy rdf:resource="http://rdf.muninn-project.org/ontologies/ott"/>
<rdf:type rdf:resource="http://dbpedia.org/resource/Irony"/>
<vs:term_status>Stable</vs:term_status>
</skos:Concept>
<skos:Concept rdf:ID="Allumettes">
<rdfs:label xml:lang="fr">Allumettes</rdfs:label>
<foaf:name>Allumettes</foaf:name>
<skos:prefLabel xml:lang="fr">Allumettes</skos:prefLabel>
<skos:definition xml:lang="fr">French term for what they sell to Tommy as matches, the sulphurous fumes from which have been known to &quot;gas&quot; a whole platoon.</skos:definition>
<skos:inScheme rdf:resource="#OverTheTopDictionary"/>
<rdfs:isDefinedBy rdf:resource="http://rdf.muninn-project.org/ontologies/ott"/>
<rdf:type rdf:resource="http://dbpedia.org/resource/Irony"/>
<vs:term_status>Stable</vs:term_status>
</skos:Concept>
<skos:Concept rdf:ID="ApreslaGuerre">
<rdfs:label xml:lang="fr">Apres la Guerre</rdfs:label>
<foaf:name>Apres la Guerre</foaf:name>
<skos:prefLabel xml:lang="fr">Apres la Guerre</skos:prefLabel>
<skos:definition xml:lang="fr">&quot;After the war.&quot; Tommy&apos;s definition of Heaven.</skos:definition>
<skos:inScheme rdf:resource="#OverTheTopDictionary"/>
<rdfs:isDefinedBy rdf:resource="http://rdf.muninn-project.org/ontologies/ott"/>
<rdf:type rdf:resource="http://dbpedia.org/resource/Irony"/>
<vs:term_status>Stable</vs:term_status>
</skos:Concept>
<skos:Concept rdf:ID="ChevauxDefrise">
<rdfs:label xml:lang="fr">Chevaux-de-frise</rdfs:label>
<foaf:name>Chevaux-de-frise</foaf:name>
<skos:prefLabel xml:lang="fr">Chevaux-de-frise</skos:prefLabel>
<skos:definition xml:lang="fr">Barbed-wire defenses against cavalry.</skos:definition>
<skos:inScheme rdf:resource="#OverTheTopDictionary"/>
<rdfs:isDefinedBy rdf:resource="http://rdf.muninn-project.org/ontologies/ott"/>
<vs:term_status>Stable</vs:term_status>
</skos:Concept>
<skos:Concept rdf:ID="Compray">
<rdfs:label xml:lang="fr">Compray</rdfs:label>
<foaf:name>Compray</foaf:name>
<skos:prefLabel xml:lang="fr">Compray</skos:prefLabel>
<skos:definition xml:lang="fr">Tommy&apos;s French for &quot;Do you understand?&quot; Universally used in the trenches.</skos:definition>
<skos:inScheme rdf:resource="#OverTheTopDictionary"/>
<rdfs:isDefinedBy rdf:resource="http://rdf.muninn-project.org/ontologies/ott"/>
<vs:term_status>Stable</vs:term_status>
<rdf:type rdf:resource="http://dbpedia.org/resource/Slang"/>
</skos:Concept>
<skos:Concept rdf:ID="Deruffs">
<rdfs:label xml:lang="fr">Deruffs</rdfs:label>
<foaf:name>Deruffs</foaf:name>
<skos:prefLabel xml:lang="fr">Deruffs</skos:prefLabel>
<skos:altLabel xml:lang="fr">Deuxosufs</skos:altLabel>
<skos:definition xml:lang="fr">Tommy&apos;s French for &quot;two eggs.&quot;</skos:definition>
<skos:inScheme rdf:resource="#OverTheTopDictionary"/>
<rdfs:isDefinedBy rdf:resource="http://rdf.muninn-project.org/ontologies/ott"/>
<vs:term_status>Stable</vs:term_status>
<rdf:type rdf:resource="http://dbpedia.org/resource/Slang"/>
</skos:Concept>
<skos:Concept rdf:ID="Dupan">
<rdfs:label xml:lang="fr">Du pan</rdfs:label>
<foaf:name>Du pan</foaf:name>
<skos:prefLabel xml:lang="fr">Du pan</skos:prefLabel>
<skos:definition xml:lang="fr">Tommy&apos;s French for bread.</skos:definition>
<skos:inScheme rdf:resource="#OverTheTopDictionary"/>
<rdfs:isDefinedBy rdf:resource="http://rdf.muninn-project.org/ontologies/ott"/>
<vs:term_status>Stable</vs:term_status>
<rdf:type rdf:resource="http://dbpedia.org/resource/Slang"/>
</skos:Concept>
<skos:Concept rdf:ID="Estaminet">
<rdfs:label xml:lang="fr">Estaminet</rdfs:label>
<foaf:name>Estaminet</foaf:name>
<skos:prefLabel xml:lang="fr">Estaminet</skos:prefLabel>
<skos:definition xml:lang="fr">A French public house, or saloon, where muddy water is sold for beer.</skos:definition>
<skos:inScheme rdf:resource="#OverTheTopDictionary"/>
<rdfs:isDefinedBy rdf:resource="http://rdf.muninn-project.org/ontologies/ott"/>
<rdf:type rdf:resource="http://dbpedia.org/resource/Irony"/>
<vs:term_status>Stable</vs:term_status>
</skos:Concept>
<skos:Concept rdf:ID="Poilu">
<rdfs:label xml:lang="fr">Poilu</rdfs:label>
<foaf:name>Poilu</foaf:name>
<skos:prefLabel xml:lang="fr">Poilu</skos:prefLabel>
<skos:definition xml:lang="fr">French term for their private soldier. Tommy would use it and sometimes does, but each time he pronounces it differently, so no one knows what he is talking about.</skos:definition>
<skos:inScheme rdf:resource="#OverTheTopDictionary"/>
<rdfs:isDefinedBy rdf:resource="http://rdf.muninn-project.org/ontologies/ott"/>
<rdf:type rdf:resource="http://dbpedia.org/resource/Irony"/>
<vs:term_status>Stable</vs:term_status>
<rdf:type rdf:resource="http://dbpedia.org/resource/Slang"/>
</skos:Concept>
<skos:Concept rdf:ID="Souvenir">
<rdfs:label xml:lang="fr">Souvenir</rdfs:label>
<foaf:name>Souvenir</foaf:name>
<skos:prefLabel xml:lang="fr">Souvenir</skos:prefLabel>
<skos:definition xml:lang="fr">A begging word used by the French kiddies. When it is addressed to Tommy it generally means, a penny, biscuits, bully beef, or a tin of jam.</skos:definition>
<skos:inScheme rdf:resource="#OverTheTopDictionary"/>
<rdfs:isDefinedBy rdf:resource="http://rdf.muninn-project.org/ontologies/ott"/>
<vs:term_status>Stable</vs:term_status>
</skos:Concept>
<skos:Concept rdf:ID="VinBlanc">
<rdfs:label xml:lang="fr">Vin Blanc</rdfs:label>
<foaf:name>Vin Blanc</foaf:name>
<skos:prefLabel xml:lang="fr">Vin Blanc</skos:prefLabel>
<skos:definition xml:lang="fr">French white wine made from vinegar. They forgot the red ink.</skos:definition>
<skos:inScheme rdf:resource="#OverTheTopDictionary"/>
<rdfs:isDefinedBy rdf:resource="http://rdf.muninn-project.org/ontologies/ott"/>
<rdf:type rdf:resource="http://dbpedia.org/resource/Irony"/>
<vs:term_status>Stable</vs:term_status>
</skos:Concept>
<skos:Concept rdf:ID="VinRouge">
<rdfs:label xml:lang="fr">Vin Rouge</rdfs:label>
<foaf:name>Vin Rouge</foaf:name>
<skos:prefLabel xml:lang="fr">Vin Rouge</skos:prefLabel>
<skos:definition xml:lang="fr">French red wine made from vinegar and red ink. Tommy pays good money for it.</skos:definition>
<skos:inScheme rdf:resource="#OverTheTopDictionary"/>
<rdfs:isDefinedBy rdf:resource="http://rdf.muninn-project.org/ontologies/ott"/>
<rdf:type rdf:resource="http://dbpedia.org/resource/Irony"/>
<vs:term_status>Stable</vs:term_status>
</skos:Concept>

<skos:Concept rdf:ID="SausageBalloon">
<rdfs:label xml:lang="en">Sausage Balloon</rdfs:label>
<foaf:name>Sausage Balloon</foaf:name>
<skos:prefLabel xml:lang="en">Sausage Balloon</skos:prefLabel>
<rdfs:comment xml:lang="en">See observation balloon.</rdfs:comment>
<skos:inScheme rdf:resource="#OverTheTopDictionary"/>
<rdfs:isDefinedBy rdf:resource="http://rdf.muninn-project.org/ontologies/ott"/>
<vs:term_status>Stable</vs:term_status>
<skos:related rdf:resource="#ObservationBalloon"/>
</skos:Concept>
<skos:Concept rdf:ID="SmokeHelmet">
<rdfs:label xml:lang="en">Smoke Helmet</rdfs:label>
<foaf:name>Smoke Helmet</foaf:name>
<skos:prefLabel xml:lang="en">Smoke Helmet</skos:prefLabel>
<rdfs:comment xml:lang="en">See respirator.</rdfs:comment>
<skos:inScheme rdf:resource="#OverTheTopDictionary"/>
<rdfs:isDefinedBy rdf:resource="http://rdf.muninn-project.org/ontologies/ott"/>
<skos:related rdf:resource="#Respirator"/>
<rdf:type rdf:resource="http://dbpedia.org/resource/Irony"/>
<vs:term_status>Stable</vs:term_status>
</skos:Concept>
<skos:Concept rdf:ID="StarShell">
<rdfs:label xml:lang="en">Star Shell</rdfs:label>
<foaf:name>Star Shell</foaf:name>
<skos:prefLabel xml:lang="en">Star Shell</skos:prefLabel>
<rdfs:comment xml:lang="en">See Flare.</rdfs:comment>
<skos:inScheme rdf:resource="#OverTheTopDictionary"/>
<rdfs:isDefinedBy rdf:resource="http://rdf.muninn-project.org/ontologies/ott"/>
<vs:term_status>Stable</vs:term_status>
<skos:related rdf:resource="#Flare"/>
</skos:Concept>
<skos:Concept rdf:ID="VeryLights">
<rdfs:label xml:lang="en">Very-Lights</rdfs:label>
<foaf:name>Very-Lights</foaf:name>
<skos:prefLabel xml:lang="en">Very-Lights</skos:prefLabel>
<rdfs:comment xml:lang="en">A star shell invented by Mr. Very. See Flare.</rdfs:comment>
<skos:inScheme rdf:resource="#OverTheTopDictionary"/>
<rdfs:isDefinedBy rdf:resource="http://rdf.muninn-project.org/ontologies/ott"/>
<rdf:type rdf:resource="http://dbpedia.org/resource/Irony"/>
<vs:term_status>Stable</vs:term_status>
<skos:related rdf:resource="#Flare"/>
</skos:Concept>
<skos:Concept rdf:ID="Wire">
<rdfs:label xml:lang="en">Wire</rdfs:label>
<foaf:name>Wire</foaf:name>
<skos:prefLabel xml:lang="en">Wire</skos:prefLabel>
<rdfs:comment xml:lang="en">See barbed wire, but don&apos;t go &quot;over the top&quot; to look at it. It isn&apos;t safe.</rdfs:comment>
<skos:inScheme rdf:resource="#OverTheTopDictionary"/>
<rdfs:isDefinedBy rdf:resource="http://rdf.muninn-project.org/ontologies/ott"/>
<rdf:type rdf:resource="http://dbpedia.org/resource/Irony"/>
<vs:term_status>Stable</vs:term_status>
<skos:related rdf:resource="#BarbedWire"/>
</skos:Concept>

<skos:Concept rdf:ID="Aboutturn">
<rdfs:label xml:lang="en">About turn</rdfs:label>
<foaf:name>About turn</foaf:name>
<skos:prefLabel xml:lang="en">About turn</skos:prefLabel>
<skos:definition xml:lang="en">A military command similar to &quot;About face&quot; or &quot;To the rear, march.&quot; Tommy&apos;s nickname for Hebuterne, a point on the British line.</skos:definition>
<skos:inScheme rdf:resource="#OverTheTopDictionary"/>
<rdfs:isDefinedBy rdf:resource="http://rdf.muninn-project.org/ontologies/ott"/>
<rdf:type rdf:resource="http://dbpedia.org/resource/Irony"/>
<vs:term_status>Stable</vs:term_status>
</skos:Concept>
<skos:Concept rdf:ID="Adjutant">
<rdfs:label xml:lang="en">Adjutant</rdfs:label>
<foaf:name>Adjutant</foaf:name>
<skos:prefLabel xml:lang="en">Adjutant</skos:prefLabel>
<skos:definition xml:lang="en">The name given to an officer who helps the Colonel do nothing. He rides a horse and you see him at guard mounting and battalion parade.</skos:definition>
<skos:inScheme rdf:resource="#OverTheTopDictionary"/>
<rdfs:isDefinedBy rdf:resource="http://rdf.muninn-project.org/ontologies/ott"/>
<rdf:type rdf:resource="http://dbpedia.org/resource/Irony"/>
<vs:term_status>Stable</vs:term_status>
</skos:Concept>
<skos:Concept rdf:ID="AssistantDirectorofMedicalService">
<rdfs:label xml:lang="en">Assistant Director of Medical Service</rdfs:label>
<muninn:acronym xml:lang="en">A.D.M.S.</muninn:acronym>
<foaf:name>Assistant Director of Medical Service</foaf:name>
<skos:prefLabel xml:lang="en">Assistant Director of Medical Service</skos:prefLabel>
<skos:definition xml:lang="en">Have never seen him but he is supposed to help the D. M. S. and pass on cases where Tommy is posted as &quot;unfit for trench service.&quot;</skos:definition>
<skos:inScheme rdf:resource="#OverTheTopDictionary"/>
<rdfs:isDefinedBy rdf:resource="http://rdf.muninn-project.org/ontologies/ott"/>
<rdf:type rdf:resource="http://dbpedia.org/resource/Irony"/>
<vs:term_status>Stable</vs:term_status>
</skos:Concept>
<skos:Concept rdf:ID="AerialTorpedo">
<rdfs:label xml:lang="en">Aerial Torpedo</rdfs:label>
<foaf:name>Aerial Torpedo</foaf:name>
<skos:prefLabel xml:lang="en">Aerial Torpedo</skos:prefLabel>
<skos:definition xml:lang="en">A kind of trench mortar shell, guaranteed by the makers to break up Fritz&apos;s supper of sausages and beer, even though said supper is in a dugout thirty feet down. Sometimes it lives up to its reputation.</skos:definition>
<skos:inScheme rdf:resource="#OverTheTopDictionary"/>
<rdfs:isDefinedBy rdf:resource="http://rdf.muninn-project.org/ontologies/ott"/>
<rdf:type rdf:resource="http://dbpedia.org/resource/Irony"/>
<vs:term_status>Stable</vs:term_status>
</skos:Concept>
<skos:Concept rdf:ID="Alarm">
<rdfs:label xml:lang="en">Alarm</rdfs:label>
<foaf:name>Alarm</foaf:name>
<skos:prefLabel xml:lang="en">Alarm</skos:prefLabel>
<skos:definition xml:lang="en">A signal given in the trenches that the enemy is about to attack, frequently false. It is mainly used to break up Tommy&apos;s dreams of home.</skos:definition>
<skos:inScheme rdf:resource="#OverTheTopDictionary"/>
<rdfs:isDefinedBy rdf:resource="http://rdf.muninn-project.org/ontologies/ott"/>
<rdf:type rdf:resource="http://dbpedia.org/resource/Irony"/>
<vs:term_status>Stable</vs:term_status>
</skos:Concept>
<skos:Concept rdf:ID="Allaroundtraverse">
<rdfs:label xml:lang="en">All around traverse</rdfs:label>
<foaf:name>All around traverse</foaf:name>
<skos:prefLabel xml:lang="en">All around traverse</skos:prefLabel>
<skos:definition xml:lang="en">A machine gun so placed that its fire can be turned in any direction.</skos:definition>
<skos:inScheme rdf:resource="#OverTheTopDictionary"/>
<rdfs:isDefinedBy rdf:resource="http://rdf.muninn-project.org/ontologies/ott"/>
<vs:term_status>Stable</vs:term_status>
</skos:Concept>
<skos:Concept rdf:ID="Allotment">
<rdfs:label xml:lang="en">Allotment</rdfs:label>
<foaf:name>Allotment</foaf:name>
<skos:prefLabel xml:lang="en">Allotment</skos:prefLabel>
<skos:definition xml:lang="en">A certain sum Tommy allows to his family.</skos:definition>
<skos:inScheme rdf:resource="#OverTheTopDictionary"/>
<rdfs:isDefinedBy rdf:resource="http://rdf.muninn-project.org/ontologies/ott"/>
<vs:term_status>Stable</vs:term_status>
</skos:Concept>
<skos:Concept rdf:ID="Ammo">
<rdfs:label xml:lang="en">Ammo</rdfs:label>
<foaf:name>Ammo</foaf:name>
<skos:prefLabel xml:lang="en">Ammo</skos:prefLabel>
<skos:definition xml:lang="en">Rifle ammunition. Used to add weight to Tommy&apos;s belt. He carries 120 rounds, at all times, except when he buries it under the straw in his billet before going on a route march. In the trenches he expends it in the direction of Berlin.</skos:definition>
<skos:inScheme rdf:resource="#OverTheTopDictionary"/>
<rdfs:isDefinedBy rdf:resource="http://rdf.muninn-project.org/ontologies/ott"/>
<rdf:type rdf:resource="http://dbpedia.org/resource/Irony"/>
<vs:term_status>Stable</vs:term_status>
</skos:Concept>
<skos:Concept rdf:ID="AmmoDepot">
<rdfs:label xml:lang="en">Ammo Depot</rdfs:label>
<foaf:name>Ammo Depot</foaf:name>
<skos:prefLabel xml:lang="en">Ammo Depot</skos:prefLabel>
<skos:definition xml:lang="en">A place where ammunition is stored. It is especially useful in making enemy airmen waste bombs trying to hit it.</skos:definition>
<skos:inScheme rdf:resource="#OverTheTopDictionary"/>
<rdfs:isDefinedBy rdf:resource="http://rdf.muninn-project.org/ontologies/ott"/>
<rdf:type rdf:resource="http://dbpedia.org/resource/Irony"/>
<vs:term_status>Stable</vs:term_status>
</skos:Concept>
<skos:Concept rdf:ID="Ammonal">
<rdfs:label xml:lang="en">Ammonal</rdfs:label>
<foaf:name>Ammonal</foaf:name>
<skos:prefLabel xml:lang="en">Ammonal</skos:prefLabel>
<skos:definition xml:lang="en">A high explosive used in the Mills bomb. The Germans are more able than Tommy to discourse on its effects.</skos:definition>
<skos:inScheme rdf:resource="#OverTheTopDictionary"/>
<rdfs:isDefinedBy rdf:resource="http://rdf.muninn-project.org/ontologies/ott"/>
<rdf:type rdf:resource="http://dbpedia.org/resource/Irony"/>
<vs:term_status>Stable</vs:term_status>
</skos:Concept>
<skos:Concept rdf:ID="Anycomplaints">
<rdfs:label xml:lang="en">Any complaints</rdfs:label>
<foaf:name>Any complaints</foaf:name>
<skos:prefLabel xml:lang="en">Any complaints</skos:prefLabel>
<skos:definition xml:lang="en">A useless question asked by an inspecting officer when he makes the rounds of billets or Tommy&apos;s meals. A complaining Tommy generally lands on the crime sheet. It is only recruits who complain; the old men just sigh with disgust.</skos:definition>
<skos:inScheme rdf:resource="#OverTheTopDictionary"/>
<rdfs:isDefinedBy rdf:resource="http://rdf.muninn-project.org/ontologies/ott"/>
<rdf:type rdf:resource="http://dbpedia.org/resource/Irony"/>
<vs:term_status>Stable</vs:term_status>
</skos:Concept>
<skos:Concept rdf:ID="ArmyOrdnanceCorps">
<rdfs:label xml:lang="en">Army Ordnance Corps</rdfs:label>
<muninn:acronym xml:lang="en">A.O.C.</muninn:acronym>
<foaf:name>Army Ordnance Corps</foaf:name>
<skos:prefLabel xml:lang="en">Army Ordnance Corps</skos:prefLabel>
<skos:definition xml:lang="en">A department which deals out supplies to the troops. Its chief asset is the returning of requisitions because a comma is misplaced.</skos:definition>
<skos:inScheme rdf:resource="#OverTheTopDictionary"/>
<rdfs:isDefinedBy rdf:resource="http://rdf.muninn-project.org/ontologies/ott"/>
<rdf:type rdf:resource="http://dbpedia.org/resource/Irony"/>
<vs:term_status>Stable</vs:term_status>
</skos:Concept>
<skos:Concept rdf:ID="AssistantProvostMarshal">
<rdfs:label xml:lang="en">Assistant Provost Marshal</rdfs:label>
<muninn:acronym xml:lang="en">A.P.M.</muninn:acronym>
<foaf:name>Assistant Provost Marshal</foaf:name>
<skos:prefLabel xml:lang="en">Assistant Provost Marshal</skos:prefLabel>
<skos:definition xml:lang="en">An officer at the head of the Military Police. His headquarters are generally out of reach of the enemy&apos;s guns. His chief duties are to ride around in a motor car and wear a red band around his cap.</skos:definition>
<skos:inScheme rdf:resource="#OverTheTopDictionary"/>
<rdfs:isDefinedBy rdf:resource="http://rdf.muninn-project.org/ontologies/ott"/>
<rdf:type rdf:resource="http://dbpedia.org/resource/Irony"/>
<vs:term_status>Stable</vs:term_status>
</skos:Concept>
<skos:Concept rdf:ID="ArmyServiceCorps">
<rdfs:label xml:lang="en">Army Service Corps</rdfs:label>
<muninn:acronym xml:lang="en">A.S.C.</muninn:acronym>
<foaf:name>Army Service Corps</foaf:name>
<skos:prefLabel xml:lang="en">Army Service Corps</skos:prefLabel>
<skos:definition xml:lang="en">, or Army Safety Corps as Tommy calls it. The members of which bring up supplies to the rear of the line.</skos:definition>
<skos:inScheme rdf:resource="#OverTheTopDictionary"/>
<rdfs:isDefinedBy rdf:resource="http://rdf.muninn-project.org/ontologies/ott"/>
<rdf:type rdf:resource="http://dbpedia.org/resource/Irony"/>
<vs:term_status>Stable</vs:term_status>
</skos:Concept>
<skos:Concept rdf:ID="Backotheline">
<rdfs:label xml:lang="en">Back &apos;o the line</rdfs:label>
<foaf:name>Back &apos;o the line</foaf:name>
<skos:prefLabel xml:lang="en">Back &apos;o the line</skos:prefLabel>
<skos:definition xml:lang="en">Any place behind the firing line out of range of enemy guns.</skos:definition>
<skos:inScheme rdf:resource="#OverTheTopDictionary"/>
<rdfs:isDefinedBy rdf:resource="http://rdf.muninn-project.org/ontologies/ott"/>
<vs:term_status>Stable</vs:term_status>
</skos:Concept>
<skos:Concept rdf:ID="Baler">
<rdfs:label xml:lang="en">Baler</rdfs:label>
<foaf:name>Baler</foaf:name>
<skos:prefLabel xml:lang="en">Baler</skos:prefLabel>
<skos:definition xml:lang="en">A scoop affair for baling out water from the trenches and dugouts. As the trenches generally drain the surrounding landscape, the sun has to be appealed to before the job is completed.</skos:definition>
<skos:inScheme rdf:resource="#OverTheTopDictionary"/>
<rdfs:isDefinedBy rdf:resource="http://rdf.muninn-project.org/ontologies/ott"/>
<rdf:type rdf:resource="http://dbpedia.org/resource/Irony"/>
<vs:term_status>Stable</vs:term_status>
</skos:Concept>
<skos:Concept rdf:ID="Bantams">
<rdfs:label xml:lang="en">Bantams</rdfs:label>
<foaf:name>Bantams</foaf:name>
<skos:prefLabel xml:lang="en">Bantams</skos:prefLabel>
<skos:definition xml:lang="en">Men under the standard army height of 5 ft. 3 in. They are in a separate organization called &quot;The Bantam Battalion,&quot; and although undersized have the opinion that they can lick the whole German Army.</skos:definition>
<skos:inScheme rdf:resource="#OverTheTopDictionary"/>
<rdfs:isDefinedBy rdf:resource="http://rdf.muninn-project.org/ontologies/ott"/>
<rdf:type rdf:resource="http://dbpedia.org/resource/Irony"/>
<vs:term_status>Stable</vs:term_status>
<rdf:type rdf:resource="http://dbpedia.org/resource/Slang"/>
</skos:Concept>
<skos:Concept rdf:ID="BarbedWire">
<rdfs:label xml:lang="en">Barbed Wire</rdfs:label>
<foaf:name>Barbed Wire</foaf:name>
<skos:prefLabel xml:lang="en">Barbed Wire</skos:prefLabel>
<skos:definition xml:lang="en">A lot of prickly wire entwined around stakes driven in front of the trenches. This obstruction is supposed to prevent the Germans from taking lodgings in your dugouts. It also affords the enemy artillery rare sport trying to blow it up.</skos:definition>
<skos:inScheme rdf:resource="#OverTheTopDictionary"/>
<rdfs:isDefinedBy rdf:resource="http://rdf.muninn-project.org/ontologies/ott"/>
<rdf:type rdf:resource="http://dbpedia.org/resource/Irony"/>
<vs:term_status>Stable</vs:term_status>
</skos:Concept>
<skos:Concept rdf:ID="Barndook">
<rdfs:label xml:lang="en">Barndook</rdfs:label>
<foaf:name>Barndook</foaf:name>
<skos:prefLabel xml:lang="en">Barndook</skos:prefLabel>
<skos:definition xml:lang="en">Tommy&apos;s nickname for his rifle. He uses it because it is harder to say and spell than &quot;rifle.&quot;</skos:definition>
<skos:inScheme rdf:resource="#OverTheTopDictionary"/>
<rdfs:isDefinedBy rdf:resource="http://rdf.muninn-project.org/ontologies/ott"/>
<rdf:type rdf:resource="http://dbpedia.org/resource/Irony"/>
<vs:term_status>Stable</vs:term_status>
<rdf:type rdf:resource="http://dbpedia.org/resource/Slang"/>
</skos:Concept>
<skos:Concept rdf:ID="Barrage">
<rdfs:label xml:lang="en">Barrage</rdfs:label>
<foaf:name>Barrage</foaf:name>
<skos:prefLabel xml:lang="en">Barrage</skos:prefLabel>
<skos:definition xml:lang="en">Concentrated shell-fire on a sector of the German line. In the early days of the war, when ammunition was defective, it often landed on Tommy himself.</skos:definition>
<skos:inScheme rdf:resource="#OverTheTopDictionary"/>
<rdfs:isDefinedBy rdf:resource="http://rdf.muninn-project.org/ontologies/ott"/>
<rdf:type rdf:resource="http://dbpedia.org/resource/Irony"/>
<vs:term_status>Stable</vs:term_status>
</skos:Concept>
<skos:Concept rdf:ID="Barricade">
<rdfs:label xml:lang="en">Barricade</rdfs:label>
<foaf:name>Barricade</foaf:name>
<skos:prefLabel xml:lang="en">Barricade</skos:prefLabel>
<skos:definition xml:lang="en">An obstruction of sandbags to impede the enemy&apos;s traffic into your trench. You build it up and he promptly knocks it down, so what&apos;s the use.</skos:definition>
<skos:inScheme rdf:resource="#OverTheTopDictionary"/>
<rdfs:isDefinedBy rdf:resource="http://rdf.muninn-project.org/ontologies/ott"/>
<rdf:type rdf:resource="http://dbpedia.org/resource/Irony"/>
<vs:term_status>Stable</vs:term_status>
</skos:Concept>
<skos:Concept rdf:ID="Bashedin">
<rdfs:label xml:lang="en">Bashed in</rdfs:label>
<foaf:name>Bashed in</foaf:name>
<skos:prefLabel xml:lang="en">Bashed in</skos:prefLabel>
<skos:definition xml:lang="en">Smashed by a shell. Generally applied to a trench or dugout.</skos:definition>
<skos:inScheme rdf:resource="#OverTheTopDictionary"/>
<rdfs:isDefinedBy rdf:resource="http://rdf.muninn-project.org/ontologies/ott"/>
<vs:term_status>Stable</vs:term_status>
</skos:Concept>
<skos:Concept rdf:ID="Batman">
<rdfs:label xml:lang="en">Batman</rdfs:label>
<foaf:name>Batman</foaf:name>
<skos:prefLabel xml:lang="en">Batman</skos:prefLabel>
<skos:definition xml:lang="en">A man who volunteers to clean a non-commissioned officer&apos;s buttons but who never volunteers for a trench raid. He ranks next to a worm.</skos:definition>
<skos:inScheme rdf:resource="#OverTheTopDictionary"/>
<rdfs:isDefinedBy rdf:resource="http://rdf.muninn-project.org/ontologies/ott"/>
<rdf:type rdf:resource="http://dbpedia.org/resource/Irony"/>
<vs:term_status>Stable</vs:term_status>
</skos:Concept>
<skos:Concept rdf:ID="Bayonet">
<rdfs:label xml:lang="en">Bayonet</rdfs:label>
<foaf:name>Bayonet</foaf:name>
<skos:prefLabel xml:lang="en">Bayonet</skos:prefLabel>
<skos:definition xml:lang="en">A sort of knife-like contrivance which fits on the end of your rifle. The Government issues it to stab Germans with. Tommy uses it to toast bread.</skos:definition>
<skos:inScheme rdf:resource="#OverTheTopDictionary"/>
<rdfs:isDefinedBy rdf:resource="http://rdf.muninn-project.org/ontologies/ott"/>
<rdf:type rdf:resource="http://dbpedia.org/resource/Irony"/>
<vs:term_status>Stable</vs:term_status>
</skos:Concept>
<skos:Concept rdf:ID="BigBoys">
<rdfs:label xml:lang="en">Big Boys</rdfs:label>
<foaf:name>Big Boys</foaf:name>
<skos:prefLabel xml:lang="en">Big Boys</skos:prefLabel>
<skos:definition xml:lang="en">Large guns, generally eight inch or above.</skos:definition>
<skos:inScheme rdf:resource="#OverTheTopDictionary"/>
<rdfs:isDefinedBy rdf:resource="http://rdf.muninn-project.org/ontologies/ott"/>
<vs:term_status>Stable</vs:term_status>
<rdf:type rdf:resource="http://dbpedia.org/resource/Slang"/>
</skos:Concept>
<skos:Concept rdf:ID="BigPush">
<rdfs:label xml:lang="en">Big Push</rdfs:label>
<foaf:name>Big Push</foaf:name>
<skos:prefLabel xml:lang="en">Big Push</skos:prefLabel>
<skos:definition xml:lang="en">&quot;The Battle of the Somme.&quot; He often calls it &quot;The First of July,&quot; the date on which it started.</skos:definition>
<skos:inScheme rdf:resource="#OverTheTopDictionary"/>
<rdfs:isDefinedBy rdf:resource="http://rdf.muninn-project.org/ontologies/ott"/>
<owl:sameAs rdf:resource="http://dbpedia.org/resource/Battle_of_the_Somme"/>
<vs:term_status>Stable</vs:term_status>
<rdf:type rdf:resource="http://dbpedia.org/resource/Slang"/>
</skos:Concept>
<skos:Concept rdf:ID="BigStuff">
<rdfs:label xml:lang="en">Big Stuff</rdfs:label>
<foaf:name>Big Stuff</foaf:name>
<skos:prefLabel xml:lang="en">Big Stuff</skos:prefLabel>
<skos:definition xml:lang="en">Large shells, eight inch or over.</skos:definition>
<skos:inScheme rdf:resource="#OverTheTopDictionary"/>
<rdfs:isDefinedBy rdf:resource="http://rdf.muninn-project.org/ontologies/ott"/>
<rdf:type rdf:resource="http://dbpedia.org/resource/Irony"/>
<vs:term_status>Stable</vs:term_status>
<rdf:type rdf:resource="http://dbpedia.org/resource/Slang"/>
</skos:Concept>
<skos:Concept rdf:ID="BigWillie">
<rdfs:label xml:lang="en">Big Willie</rdfs:label>
<foaf:name>Big Willie</foaf:name>
<skos:prefLabel xml:lang="en">Big Willie</skos:prefLabel>
<skos:definition xml:lang="en">Tommy&apos;s term for his personal friend, the Kaiser.</skos:definition>
<skos:inScheme rdf:resource="#OverTheTopDictionary"/>
<rdfs:isDefinedBy rdf:resource="http://rdf.muninn-project.org/ontologies/ott"/>
<rdf:type rdf:resource="http://dbpedia.org/resource/Irony"/>
<rdf:type rdf:resource="http://dbpedia.org/resource/Nickname"/>
<vs:term_status>Stable</vs:term_status>
</skos:Concept>
<skos:Concept rdf:ID="Billet">
<rdfs:label xml:lang="en">Billet</rdfs:label>
<foaf:name>Billet</foaf:name>
<skos:prefLabel xml:lang="en">Billet</skos:prefLabel>
<skos:definition xml:lang="en">Sometimes a regular house but generally a stable where Tommy sleeps while behind the lines. It is generally located near a large manure pile. Most billets have numerous entrances-one for Tommy and the rest for rain, rats, wind, and shells.</skos:definition>
<skos:inScheme rdf:resource="#OverTheTopDictionary"/>
<rdfs:isDefinedBy rdf:resource="http://rdf.muninn-project.org/ontologies/ott"/>
<rdf:type rdf:resource="http://dbpedia.org/resource/Irony"/>
<vs:term_status>Stable</vs:term_status>
</skos:Concept>
<skos:Concept rdf:ID="BilletGuard">
<rdfs:label xml:lang="en">Billet Guard</rdfs:label>
<foaf:name>Billet Guard</foaf:name>
<skos:prefLabel xml:lang="en">Billet Guard</skos:prefLabel>
<skos:definition xml:lang="en">Three men and a corporal who are posted to guard the billets of soldiers. They do this until the orderly officer has made his rounds at night, then they go to sleep.</skos:definition>
<skos:inScheme rdf:resource="#OverTheTopDictionary"/>
<rdfs:isDefinedBy rdf:resource="http://rdf.muninn-project.org/ontologies/ott"/>
<rdf:type rdf:resource="http://dbpedia.org/resource/Irony"/>
<vs:term_status>Stable</vs:term_status>
</skos:Concept>
<skos:Concept rdf:ID="Biscuit">
<rdfs:label xml:lang="en">Biscuit</rdfs:label>
<foaf:name>Biscuit</foaf:name>
<skos:prefLabel xml:lang="en">Biscuit</skos:prefLabel>
<skos:definition xml:lang="en">A concoction of flour and water, baked until very hard. Its original use was for building purposes, but Tommy is supposed to eat it. Tommy is no coward but he balks at this. Biscuits make excellent fuel, and give no smoke.</skos:definition>
<skos:inScheme rdf:resource="#OverTheTopDictionary"/>
<rdfs:isDefinedBy rdf:resource="http://rdf.muninn-project.org/ontologies/ott"/>
<rdf:type rdf:resource="http://dbpedia.org/resource/Irony"/>
<vs:term_status>Stable</vs:term_status>
</skos:Concept>
<skos:Concept rdf:ID="Bivouac">
<rdfs:label xml:lang="en">Bivouac</rdfs:label>
<foaf:name>Bivouac</foaf:name>
<skos:prefLabel xml:lang="en">Bivouac</skos:prefLabel>
<skos:definition xml:lang="en">A term given by Tommy to a sort of tent made out of waterproof sheets.</skos:definition>
<skos:inScheme rdf:resource="#OverTheTopDictionary"/>
<rdfs:isDefinedBy rdf:resource="http://rdf.muninn-project.org/ontologies/ott"/>
<rdf:type rdf:resource="http://dbpedia.org/resource/Irony"/>
<vs:term_status>Stable</vs:term_status>
</skos:Concept>
<skos:Concept rdf:ID="Blastine">
<rdfs:label xml:lang="en">Blastine</rdfs:label>
<foaf:name>Blastine</foaf:name>
<skos:prefLabel xml:lang="en">Blastine</skos:prefLabel>
<skos:definition xml:lang="en">A high explosive which promotes Kultur in the German lines,</skos:definition>
<skos:inScheme rdf:resource="#OverTheTopDictionary"/>
<rdfs:isDefinedBy rdf:resource="http://rdf.muninn-project.org/ontologies/ott"/>
<rdf:type rdf:resource="http://dbpedia.org/resource/Irony"/>
<vs:term_status>Stable</vs:term_status>
</skos:Concept>
<skos:Concept rdf:ID="Blighty">
<rdfs:label xml:lang="en">Blighty</rdfs:label>
<foaf:name>Blighty</foaf:name>
<skos:prefLabel xml:lang="en">Blighty</skos:prefLabel>
<skos:definition xml:lang="en">An East Indian term meaning &quot;over the seas.&quot; Tommy has adopted it as a synonym for home. He tries numerous ways of reaching Blighty, but the &quot;powers that be&quot; are wise to all of his attempts, so he generally fails.</skos:definition>
<skos:inScheme rdf:resource="#OverTheTopDictionary"/>
<rdfs:isDefinedBy rdf:resource="http://rdf.muninn-project.org/ontologies/ott"/>
<rdf:type rdf:resource="http://dbpedia.org/resource/Irony"/>
<vs:term_status>Stable</vs:term_status>
</skos:Concept>
<skos:Concept rdf:ID="BlightyOne">
<rdfs:label xml:lang="en">Blighty One</rdfs:label>
<foaf:name>Blighty One</foaf:name>
<skos:prefLabel xml:lang="en">Blighty One</skos:prefLabel>
<skos:definition xml:lang="en">A wound serious enough to send Tommy to England.</skos:definition>
<skos:inScheme rdf:resource="#OverTheTopDictionary"/>
<rdfs:isDefinedBy rdf:resource="http://rdf.muninn-project.org/ontologies/ott"/>
<vs:term_status>Stable</vs:term_status>
<rdf:type rdf:resource="http://dbpedia.org/resource/Slang"/>
</skos:Concept>
<skos:Concept rdf:ID="BrigadeMachineGunCompany">
<rdfs:label xml:lang="en">Brigade Machine Gun Company</rdfs:label>
<muninn:acronym xml:lang="en">B.M.G.C.</muninn:acronym>
<foaf:name>Brigade Machine Gun Company</foaf:name>
<skos:prefLabel xml:lang="en">Brigade Machine Gun Company</skos:prefLabel>
<skos:definition xml:lang="en">Brigade Machine Gun Company, composed of Vickers machine gunners. They always put their packs on a limber or small wagon while route marching, which fact greatly arouses the Jealousy of Tommy.</skos:definition>
<skos:inScheme rdf:resource="#OverTheTopDictionary"/>
<rdfs:isDefinedBy rdf:resource="http://rdf.muninn-project.org/ontologies/ott"/>
<rdf:type rdf:resource="http://dbpedia.org/resource/Irony"/>
<vs:term_status>Stable</vs:term_status>
</skos:Concept>
<skos:Concept rdf:ID="BodySnatcher">
<rdfs:label xml:lang="en">Body Snatcher</rdfs:label>
<foaf:name>Body Snatcher</foaf:name>
<skos:prefLabel xml:lang="en">Body Snatcher</skos:prefLabel>
<skos:definition xml:lang="en">Tommy&apos;s term for a sniper.</skos:definition>
<skos:inScheme rdf:resource="#OverTheTopDictionary"/>
<rdfs:isDefinedBy rdf:resource="http://rdf.muninn-project.org/ontologies/ott"/>
<vs:term_status>Stable</vs:term_status>
<rdf:type rdf:resource="http://dbpedia.org/resource/Slang"/>
</skos:Concept>
<skos:Concept rdf:ID="Bomb">
<rdfs:label xml:lang="en">Bomb</rdfs:label>
<foaf:name>Bomb</foaf:name>
<skos:prefLabel xml:lang="en">Bomb</skos:prefLabel>
<skos:definition xml:lang="en">An infernal device filled with high explosive which you throw at the Germans. Its chief delight is to explode before it leaves your hand.</skos:definition>
<skos:inScheme rdf:resource="#OverTheTopDictionary"/>
<rdfs:isDefinedBy rdf:resource="http://rdf.muninn-project.org/ontologies/ott"/>
<rdf:type rdf:resource="http://dbpedia.org/resource/Irony"/>
<vs:term_status>Stable</vs:term_status>
</skos:Concept>
<skos:Concept rdf:ID="BombStore">
<rdfs:label xml:lang="en">Bomb Store</rdfs:label>
<foaf:name>Bomb Store</foaf:name>
<skos:prefLabel xml:lang="en">Bomb Store</skos:prefLabel>
<skos:definition xml:lang="en">A place where bombs are kept, built so the enemy cannot locate them with his fire. For that matter, Tommy can&apos;t either when he needs them.</skos:definition>
<skos:inScheme rdf:resource="#OverTheTopDictionary"/>
<rdfs:isDefinedBy rdf:resource="http://rdf.muninn-project.org/ontologies/ott"/>
<rdf:type rdf:resource="http://dbpedia.org/resource/Irony"/>
<vs:term_status>Stable</vs:term_status>
</skos:Concept>
<skos:Concept rdf:ID="BombingPost">
<rdfs:label xml:lang="en">Bombing Post</rdfs:label>
<foaf:name>Bombing Post</foaf:name>
<skos:prefLabel xml:lang="en">Bombing Post</skos:prefLabel>
<skos:definition xml:lang="en">A sort of trench or sap running from your front line to within a few yards of the enemy&apos;s trench. It is occupied by bomb throwers who would like to sign an agreement with the Germans for neither side to throw bombs.</skos:definition>
<skos:inScheme rdf:resource="#OverTheTopDictionary"/>
<rdfs:isDefinedBy rdf:resource="http://rdf.muninn-project.org/ontologies/ott"/>
<rdf:type rdf:resource="http://dbpedia.org/resource/Irony"/>
<vs:term_status>Stable</vs:term_status>
</skos:Concept>
<skos:Concept rdf:ID="Brag">
<rdfs:label xml:lang="en">Brag</rdfs:label>
<foaf:name>Brag</foaf:name>
<skos:prefLabel xml:lang="en">Brag</skos:prefLabel>
<skos:definition xml:lang="en">A card game similar to poker at which every player quits a loser and no one wins, that is, according to the statements of the several players.</skos:definition>
<skos:inScheme rdf:resource="#OverTheTopDictionary"/>
<rdfs:isDefinedBy rdf:resource="http://rdf.muninn-project.org/ontologies/ott"/>
<rdf:type rdf:resource="http://dbpedia.org/resource/Irony"/>
<vs:term_status>Stable</vs:term_status>
</skos:Concept>
<skos:Concept rdf:ID="Brazier">
<rdfs:label xml:lang="en">Brazier</rdfs:label>
<foaf:name>Brazier</foaf:name>
<skos:prefLabel xml:lang="en">Brazier</skos:prefLabel>
<skos:definition xml:lang="en">A sheet iron pot punched full of holes in which a fire is built. It is used to keep Tommy warm in his dugout until he becomes unconscious from its smoke and fumes. He calls it a &quot;fire bucket.&quot;</skos:definition>
<skos:inScheme rdf:resource="#OverTheTopDictionary"/>
<rdfs:isDefinedBy rdf:resource="http://rdf.muninn-project.org/ontologies/ott"/>
<rdf:type rdf:resource="http://dbpedia.org/resource/Irony"/>
<vs:term_status>Stable</vs:term_status>
</skos:Concept>
<skos:Concept rdf:ID="BrigadeGuard">
<rdfs:label xml:lang="en">Brigade Guard</rdfs:label>
<foaf:name>Brigade Guard</foaf:name>
<skos:prefLabel xml:lang="en">Brigade Guard</skos:prefLabel>
<skos:definition xml:lang="en">Several men who are detailed to guard Brigade Headquarters. They don&apos;t go to sleep.</skos:definition>
<skos:inScheme rdf:resource="#OverTheTopDictionary"/>
<rdfs:isDefinedBy rdf:resource="http://rdf.muninn-project.org/ontologies/ott"/>
<rdf:type rdf:resource="http://dbpedia.org/resource/Irony"/>
<vs:term_status>Stable</vs:term_status>
</skos:Concept>
<skos:Concept rdf:ID="BattalionSergeantMajor">
<rdfs:label xml:lang="en">Battalion Sergeant-Major. The highest ranking non-commissioned officer in the battalion. A constant dread to Tommy when he has forgotten to polish his buttons or dubbin his boots.</rdfs:label>
<muninn:acronym xml:lang="en">B.S.M.</muninn:acronym>
<foaf:name>Battalion Sergeant-Major. The highest ranking non-commissioned officer in the battalion. A constant dread to Tommy when he has forgotten to polish his buttons or dubbin his boots.</foaf:name>
<skos:prefLabel xml:lang="en">Battalion Sergeant-Major. The highest ranking non-commissioned officer in the battalion. A constant dread to Tommy when he has forgotten to polish his buttons or dubbin his boots.</skos:prefLabel>
<skos:definition xml:lang="en"></skos:definition>
<skos:inScheme rdf:resource="#OverTheTopDictionary"/>
<rdfs:isDefinedBy rdf:resource="http://rdf.muninn-project.org/ontologies/ott"/>
<rdf:type rdf:resource="http://dbpedia.org/resource/Irony"/>
<vs:term_status>Stable</vs:term_status>
</skos:Concept>
<skos:Concept rdf:ID="BullyBeef">
<rdfs:label xml:lang="en">Bully Beef</rdfs:label>
<foaf:name>Bully Beef</foaf:name>
<skos:prefLabel xml:lang="en">Bully Beef</skos:prefLabel>
<skos:definition xml:lang="en">A kind of corned beef with tin round it. The unopened cans make excellent walls for dugouts.</skos:definition>
<skos:inScheme rdf:resource="#OverTheTopDictionary"/>
<rdfs:isDefinedBy rdf:resource="http://rdf.muninn-project.org/ontologies/ott"/>
<rdf:type rdf:resource="http://dbpedia.org/resource/Irony"/>
<vs:term_status>Stable</vs:term_status>
<rdf:type rdf:resource="http://dbpedia.org/resource/Slang"/>
</skos:Concept>
<skos:Concept rdf:ID="Burm">
<rdfs:label xml:lang="en">Burm</rdfs:label>
<foaf:name>Burm</foaf:name>
<skos:prefLabel xml:lang="en">Burm</skos:prefLabel>
<skos:definition xml:lang="en">A narrow ledge cut along the walls of a trench to prevent earth from caving in. &quot;Burm&quot; to Tommy is a cuss word, because he has to &quot;go over the top&quot; at night to construct it.</skos:definition>
<skos:inScheme rdf:resource="#OverTheTopDictionary"/>
<rdfs:isDefinedBy rdf:resource="http://rdf.muninn-project.org/ontologies/ott"/>
<rdf:type rdf:resource="http://dbpedia.org/resource/Irony"/>
<vs:term_status>Stable</vs:term_status>
</skos:Concept>
<skos:Concept rdf:ID="Busted">
<rdfs:label xml:lang="en">Busted</rdfs:label>
<foaf:name>Busted</foaf:name>
<skos:prefLabel xml:lang="en">Busted</skos:prefLabel>
<skos:definition xml:lang="en">Term applied when a non-commissioned officer is reduced by court-martial.</skos:definition>
<skos:inScheme rdf:resource="#OverTheTopDictionary"/>
<rdfs:isDefinedBy rdf:resource="http://rdf.muninn-project.org/ontologies/ott"/>
<rdf:type rdf:resource="http://dbpedia.org/resource/Slang"/>
<vs:term_status>Stable</vs:term_status>
</skos:Concept>
<skos:Concept rdf:ID="ButtonStick">
<rdfs:label xml:lang="en">Button Stick</rdfs:label>
<foaf:name>Button Stick</foaf:name>
<skos:prefLabel xml:lang="en">Button Stick</skos:prefLabel>
<skos:definition xml:lang="en">A contrivance made of brass ten inches long which slides over the buttons and protects the tunic in cleaning.</skos:definition>
<skos:inScheme rdf:resource="#OverTheTopDictionary"/>
<rdfs:isDefinedBy rdf:resource="http://rdf.muninn-project.org/ontologies/ott"/>
<rdf:type rdf:resource="http://dbpedia.org/resource/Irony"/>
<vs:term_status>Stable</vs:term_status>
</skos:Concept>
<skos:Concept rdf:ID="Calledtothecolors">
<rdfs:label xml:lang="en">Called to the colors</rdfs:label>
<foaf:name>Called to the colors</foaf:name>
<skos:prefLabel xml:lang="en">Called to the colors</skos:prefLabel>
<skos:definition xml:lang="en">A man on reserve who has been ordered to report for service.</skos:definition>
<skos:inScheme rdf:resource="#OverTheTopDictionary"/>
<rdfs:isDefinedBy rdf:resource="http://rdf.muninn-project.org/ontologies/ott"/>
<rdf:type rdf:resource="http://dbpedia.org/resource/Slang"/>
<vs:term_status>Stable</vs:term_status>
</skos:Concept>
<skos:Concept rdf:ID="CamelCorps">
<rdfs:label xml:lang="en">Camel Corps</rdfs:label>
<foaf:name>Camel Corps</foaf:name>
<skos:prefLabel xml:lang="en">Camel Corps</skos:prefLabel>
<skos:definition xml:lang="en">Tommy&apos;s nickname for the Infantry because they look like overloaded camels, and probably because they also go eight days, and longer, without a drink, that is, of the real stuff.</skos:definition>
<skos:inScheme rdf:resource="#OverTheTopDictionary"/>
<rdfs:isDefinedBy rdf:resource="http://rdf.muninn-project.org/ontologies/ott"/>
<rdf:type rdf:resource="http://dbpedia.org/resource/Irony"/>
<rdf:type rdf:resource="http://dbpedia.org/resource/Slang"/>
<vs:term_status>Stable</vs:term_status>
</skos:Concept>
<skos:Concept rdf:ID="Candle">
<rdfs:label xml:lang="en">Candle</rdfs:label>
<foaf:name>Candle</foaf:name>
<skos:prefLabel xml:lang="en">Candle</skos:prefLabel>
<skos:definition xml:lang="en">A piece of wick surrounded by wax or tallow used for lighting purposes. One candle among six men is the general issue.</skos:definition>
<skos:inScheme rdf:resource="#OverTheTopDictionary"/>
<rdfs:isDefinedBy rdf:resource="http://rdf.muninn-project.org/ontologies/ott"/>
<rdf:type rdf:resource="http://dbpedia.org/resource/Irony"/>
<vs:term_status>Stable</vs:term_status>
</skos:Concept>
<skos:Concept rdf:ID="Canister">
<rdfs:label xml:lang="en">Canister</rdfs:label>
<foaf:name>Canister</foaf:name>
<skos:prefLabel xml:lang="en">Canister</skos:prefLabel>
<skos:definition xml:lang="en">A German trench mortar shell filled with scraps of iron and nails. Tommy really has a great contempt for this little token of German affection and he uses the nails to hang his equipment on in the dugouts.</skos:definition>
<skos:inScheme rdf:resource="#OverTheTopDictionary"/>
<rdfs:isDefinedBy rdf:resource="http://rdf.muninn-project.org/ontologies/ott"/>
<rdf:type rdf:resource="http://dbpedia.org/resource/Irony"/>
<vs:term_status>Stable</vs:term_status>
</skos:Concept>
<skos:Concept rdf:ID="Canteen">
<rdfs:label xml:lang="en">Canteen</rdfs:label>
<foaf:name>Canteen</foaf:name>
<skos:prefLabel xml:lang="en">Canteen</skos:prefLabel>
<skos:definition xml:lang="en">A mess tin issued to Tommy, who, after dinner, generally forgets to wash it, and pinches his mates for tea in the evening.</skos:definition>
<skos:inScheme rdf:resource="#OverTheTopDictionary"/>
<rdfs:isDefinedBy rdf:resource="http://rdf.muninn-project.org/ontologies/ott"/>
<rdf:type rdf:resource="http://dbpedia.org/resource/Irony"/>
<vs:term_status>Stable</vs:term_status>
</skos:Concept>
<skos:Concept rdf:ID="Carryon">
<rdfs:label xml:lang="en">Carry on</rdfs:label>
<foaf:name>Carry on</foaf:name>
<skos:prefLabel xml:lang="en">Carry on</skos:prefLabel>
<skos:definition xml:lang="en">Resume. Keep on with what you are doing. Go ahead.</skos:definition>
<skos:inScheme rdf:resource="#OverTheTopDictionary"/>
<rdfs:isDefinedBy rdf:resource="http://rdf.muninn-project.org/ontologies/ott"/>
<vs:term_status>Stable</vs:term_status>
</skos:Concept>
<skos:Concept rdf:ID="Carryingin">
<rdfs:label xml:lang="en">Carrying in</rdfs:label>
<foaf:name>Carrying in</foaf:name>
<skos:prefLabel xml:lang="en">Carrying in</skos:prefLabel>
<skos:definition xml:lang="en">Machine gunners&apos; term for taking guns, ammunition, etc., into front-line trench.</skos:definition>
<skos:inScheme rdf:resource="#OverTheTopDictionary"/>
<rdfs:isDefinedBy rdf:resource="http://rdf.muninn-project.org/ontologies/ott"/>
<rdf:type rdf:resource="http://dbpedia.org/resource/Slang"/>
<vs:term_status>Stable</vs:term_status>
</skos:Concept>
<skos:Concept rdf:ID="Caterpillar">
<rdfs:label xml:lang="en">Caterpillar</rdfs:label>
<foaf:name>Caterpillar</foaf:name>
<skos:prefLabel xml:lang="en">Caterpillar</skos:prefLabel>
<skos:definition xml:lang="en">Is not a bug, but the name given to a powerful engine used to haul the big guns over rough roads.</skos:definition>
<skos:inScheme rdf:resource="#OverTheTopDictionary"/>
<rdfs:isDefinedBy rdf:resource="http://rdf.muninn-project.org/ontologies/ott"/>
<rdf:type rdf:resource="http://dbpedia.org/resource/Irony"/>
<vs:term_status>Stable</vs:term_status>
</skos:Concept>
<skos:Concept rdf:ID="CasualtyClearingStation">
<rdfs:label xml:lang="en">Casualty Clearing Station</rdfs:label>
<muninn:acronym xml:lang="en">C.C.S.</muninn:acronym>
<foaf:name>Casualty Clearing Station</foaf:name>
<skos:prefLabel xml:lang="en">Casualty Clearing Station</skos:prefLabel>
<skos:definition xml:lang="en">A place where the doctors draw lots to see if Tommy is badly wounded enough to be sent to Blighty.</skos:definition>
<skos:inScheme rdf:resource="#OverTheTopDictionary"/>
<rdfs:isDefinedBy rdf:resource="http://rdf.muninn-project.org/ontologies/ott"/>
<rdf:type rdf:resource="http://dbpedia.org/resource/Irony"/>
<vs:term_status>Stable</vs:term_status>
</skos:Concept>
<skos:Concept rdf:ID="ChalkPit">
<rdfs:label xml:lang="en">Chalk Pit</rdfs:label>
<foaf:name>Chalk Pit</foaf:name>
<skos:prefLabel xml:lang="en">Chalk Pit</skos:prefLabel>
<skos:definition xml:lang="en">A white spot on a painted landscape used at the Machine Gunners&apos; School to train would-be gunners in picking out distinctive objects in landscapes and guessing ranges.</skos:definition>
<skos:inScheme rdf:resource="#OverTheTopDictionary"/>
<rdfs:isDefinedBy rdf:resource="http://rdf.muninn-project.org/ontologies/ott"/>
<rdf:type rdf:resource="http://dbpedia.org/resource/Irony"/>
<vs:term_status>Stable</vs:term_status>
</skos:Concept>
<skos:Concept rdf:ID="Challenge">
<rdfs:label xml:lang="en">Challenge</rdfs:label>
<foaf:name>Challenge</foaf:name>
<skos:prefLabel xml:lang="en">Challenge</skos:prefLabel>
<skos:definition xml:lang="en">A question, &quot;Who goes there?&quot; thrown at an unknown moving object by a sentry in the darkness, who hopes that said moving object will answer, &quot;Friend.&quot;</skos:definition>
<skos:inScheme rdf:resource="#OverTheTopDictionary"/>
<rdfs:isDefinedBy rdf:resource="http://rdf.muninn-project.org/ontologies/ott"/>
<rdf:type rdf:resource="http://dbpedia.org/resource/Irony"/>
<vs:term_status>Stable</vs:term_status>
</skos:Concept>
<skos:Concept rdf:ID="Char">
<rdfs:label xml:lang="en">Char</rdfs:label>
<foaf:name>Char</foaf:name>
<skos:prefLabel xml:lang="en">Char</skos:prefLabel>
<skos:definition xml:lang="en">A black poisonous brew which Tommy calls tea.</skos:definition>
<skos:inScheme rdf:resource="#OverTheTopDictionary"/>
<rdfs:isDefinedBy rdf:resource="http://rdf.muninn-project.org/ontologies/ott"/>
<rdf:type rdf:resource="http://dbpedia.org/resource/Irony"/>
<vs:term_status>Stable</vs:term_status>
<rdf:type rdf:resource="http://dbpedia.org/resource/Slang"/>
</skos:Concept>
<skos:Concept rdf:ID="Chuckinghisweightabout">
<rdfs:label xml:lang="en">Chucking his weight about</rdfs:label>
<foaf:name>Chucking his weight about</foaf:name>
<skos:prefLabel xml:lang="en">Chucking his weight about</skos:prefLabel>
<skos:definition xml:lang="en">Self-important. Generally applied to a newly promoted non-commissioned officer or a recruit airing his knowledge.</skos:definition>
<skos:inScheme rdf:resource="#OverTheTopDictionary"/>
<rdfs:isDefinedBy rdf:resource="http://rdf.muninn-project.org/ontologies/ott"/>
<rdf:type rdf:resource="http://dbpedia.org/resource/Irony"/>
<vs:term_status>Stable</vs:term_status>
<rdf:type rdf:resource="http://dbpedia.org/resource/Slang"/>
</skos:Concept>
<skos:Concept rdf:ID="Chum">
<rdfs:label xml:lang="en">Chum</rdfs:label>
<foaf:name>Chum</foaf:name>
<skos:prefLabel xml:lang="en">Chum</skos:prefLabel>
<skos:definition xml:lang="en">An endearing word used by Tommy to his mate when he wants to borrow something or have a favor done.</skos:definition>
<skos:inScheme rdf:resource="#OverTheTopDictionary"/>
<rdfs:isDefinedBy rdf:resource="http://rdf.muninn-project.org/ontologies/ott"/>
<rdf:type rdf:resource="http://dbpedia.org/resource/Irony"/>
<vs:term_status>Stable</vs:term_status>
</skos:Concept>
<skos:Concept rdf:ID="Clickedit">
<rdfs:label xml:lang="en">Clicked it</rdfs:label>
<foaf:name>Clicked it</foaf:name>
<skos:prefLabel xml:lang="en">Clicked it</skos:prefLabel>
<skos:definition xml:lang="en">Got killed; up against it; wounded.</skos:definition>
<skos:inScheme rdf:resource="#OverTheTopDictionary"/>
<rdfs:isDefinedBy rdf:resource="http://rdf.muninn-project.org/ontologies/ott"/>
<rdf:type rdf:resource="http://dbpedia.org/resource/Irony"/>
<vs:term_status>Stable</vs:term_status>
<rdf:type rdf:resource="http://dbpedia.org/resource/Slang"/>
</skos:Concept>
<skos:Concept rdf:ID="Clock">
<rdfs:label xml:lang="en">Clock</rdfs:label>
<foaf:name>Clock</foaf:name>
<skos:prefLabel xml:lang="en">Clock</skos:prefLabel>
<skos:definition xml:lang="en">&quot;Trench&quot; for the face.</skos:definition>
<skos:inScheme rdf:resource="#OverTheTopDictionary"/>
<rdfs:isDefinedBy rdf:resource="http://rdf.muninn-project.org/ontologies/ott"/>
<rdf:type rdf:resource="http://dbpedia.org/resource/Irony"/>
<vs:term_status>Stable</vs:term_status>
</skos:Concept>
<skos:Concept rdf:ID="CoalBox">
<rdfs:label xml:lang="en">Coal Box</rdfs:label>
<foaf:name>Coal Box</foaf:name>
<skos:prefLabel xml:lang="en">Coal Box</skos:prefLabel>
<skos:definition xml:lang="en">The nickname for a high explosive German shell fired from a 5.9 howitzer which emits a heavy black smoke and makes Tommy&apos;s hair stand on end.</skos:definition>
<skos:inScheme rdf:resource="#OverTheTopDictionary"/>
<rdfs:isDefinedBy rdf:resource="http://rdf.muninn-project.org/ontologies/ott"/>
<rdf:type rdf:resource="http://dbpedia.org/resource/Irony"/>
<vs:term_status>Stable</vs:term_status>
<rdf:type rdf:resource="http://dbpedia.org/resource/Slang"/>
</skos:Concept>
<skos:Concept rdf:ID="CoalFatigue">
<rdfs:label xml:lang="en">Coal Fatigue</rdfs:label>
<foaf:name>Coal Fatigue</foaf:name>
<skos:prefLabel xml:lang="en">Coal Fatigue</skos:prefLabel>
<skos:definition xml:lang="en">A detail on which Tommy has to ride in a limber and fill two sacks with coal. It takes him exactly four hours to do this. He always misses morning parade, but manages to get back in time for dinner.</skos:definition>
<skos:inScheme rdf:resource="#OverTheTopDictionary"/>
<rdfs:isDefinedBy rdf:resource="http://rdf.muninn-project.org/ontologies/ott"/>
<rdf:type rdf:resource="http://dbpedia.org/resource/Irony"/>
<vs:term_status>Stable</vs:term_status>
<rdf:type rdf:resource="http://dbpedia.org/resource/Slang"/>
</skos:Concept>
<skos:Concept rdf:ID="Cole">
<rdfs:label xml:lang="en">Cole</rdfs:label>
<foaf:name>Cole</foaf:name>
<skos:prefLabel xml:lang="en">Cole</skos:prefLabel>
<skos:definition xml:lang="en">Tommy&apos;s nickname for a penny. It buys one glass of French beer.</skos:definition>
<skos:inScheme rdf:resource="#OverTheTopDictionary"/>
<rdfs:isDefinedBy rdf:resource="http://rdf.muninn-project.org/ontologies/ott"/>
<rdf:type rdf:resource="http://dbpedia.org/resource/Irony"/>
<vs:term_status>Stable</vs:term_status>
<rdf:type rdf:resource="http://dbpedia.org/resource/Slang"/>
</skos:Concept>
<skos:Concept rdf:ID="Comingit">
<rdfs:label xml:lang="en">Coming it</rdfs:label>
<foaf:name>Coming it</foaf:name>
<skos:prefLabel xml:lang="en">Coming it</skos:prefLabel>
<skos:definition xml:lang="en">Trying to &quot;put something over.&quot;</skos:definition>
<skos:inScheme rdf:resource="#OverTheTopDictionary"/>
<rdfs:isDefinedBy rdf:resource="http://rdf.muninn-project.org/ontologies/ott"/>
<rdf:type rdf:resource="http://dbpedia.org/resource/Irony"/>
<vs:term_status>Stable</vs:term_status>
<rdf:type rdf:resource="http://dbpedia.org/resource/Slang"/>
</skos:Concept>
<skos:Concept rdf:ID="Comingtheadd">
<rdfs:label xml:lang="en">Coming the add</rdfs:label>
<foaf:name>Coming the add</foaf:name>
<skos:prefLabel xml:lang="en">Coming the add</skos:prefLabel>
<skos:definition xml:lang="en">Boasting; lying about something.</skos:definition>
<skos:inScheme rdf:resource="#OverTheTopDictionary"/>
<rdfs:isDefinedBy rdf:resource="http://rdf.muninn-project.org/ontologies/ott"/>
<rdf:type rdf:resource="http://dbpedia.org/resource/Irony"/>
<vs:term_status>Stable</vs:term_status>
<rdf:type rdf:resource="http://dbpedia.org/resource/Slang"/>
</skos:Concept>
<skos:Concept rdf:ID="CommunicationTrench">
<rdfs:label xml:lang="en">Communication Trench</rdfs:label>
<foaf:name>Communication Trench</foaf:name>
<skos:prefLabel xml:lang="en">Communication Trench</skos:prefLabel>
<skos:definition xml:lang="en">A zigzag ditch leading from the rear to the front-line trench, through which reinforcements, reliefs, ammunition, and rations are brought up. Its real use is to teach Tommy how to swear and how to wade through mud up to his knees.</skos:definition>
<skos:inScheme rdf:resource="#OverTheTopDictionary"/>
<rdfs:isDefinedBy rdf:resource="http://rdf.muninn-project.org/ontologies/ott"/>
<rdf:type rdf:resource="http://dbpedia.org/resource/Irony"/>
<vs:term_status>Stable</vs:term_status>
</skos:Concept>
<skos:Concept rdf:ID="Communique">
<rdfs:label xml:lang="en">Communique</rdfs:label>
<foaf:name>Communique</foaf:name>
<skos:prefLabel xml:lang="en">Communique</skos:prefLabel>
<skos:definition xml:lang="en">An official report which is published daily by the different warring governments for the purpose of kidding the public. They don&apos;t kid Tommy.</skos:definition>
<skos:inScheme rdf:resource="#OverTheTopDictionary"/>
<rdfs:isDefinedBy rdf:resource="http://rdf.muninn-project.org/ontologies/ott"/>
<rdf:type rdf:resource="http://dbpedia.org/resource/Irony"/>
<vs:term_status>Stable</vs:term_status>
</skos:Concept>
<skos:Concept rdf:ID="CompanyStores">
<rdfs:label xml:lang="en">Company Stores</rdfs:label>
<foaf:name>Company Stores</foaf:name>
<skos:prefLabel xml:lang="en">Company Stores</skos:prefLabel>
<skos:definition xml:lang="en">The Quartermaster-Sergeant&apos;s headquarters where stores are kept. A general hang-out for batmen, officers&apos; servants, and N.C.O.&apos;s.</skos:definition>
<skos:inScheme rdf:resource="#OverTheTopDictionary"/>
<rdfs:isDefinedBy rdf:resource="http://rdf.muninn-project.org/ontologies/ott"/>
<rdf:type rdf:resource="http://dbpedia.org/resource/Irony"/>
<vs:term_status>Stable</vs:term_status>
</skos:Concept>
<skos:Concept rdf:ID="Conscript">
<rdfs:label xml:lang="en">Conscript</rdfs:label>
<foaf:name>Conscript</foaf:name>
<skos:prefLabel xml:lang="en">Conscript</skos:prefLabel>
<skos:definition xml:lang="en">A man who tried to wait until the war was over before volunteering for the army, but was balked by the Government.</skos:definition>
<skos:inScheme rdf:resource="#OverTheTopDictionary"/>
<rdfs:isDefinedBy rdf:resource="http://rdf.muninn-project.org/ontologies/ott"/>
<rdf:type rdf:resource="http://dbpedia.org/resource/Irony"/>
<vs:term_status>Stable</vs:term_status>
</skos:Concept>
<skos:Concept rdf:ID="Consolidatecapturedline">
<rdfs:label xml:lang="en">Consolidate captured line</rdfs:label>
<foaf:name>Consolidate captured line</foaf:name>
<skos:prefLabel xml:lang="en">Consolidate captured line</skos:prefLabel>
<skos:definition xml:lang="en">Digging in or preparing a captured position for defence against a counter-attack.</skos:definition>
<skos:inScheme rdf:resource="#OverTheTopDictionary"/>
<rdfs:isDefinedBy rdf:resource="http://rdf.muninn-project.org/ontologies/ott"/>
<rdf:type rdf:resource="http://dbpedia.org/resource/Irony"/>
<vs:term_status>Stable</vs:term_status>
</skos:Concept>
<skos:Concept rdf:ID="Convalescence">
<rdfs:label xml:lang="en">Convalescence</rdfs:label>
<foaf:name>Convalescence</foaf:name>
<skos:prefLabel xml:lang="en">Convalescence</skos:prefLabel>
<skos:definition xml:lang="en">Six weeks&apos; rest allotted to a wounded Tommy. During this time the Government is planning where they will send Tommy to be wounded a second time.</skos:definition>
<skos:inScheme rdf:resource="#OverTheTopDictionary"/>
<rdfs:isDefinedBy rdf:resource="http://rdf.muninn-project.org/ontologies/ott"/>
<rdf:type rdf:resource="http://dbpedia.org/resource/Irony"/>
<vs:term_status>Stable</vs:term_status>
</skos:Concept>
<skos:Concept rdf:ID="ChurchofEngland">
<rdfs:label xml:lang="en">Church of England</rdfs:label>
<muninn:acronym xml:lang="en">C. of E.</muninn:acronym>
<foaf:name>Church of England</foaf:name>
<skos:prefLabel xml:lang="en">Church of England</skos:prefLabel>
<skos:definition xml:lang="en">This is stamped on Tommy&apos;s identification disk. He has to attend church parade whether or not he wants to go to Heaven.</skos:definition>
<skos:inScheme rdf:resource="#OverTheTopDictionary"/>
<rdfs:isDefinedBy rdf:resource="http://rdf.muninn-project.org/ontologies/ott"/>
<rdf:type rdf:resource="http://dbpedia.org/resource/Irony"/>
<vs:term_status>Stable</vs:term_status>
</skos:Concept>
<skos:Concept rdf:ID="Cook">
<rdfs:label xml:lang="en">Cook</rdfs:label>
<foaf:name>Cook</foaf:name>
<skos:prefLabel xml:lang="en">Cook</skos:prefLabel>
<skos:definition xml:lang="en">A soldier detailed to spoil Tommy&apos;s rations. He is generally picked because he was a blacksmith in civil life.</skos:definition>
<skos:inScheme rdf:resource="#OverTheTopDictionary"/>
<rdfs:isDefinedBy rdf:resource="http://rdf.muninn-project.org/ontologies/ott"/>
<rdf:type rdf:resource="http://dbpedia.org/resource/Irony"/>
<vs:term_status>Stable</vs:term_status>
</skos:Concept>
<skos:Concept rdf:ID="Cooties">
<rdfs:label xml:lang="en">Cooties</rdfs:label>
<foaf:name>Cooties</foaf:name>
<skos:prefLabel xml:lang="en">Cooties</skos:prefLabel>
<skos:definition xml:lang="en">Unwelcome inhabitants of Tommy&apos;s shirt.</skos:definition>
<skos:inScheme rdf:resource="#OverTheTopDictionary"/>
<rdfs:isDefinedBy rdf:resource="http://rdf.muninn-project.org/ontologies/ott"/>
<rdf:type rdf:resource="http://dbpedia.org/resource/Irony"/>
<vs:term_status>Stable</vs:term_status>
<rdf:type rdf:resource="http://dbpedia.org/resource/Slang"/>
</skos:Concept>
<skos:Concept rdf:ID="CounterAttack">
<rdfs:label xml:lang="en">Counter Attack</rdfs:label>
<foaf:name>Counter Attack</foaf:name>
<skos:prefLabel xml:lang="en">Counter Attack</skos:prefLabel>
<skos:definition xml:lang="en">A disagreeable habit of the enemy which makes Tommy realize that after capturing a position the hardest work is to hold it.</skos:definition>
<skos:inScheme rdf:resource="#OverTheTopDictionary"/>
<rdfs:isDefinedBy rdf:resource="http://rdf.muninn-project.org/ontologies/ott"/>
<rdf:type rdf:resource="http://dbpedia.org/resource/Irony"/>
<vs:term_status>Stable</vs:term_status>
</skos:Concept>
<skos:Concept rdf:ID="CoveringParty">
<rdfs:label xml:lang="en">Covering Party</rdfs:label>
<foaf:name>Covering Party</foaf:name>
<skos:prefLabel xml:lang="en">Covering Party</skos:prefLabel>
<skos:definition xml:lang="en">A number of men detailed to lie down in front of a working party while &quot;out in front&quot; to prevent surprise and capture by German patrols. Tommy loves this job, I don&apos;t think!</skos:definition>
<skos:inScheme rdf:resource="#OverTheTopDictionary"/>
<rdfs:isDefinedBy rdf:resource="http://rdf.muninn-project.org/ontologies/ott"/>
<rdf:type rdf:resource="http://dbpedia.org/resource/Irony"/>
<vs:term_status>Stable</vs:term_status>
</skos:Concept>
<skos:Concept rdf:ID="Crater">
<rdfs:label xml:lang="en">Crater</rdfs:label>
<foaf:name>Crater</foaf:name>
<skos:prefLabel xml:lang="en">Crater</skos:prefLabel>
<skos:definition xml:lang="en">A large circular hole in the ground made by the explosion of a mine. According to Official Communiques, Tommy always occupies a crater with great credit to himself. But sometimes the Germans get there first.</skos:definition>
<skos:inScheme rdf:resource="#OverTheTopDictionary"/>
<rdfs:isDefinedBy rdf:resource="http://rdf.muninn-project.org/ontologies/ott"/>
<rdf:type rdf:resource="http://dbpedia.org/resource/Irony"/>
<vs:term_status>Stable</vs:term_status>
</skos:Concept>
<skos:Concept rdf:ID="Cricketball">
<rdfs:label xml:lang="en">Cricket ball</rdfs:label>
<foaf:name>Cricket ball</foaf:name>
<skos:prefLabel xml:lang="en">Cricket ball</skos:prefLabel>
<skos:definition xml:lang="en">The name given to a bomb the shape and size of a cricket ball. Tommy does not use it to play cricket with.</skos:definition>
<skos:inScheme rdf:resource="#OverTheTopDictionary"/>
<rdfs:isDefinedBy rdf:resource="http://rdf.muninn-project.org/ontologies/ott"/>
<rdf:type rdf:resource="http://dbpedia.org/resource/Irony"/>
<vs:term_status>Stable</vs:term_status>
</skos:Concept>
<skos:Concept rdf:ID="CrimeSheet">
<rdfs:label xml:lang="en">Crime Sheet</rdfs:label>
<foaf:name>Crime Sheet</foaf:name>
<skos:prefLabel xml:lang="en">Crime Sheet</skos:prefLabel>
<skos:definition xml:lang="en">A useless piece of paper on which is kept a record of Tommy&apos;s misdemeanors.</skos:definition>
<skos:inScheme rdf:resource="#OverTheTopDictionary"/>
<rdfs:isDefinedBy rdf:resource="http://rdf.muninn-project.org/ontologies/ott"/>
<rdf:type rdf:resource="http://dbpedia.org/resource/Irony"/>
<vs:term_status>Stable</vs:term_status>
<rdf:type rdf:resource="http://dbpedia.org/resource/Slang"/>
</skos:Concept>
<skos:Concept rdf:ID="Crump">
<rdfs:label xml:lang="en">Crump</rdfs:label>
<foaf:name>Crump</foaf:name>
<skos:prefLabel xml:lang="en">Crump</skos:prefLabel>
<skos:definition xml:lang="en">A name given by Tommy to a high explosive German shell which when it bursts makes a &quot;Crump&quot; sort of noise.</skos:definition>
<skos:inScheme rdf:resource="#OverTheTopDictionary"/>
<rdfs:isDefinedBy rdf:resource="http://rdf.muninn-project.org/ontologies/ott"/>
<rdf:type rdf:resource="http://dbpedia.org/resource/Irony"/>
<vs:term_status>Stable</vs:term_status>
<rdf:type rdf:resource="http://dbpedia.org/resource/Slang"/>
</skos:Concept>
<skos:Concept rdf:ID="CompanySergeantMajor">
<rdfs:label xml:lang="en">Company Sergeant-Major</rdfs:label>
<muninn:acronym xml:lang="en">C.S.M.</muninn:acronym>
<foaf:name>Company Sergeant-Major</foaf:name>
<skos:prefLabel xml:lang="en">Company Sergeant-Major</skos:prefLabel>
<skos:definition xml:lang="en">Company Sergeant-Major, the head non-commissioned officer of a company, whose chief duty is to wear a crown on his arm, a couple of Boer War ribbons on his chest, and to put Tommy&apos;s name and number on the crime sheet.</skos:definition>
<skos:inScheme rdf:resource="#OverTheTopDictionary"/>
<rdfs:isDefinedBy rdf:resource="http://rdf.muninn-project.org/ontologies/ott"/>
<rdf:type rdf:resource="http://dbpedia.org/resource/Irony"/>
<vs:term_status>Stable</vs:term_status>
</skos:Concept>
<skos:Concept rdf:ID="Curtainfire">
<rdfs:label xml:lang="en">Curtain fire</rdfs:label>
<foaf:name>Curtain fire</foaf:name>
<skos:prefLabel xml:lang="en">Curtain fire</skos:prefLabel>
<skos:definition xml:lang="en">A term-applied by the artillery to a wall of shell fire on the enemy communication trenches, to prevent the bringing up of men and supplies, and also to keep our own front lines from wavering. But somehow or other men and supplies manage to leak through it.</skos:definition>
<skos:inScheme rdf:resource="#OverTheTopDictionary"/>
<rdfs:isDefinedBy rdf:resource="http://rdf.muninn-project.org/ontologies/ott"/>
<rdf:type rdf:resource="http://dbpedia.org/resource/Irony"/>
<vs:term_status>Stable</vs:term_status>
</skos:Concept>
<skos:Concept rdf:ID="Cushy">
<rdfs:label xml:lang="en">Cushy</rdfs:label>
<foaf:name>Cushy</foaf:name>
<skos:prefLabel xml:lang="en">Cushy</skos:prefLabel>
<skos:definition xml:lang="en">Easy; comfortable; &apos;&apos;pretty soft.&quot;</skos:definition>
<skos:inScheme rdf:resource="#OverTheTopDictionary"/>
<rdfs:isDefinedBy rdf:resource="http://rdf.muninn-project.org/ontologies/ott"/>
<rdf:type rdf:resource="http://dbpedia.org/resource/Irony"/>
<vs:term_status>Stable</vs:term_status>
</skos:Concept>
<skos:Concept rdf:ID="DivisionalAmmunitionColumn">
<rdfs:label xml:lang="en">Divisional Ammunition Column</rdfs:label>
<muninn:acronym xml:lang="en">D.A.C.</muninn:acronym>
<foaf:name>Divisional Ammunition Column</foaf:name>
<skos:prefLabel xml:lang="en">Divisional Ammunition Column</skos:prefLabel>
<skos:definition xml:lang="en">A collection of men, horses, and limbers, which supplies ammunition for the line and keeps Tommy awake, while in billets, with their infernal noise. They are like owls-always working at night.</skos:definition>
<skos:inScheme rdf:resource="#OverTheTopDictionary"/>
<rdfs:isDefinedBy rdf:resource="http://rdf.muninn-project.org/ontologies/ott"/>
<rdf:type rdf:resource="http://dbpedia.org/resource/Irony"/>
<vs:term_status>Stable</vs:term_status>
</skos:Concept>
<skos:Concept rdf:ID="DistinguishedConductMedal">
<rdfs:label xml:lang="en">Distinguished Conduct Medal</rdfs:label>
<muninn:acronym xml:lang="en">D.C.M.</muninn:acronym>
<foaf:name>Distinguished Conduct Medal</foaf:name>
<skos:prefLabel xml:lang="en">Distinguished Conduct Medal</skos:prefLabel>
<skos:definition xml:lang="en">A piece of bronze which a soldier gets for being foolish.</skos:definition>
<skos:inScheme rdf:resource="#OverTheTopDictionary"/>
<rdfs:isDefinedBy rdf:resource="http://rdf.muninn-project.org/ontologies/ott"/>
<rdf:type rdf:resource="http://dbpedia.org/resource/Irony"/>
<vs:term_status>Stable</vs:term_status>
</skos:Concept>
<skos:Concept rdf:ID="DivisionalConcertParty">
<rdfs:label xml:lang="en">Divisional Concert Party</rdfs:label>
<muninn:acronym xml:lang="en">D.C.P.</muninn:acronym>
<foaf:name>Divisional Concert Party</foaf:name>
<skos:prefLabel xml:lang="en">Divisional Concert Party</skos:prefLabel>
<skos:definition xml:lang="en">An aggregation of would-be actors who inflict their talents on Tommy at half a franc per head.</skos:definition>
<skos:inScheme rdf:resource="#OverTheTopDictionary"/>
<rdfs:isDefinedBy rdf:resource="http://rdf.muninn-project.org/ontologies/ott"/>
<rdf:type rdf:resource="http://dbpedia.org/resource/Irony"/>
<vs:term_status>Stable</vs:term_status>
</skos:Concept>
<skos:Concept rdf:ID="Defaulter">
<rdfs:label xml:lang="en">Defaulter</rdfs:label>
<foaf:name>Defaulter</foaf:name>
<skos:prefLabel xml:lang="en">Defaulter</skos:prefLabel>
<skos:definition xml:lang="en">Not an absconding cashier, but a Tommy who has been sentenced to extra pack drill for breathing while on parade or doing some other little thing like that.</skos:definition>
<skos:inScheme rdf:resource="#OverTheTopDictionary"/>
<rdfs:isDefinedBy rdf:resource="http://rdf.muninn-project.org/ontologies/ott"/>
<rdf:type rdf:resource="http://dbpedia.org/resource/Irony"/>
<vs:term_status>Stable</vs:term_status>
<rdf:type rdf:resource="http://dbpedia.org/resource/Slang"/>
</skos:Concept>
<skos:Concept rdf:ID="Dekko">
<rdfs:label xml:lang="en">Dekko</rdfs:label>
<foaf:name>Dekko</foaf:name>
<skos:prefLabel xml:lang="en">Dekko</skos:prefLabel>
<skos:definition xml:lang="en">To look; a look at something.</skos:definition>
<skos:inScheme rdf:resource="#OverTheTopDictionary"/>
<rdfs:isDefinedBy rdf:resource="http://rdf.muninn-project.org/ontologies/ott"/>
<rdf:type rdf:resource="http://dbpedia.org/resource/Irony"/>
<vs:term_status>Stable</vs:term_status>
<rdf:type rdf:resource="http://dbpedia.org/resource/Slang"/>
</skos:Concept>
<skos:Concept rdf:ID="Detonator">
<rdfs:label xml:lang="en">Detonator</rdfs:label>
<foaf:name>Detonator</foaf:name>
<skos:prefLabel xml:lang="en">Detonator</skos:prefLabel>
<skos:definition xml:lang="en">A contrivance in a bomb containing fulminate of mercury, which, ignited by a fuse, explodes the charge.</skos:definition>
<skos:inScheme rdf:resource="#OverTheTopDictionary"/>
<rdfs:isDefinedBy rdf:resource="http://rdf.muninn-project.org/ontologies/ott"/>
<rdf:type rdf:resource="http://dbpedia.org/resource/Irony"/>
<vs:term_status>Stable</vs:term_status>
</skos:Concept>
<skos:Concept rdf:ID="Dial">
<rdfs:label xml:lang="en">Dial</rdfs:label>
<foaf:name>Dial</foaf:name>
<skos:prefLabel xml:lang="en">Dial</skos:prefLabel>
<skos:definition xml:lang="en">Another term of Tommy&apos;s for his map, or face.</skos:definition>
<skos:inScheme rdf:resource="#OverTheTopDictionary"/>
<rdfs:isDefinedBy rdf:resource="http://rdf.muninn-project.org/ontologies/ott"/>
<rdf:type rdf:resource="http://dbpedia.org/resource/Irony"/>
<vs:term_status>Stable</vs:term_status>
</skos:Concept>
<skos:Concept rdf:ID="Diggingin">
<rdfs:label xml:lang="en">Digging in</rdfs:label>
<foaf:name>Digging in</foaf:name>
<skos:prefLabel xml:lang="en">Digging in</skos:prefLabel>
<skos:definition xml:lang="en">Digging trenches and dugouts in a captured position.</skos:definition>
<skos:inScheme rdf:resource="#OverTheTopDictionary"/>
<rdfs:isDefinedBy rdf:resource="http://rdf.muninn-project.org/ontologies/ott"/>
<rdf:type rdf:resource="http://dbpedia.org/resource/Irony"/>
<vs:term_status>Stable</vs:term_status>
</skos:Concept>
<skos:Concept rdf:ID="DiggingParty">
<rdfs:label xml:lang="en">Digging Party</rdfs:label>
<foaf:name>Digging Party</foaf:name>
<skos:prefLabel xml:lang="en">Digging Party</skos:prefLabel>
<skos:definition xml:lang="en">A detail of men told off to dig trenches, graves, or dugouts. Tommy is not particular as to what he has to dig; it&apos;s the actual digging he objects to.</skos:definition>
<skos:inScheme rdf:resource="#OverTheTopDictionary"/>
<rdfs:isDefinedBy rdf:resource="http://rdf.muninn-project.org/ontologies/ott"/>
<rdf:type rdf:resource="http://dbpedia.org/resource/Irony"/>
<vs:term_status>Stable</vs:term_status>
</skos:Concept>
<skos:Concept rdf:ID="Dinnerup">
<rdfs:label xml:lang="en">Dinner up</rdfs:label>
<foaf:name>Dinner up</foaf:name>
<skos:prefLabel xml:lang="en">Dinner up</skos:prefLabel>
<skos:definition xml:lang="en">Dinner is ready.</skos:definition>
<skos:inScheme rdf:resource="#OverTheTopDictionary"/>
<rdfs:isDefinedBy rdf:resource="http://rdf.muninn-project.org/ontologies/ott"/>
<rdf:type rdf:resource="http://dbpedia.org/resource/Irony"/>
<vs:term_status>Stable</vs:term_status>
</skos:Concept>
<skos:Concept rdf:ID="DivisionalBand">
<rdfs:label xml:lang="en">Divisional Band</rdfs:label>
<foaf:name>Divisional Band</foaf:name>
<skos:prefLabel xml:lang="en">Divisional Band</skos:prefLabel>
<skos:definition xml:lang="en">Another devilish aggregation which wastes moat of its time in practicing and polishing its instruments.</skos:definition>
<skos:inScheme rdf:resource="#OverTheTopDictionary"/>
<rdfs:isDefinedBy rdf:resource="http://rdf.muninn-project.org/ontologies/ott"/>
<rdf:type rdf:resource="http://dbpedia.org/resource/Irony"/>
<vs:term_status>Stable</vs:term_status>
</skos:Concept>
<skos:Concept rdf:ID="Dixie">
<rdfs:label xml:lang="en">Dixie</rdfs:label>
<foaf:name>Dixie</foaf:name>
<skos:prefLabel xml:lang="en">Dixie</skos:prefLabel>
<skos:definition xml:lang="en">An iron pot with two handles on it in which Tommy&apos;s meals are cooked. Its real efficiency lies in the fact that when carrying it, your puttees absorb all the black grease on its sides.</skos:definition>
<skos:inScheme rdf:resource="#OverTheTopDictionary"/>
<rdfs:isDefinedBy rdf:resource="http://rdf.muninn-project.org/ontologies/ott"/>
<rdf:type rdf:resource="http://dbpedia.org/resource/Irony"/>
<vs:term_status>Stable</vs:term_status>
</skos:Concept>
<skos:Concept rdf:ID="Doingthemin">
<rdfs:label xml:lang="en">Doing them in</rdfs:label>
<foaf:name>Doing them in</foaf:name>
<skos:prefLabel xml:lang="en">Doing them in</skos:prefLabel>
<skos:definition xml:lang="en">Killing them. Cutting up a body of German troops.</skos:definition>
<skos:inScheme rdf:resource="#OverTheTopDictionary"/>
<rdfs:isDefinedBy rdf:resource="http://rdf.muninn-project.org/ontologies/ott"/>
<rdf:type rdf:resource="http://dbpedia.org/resource/Irony"/>
<vs:term_status>Stable</vs:term_status>
<rdf:type rdf:resource="http://dbpedia.org/resource/Slang"/>
</skos:Concept>
<skos:Concept rdf:ID="Donkey">
<rdfs:label xml:lang="en">Donkey</rdfs:label>
<foaf:name>Donkey</foaf:name>
<skos:prefLabel xml:lang="en">Donkey</skos:prefLabel>
<skos:definition xml:lang="en">An army mule. An animal for which Tommy has the greatest respect. He never pets or in any way becomes familiar with said mule.</skos:definition>
<skos:inScheme rdf:resource="#OverTheTopDictionary"/>
<rdfs:isDefinedBy rdf:resource="http://rdf.muninn-project.org/ontologies/ott"/>
<rdf:type rdf:resource="http://dbpedia.org/resource/Irony"/>
<vs:term_status>Stable</vs:term_status>
</skos:Concept>
<skos:Concept rdf:ID="Draft">
<rdfs:label xml:lang="en">Draft</rdfs:label>
<foaf:name>Draft</foaf:name>
<skos:prefLabel xml:lang="en">Draft</skos:prefLabel>
<skos:definition xml:lang="en">A contingent of new men sent as reinforcements for the trenches. Tommy takes special delight in scaring these men with tales of his own experiences which he never had.</skos:definition>
<skos:inScheme rdf:resource="#OverTheTopDictionary"/>
<rdfs:isDefinedBy rdf:resource="http://rdf.muninn-project.org/ontologies/ott"/>
<rdf:type rdf:resource="http://dbpedia.org/resource/Irony"/>
<vs:term_status>Stable</vs:term_status>
</skos:Concept>
<skos:Concept rdf:ID="Draftman">
<rdfs:label xml:lang="en">Draftman</rdfs:label>
<foaf:name>Draftman</foaf:name>
<skos:prefLabel xml:lang="en">Draftman</skos:prefLabel>
<skos:definition xml:lang="en">A member of a draft who listens to and believes Tommy&apos;s weird tales of trench warfare.</skos:definition>
<skos:inScheme rdf:resource="#OverTheTopDictionary"/>
<rdfs:isDefinedBy rdf:resource="http://rdf.muninn-project.org/ontologies/ott"/>
<rdf:type rdf:resource="http://dbpedia.org/resource/Irony"/>
<vs:term_status>Stable</vs:term_status>
</skos:Concept>
<skos:Concept rdf:ID="DressingStation">
<rdfs:label xml:lang="en">Dressing Station</rdfs:label>
<foaf:name>Dressing Station</foaf:name>
<skos:prefLabel xml:lang="en">Dressing Station</skos:prefLabel>
<skos:definition xml:lang="en">A medical post where Tommy gets his wounds attended to, if he is lucky enough to get wounded. He is &quot;lucky,&quot; because a wound means Blighty.</skos:definition>
<skos:inScheme rdf:resource="#OverTheTopDictionary"/>
<rdfs:isDefinedBy rdf:resource="http://rdf.muninn-project.org/ontologies/ott"/>
<rdf:type rdf:resource="http://dbpedia.org/resource/Irony"/>
<vs:term_status>Stable</vs:term_status>
</skos:Concept>
<skos:Concept rdf:ID="Drillorder">
<rdfs:label xml:lang="en">Drill order</rdfs:label>
<foaf:name>Drill order</foaf:name>
<skos:prefLabel xml:lang="en">Drill order</skos:prefLabel>
<skos:definition xml:lang="en">Rifle, belt, bayonet, and respirator.</skos:definition>
<skos:inScheme rdf:resource="#OverTheTopDictionary"/>
<rdfs:isDefinedBy rdf:resource="http://rdf.muninn-project.org/ontologies/ott"/>
<rdf:type rdf:resource="http://dbpedia.org/resource/Irony"/>
<vs:term_status>Stable</vs:term_status>
</skos:Concept>
<skos:Concept rdf:ID="DryCanteen">
<rdfs:label xml:lang="en">Dry Canteen</rdfs:label>
<foaf:name>Dry Canteen</foaf:name>
<skos:prefLabel xml:lang="en">Dry Canteen</skos:prefLabel>
<skos:definition xml:lang="en">An army store where Tommy may buy cigarettes, chocolate, and tinned fruit, that is, if he has any money.</skos:definition>
<skos:inScheme rdf:resource="#OverTheTopDictionary"/>
<rdfs:isDefinedBy rdf:resource="http://rdf.muninn-project.org/ontologies/ott"/>
<rdf:type rdf:resource="http://dbpedia.org/resource/Irony"/>
<vs:term_status>Stable</vs:term_status>
</skos:Concept>
<skos:Concept rdf:ID="DistinguishedServiceOrder">
<rdfs:label xml:lang="en">Distinguished Service Order</rdfs:label>
<muninn:acronym xml:lang="en">D.S.O.</muninn:acronym>
<foaf:name>Distinguished Service Order</foaf:name>
<skos:prefLabel xml:lang="en">Distinguished Service Order</skos:prefLabel>
<skos:definition xml:lang="en">Another piece of metal issued to officers for being brave. Tommy says it is mostly won in dugouts and calls it a &quot;Dugout Service Order.&quot;</skos:definition>
<skos:inScheme rdf:resource="#OverTheTopDictionary"/>
<rdfs:isDefinedBy rdf:resource="http://rdf.muninn-project.org/ontologies/ott"/>
<rdf:type rdf:resource="http://dbpedia.org/resource/Irony"/>
<vs:term_status>Stable</vs:term_status>
</skos:Concept>
<skos:Concept rdf:ID="Dubbin">
<rdfs:label xml:lang="en">Dubbin</rdfs:label>
<foaf:name>Dubbin</foaf:name>
<skos:prefLabel xml:lang="en">Dubbin</skos:prefLabel>
<skos:definition xml:lang="en">A grease for boots.</skos:definition>
<skos:inScheme rdf:resource="#OverTheTopDictionary"/>
<rdfs:isDefinedBy rdf:resource="http://rdf.muninn-project.org/ontologies/ott"/>
<rdf:type rdf:resource="http://dbpedia.org/resource/Irony"/>
<vs:term_status>Stable</vs:term_status>
<rdf:type rdf:resource="http://dbpedia.org/resource/Slang"/>
</skos:Concept>
<skos:Concept rdf:ID="Dud">
<rdfs:label xml:lang="en">Dud</rdfs:label>
<foaf:name>Dud</foaf:name>
<skos:prefLabel xml:lang="en">Dud</skos:prefLabel>
<skos:definition xml:lang="en">A German shell or bomb which has not exploded on account of a defective fuse. Tommy is a great souvenir collector so he gathers these &quot;duds.&quot; Sometimes when he tries to unscrew the nose-cap it sticks. Then in his hurry to confiscate it before an officer appears he doesn&apos;t hammer it just right-and the printer of the casualty list has to use a little more type.</skos:definition>
<skos:inScheme rdf:resource="#OverTheTopDictionary"/>
<rdfs:isDefinedBy rdf:resource="http://rdf.muninn-project.org/ontologies/ott"/>
<rdf:type rdf:resource="http://dbpedia.org/resource/Irony"/>
<vs:term_status>Stable</vs:term_status>
<rdf:type rdf:resource="http://dbpedia.org/resource/Slang"/>
</skos:Concept>
<skos:Concept rdf:ID="Dugout">
<rdfs:label xml:lang="en">Dugout</rdfs:label>
<foaf:name>Dugout</foaf:name>
<skos:prefLabel xml:lang="en">Dugout</skos:prefLabel>
<skos:definition xml:lang="en">A deep hole in the trenches dug by the Royal Engineer Corps; supposed to be shell proof. It is, until a shell hits it. Rat and Tommy find it an excellent habitation in which to contract rheumatism.</skos:definition>
<skos:inScheme rdf:resource="#OverTheTopDictionary"/>
<rdfs:isDefinedBy rdf:resource="http://rdf.muninn-project.org/ontologies/ott"/>
<rdf:type rdf:resource="http://dbpedia.org/resource/Irony"/>
<vs:term_status>Stable</vs:term_status>
</skos:Concept>
<skos:Concept rdf:ID="Dump">
<rdfs:label xml:lang="en">Dump</rdfs:label>
<foaf:name>Dump</foaf:name>
<skos:prefLabel xml:lang="en">Dump</skos:prefLabel>
<skos:definition xml:lang="en">An uncovered spot where trench tools and supplies are placed. It is uncovered so that these will become rusty and worthless from the elements. This so that the contractors at home won&apos;t starve.</skos:definition>
<skos:inScheme rdf:resource="#OverTheTopDictionary"/>
<rdfs:isDefinedBy rdf:resource="http://rdf.muninn-project.org/ontologies/ott"/>
<rdf:type rdf:resource="http://dbpedia.org/resource/Irony"/>
<vs:term_status>Stable</vs:term_status>
</skos:Concept>
<skos:Concept rdf:ID="EfficiencyPay">
<rdfs:label xml:lang="en">Efficiency Pay</rdfs:label>
<foaf:name>Efficiency Pay</foaf:name>
<skos:prefLabel xml:lang="en">Efficiency Pay</skos:prefLabel>
<skos:definition xml:lang="en">Extra pay allowed by the Government for long service. Tommy is very efficient if he manages to get it from the Government.</skos:definition>
<skos:inScheme rdf:resource="#OverTheTopDictionary"/>
<rdfs:isDefinedBy rdf:resource="http://rdf.muninn-project.org/ontologies/ott"/>
<rdf:type rdf:resource="http://dbpedia.org/resource/Irony"/>
<vs:term_status>Stable</vs:term_status>
</skos:Concept>
<skos:Concept rdf:ID="EighteenPounder">
<rdfs:label xml:lang="en">Eighteen-Pounder</rdfs:label>
<foaf:name>Eighteen-Pounder</foaf:name>
<skos:prefLabel xml:lang="en">Eighteen-Pounder</skos:prefLabel>
<skos:definition xml:lang="en">One of our guns which fires an eighteen pound shell, used for destroying German barbed wire previous to an attack. If it does its duty you bet Tommy is grateful to the eighteen-pounders.</skos:definition>
<skos:inScheme rdf:resource="#OverTheTopDictionary"/>
<rdfs:isDefinedBy rdf:resource="http://rdf.muninn-project.org/ontologies/ott"/>
<rdf:type rdf:resource="http://dbpedia.org/resource/Irony"/>
<vs:term_status>Stable</vs:term_status>
</skos:Concept>
<skos:Concept rdf:ID="ElephantDugout">
<rdfs:label xml:lang="en">Elephant Dugout</rdfs:label>
<foaf:name>Elephant Dugout</foaf:name>
<skos:prefLabel xml:lang="en">Elephant Dugout</skos:prefLabel>
<skos:definition xml:lang="en">A large, safe, and roomy dugout, braced by heavy steel ribs or girders.</skos:definition>
<skos:inScheme rdf:resource="#OverTheTopDictionary"/>
<rdfs:isDefinedBy rdf:resource="http://rdf.muninn-project.org/ontologies/ott"/>
<rdf:type rdf:resource="http://dbpedia.org/resource/Irony"/>
<vs:term_status>Stable</vs:term_status>
</skos:Concept>
<skos:Concept rdf:ID="Emplacement">
<rdfs:label xml:lang="en">Emplacement</rdfs:label>
<foaf:name>Emplacement</foaf:name>
<skos:prefLabel xml:lang="en">Emplacement</skos:prefLabel>
<skos:definition xml:lang="en">A position made of earth or sandbags from which a machine gun is fired. It is supposed to be invisible to the enemy. They generally blow it up in the course of a couple of days, just by luck, of course.</skos:definition>
<skos:inScheme rdf:resource="#OverTheTopDictionary"/>
<rdfs:isDefinedBy rdf:resource="http://rdf.muninn-project.org/ontologies/ott"/>
<rdf:type rdf:resource="http://dbpedia.org/resource/Irony"/>
<vs:term_status>Stable</vs:term_status>
</skos:Concept>
<skos:Concept rdf:ID="EntrenchingTool">
<rdfs:label xml:lang="en">Entrenching Tool</rdfs:label>
<foaf:name>Entrenching Tool</foaf:name>
<skos:prefLabel xml:lang="en">Entrenching Tool</skos:prefLabel>
<skos:definition xml:lang="en">A spade-like tool for digging hasty entrenchments. It takes about a week to dig a decent hole with it, so &quot;hasty&quot; must have another meaning.</skos:definition>
<skos:inScheme rdf:resource="#OverTheTopDictionary"/>
<rdfs:isDefinedBy rdf:resource="http://rdf.muninn-project.org/ontologies/ott"/>
<rdf:type rdf:resource="http://dbpedia.org/resource/Irony"/>
<vs:term_status>Stable</vs:term_status>
</skos:Concept>
<skos:Concept rdf:ID="Equipmenton">
<rdfs:label xml:lang="en">Equipment on</rdfs:label>
<foaf:name>Equipment on</foaf:name>
<skos:prefLabel xml:lang="en">Equipment on</skos:prefLabel>
<skos:definition xml:lang="en">Put on equipment for drill or parade.</skos:definition>
<skos:inScheme rdf:resource="#OverTheTopDictionary"/>
<rdfs:isDefinedBy rdf:resource="http://rdf.muninn-project.org/ontologies/ott"/>
<rdf:type rdf:resource="http://dbpedia.org/resource/Irony"/>
<vs:term_status>Stable</vs:term_status>
</skos:Concept>
<skos:Concept rdf:ID="Escort">
<rdfs:label xml:lang="en">Escort</rdfs:label>
<foaf:name>Escort</foaf:name>
<skos:prefLabel xml:lang="en">Escort</skos:prefLabel>
<skos:definition xml:lang="en">A guard of soldiers who conduct prisoners to different points. Tommy is just as liable to be a prisoner as an escort.</skos:definition>
<skos:inScheme rdf:resource="#OverTheTopDictionary"/>
<rdfs:isDefinedBy rdf:resource="http://rdf.muninn-project.org/ontologies/ott"/>
<rdf:type rdf:resource="http://dbpedia.org/resource/Irony"/>
<vs:term_status>Stable</vs:term_status>
</skos:Concept>
<skos:Concept rdf:ID="Fag">
<rdfs:label xml:lang="en">Fag</rdfs:label>
<foaf:name>Fag</foaf:name>
<skos:prefLabel xml:lang="en">Fag</skos:prefLabel>
<skos:definition xml:lang="en">Cigarette. Something Tommy is always touching you for, &quot;Fag issue.&quot; Army issue of cigarettes, generally on Sunday.</skos:definition>
<skos:inScheme rdf:resource="#OverTheTopDictionary"/>
<rdfs:isDefinedBy rdf:resource="http://rdf.muninn-project.org/ontologies/ott"/>
<rdf:type rdf:resource="http://dbpedia.org/resource/Irony"/>
<vs:term_status>Stable</vs:term_status>
<rdf:type rdf:resource="http://dbpedia.org/resource/Slang"/>
</skos:Concept>
<skos:Concept rdf:ID="Fatigue">
<rdfs:label xml:lang="en">Fatigue</rdfs:label>
<foaf:name>Fatigue</foaf:name>
<skos:prefLabel xml:lang="en">Fatigue</skos:prefLabel>
<skos:definition xml:lang="en">Various kinds of work done by Tommy while he is &quot;resting.&quot;</skos:definition>
<skos:inScheme rdf:resource="#OverTheTopDictionary"/>
<rdfs:isDefinedBy rdf:resource="http://rdf.muninn-project.org/ontologies/ott"/>
<rdf:type rdf:resource="http://dbpedia.org/resource/Irony"/>
<vs:term_status>Stable</vs:term_status>
</skos:Concept>
<skos:Concept rdf:ID="Fedup">
<rdfs:label xml:lang="en">Fed up</rdfs:label>
<foaf:name>Fed up</foaf:name>
<skos:prefLabel xml:lang="en">Fed up</skos:prefLabel>
<skos:definition xml:lang="en">Disgusted; got enough of it -- as the rich Mr. Hoggenheimer used to say, &quot;Sufficiency.&quot;</skos:definition>
<skos:inScheme rdf:resource="#OverTheTopDictionary"/>
<rdfs:isDefinedBy rdf:resource="http://rdf.muninn-project.org/ontologies/ott"/>
<rdf:type rdf:resource="http://dbpedia.org/resource/Irony"/>
<vs:term_status>Stable</vs:term_status>
</skos:Concept>
<skos:Concept rdf:ID="FieldDressing">
<rdfs:label xml:lang="en">Field Dressing</rdfs:label>
<foaf:name>Field Dressing</foaf:name>
<skos:prefLabel xml:lang="en">Field Dressing</skos:prefLabel>
<skos:definition xml:lang="en">Bandages issued to soldiers for first aid when wounded. They use them for handkerchiefs and to clean their rifles.</skos:definition>
<skos:inScheme rdf:resource="#OverTheTopDictionary"/>
<rdfs:isDefinedBy rdf:resource="http://rdf.muninn-project.org/ontologies/ott"/>
<rdf:type rdf:resource="http://dbpedia.org/resource/Irony"/>
<vs:term_status>Stable</vs:term_status>
</skos:Concept>
<skos:Concept rdf:ID="FieldPostCard">
<rdfs:label xml:lang="en">Field Post Card</rdfs:label>
<foaf:name>Field Post Card</foaf:name>
<skos:prefLabel xml:lang="en">Field Post Card</skos:prefLabel>
<skos:definition xml:lang="en">A card on which Tommy is allowed to tell his family and friends that he is alive; if he is dead the War Office sends a card, sometimes.</skos:definition>
<skos:inScheme rdf:resource="#OverTheTopDictionary"/>
<rdfs:isDefinedBy rdf:resource="http://rdf.muninn-project.org/ontologies/ott"/>
<rdf:type rdf:resource="http://dbpedia.org/resource/Irony"/>
<vs:term_status>Stable</vs:term_status>
</skos:Concept>
<skos:Concept rdf:ID="FieldPunishmentNoI">
<rdfs:label xml:lang="en">Field Punishment No. I.</rdfs:label>
<foaf:name>Field Punishment No. I.</foaf:name>
<skos:prefLabel xml:lang="en">Field Punishment No. I.</skos:prefLabel>
<skos:definition xml:lang="en">Official name for spread-eagling a man on a limber wheel, two hours a day for twenty-one days. His rations consist of bully beef, water, and biscuits. Tommy calls this punishment &quot;Crucifixion,&quot; especially if he has undergone it.</skos:definition>
<skos:inScheme rdf:resource="#OverTheTopDictionary"/>
<rdfs:isDefinedBy rdf:resource="http://rdf.muninn-project.org/ontologies/ott"/>
<rdf:type rdf:resource="http://dbpedia.org/resource/Irony"/>
<vs:term_status>Stable</vs:term_status>
</skos:Concept>
<skos:Concept rdf:ID="FifteenPounder">
<rdfs:label xml:lang="en">Fifteen-pounder</rdfs:label>
<foaf:name>Fifteen-pounder</foaf:name>
<skos:prefLabel xml:lang="en">Fifteen-pounder</skos:prefLabel>
<skos:definition xml:lang="en">Still another of ours; shell weighs fifteen pounds. Used for killing rats on the German parapets.</skos:definition>
<skos:inScheme rdf:resource="#OverTheTopDictionary"/>
<rdfs:isDefinedBy rdf:resource="http://rdf.muninn-project.org/ontologies/ott"/>
<rdf:type rdf:resource="http://dbpedia.org/resource/Irony"/>
<vs:term_status>Stable</vs:term_status>
</skos:Concept>
<skos:Concept rdf:ID="Findingtherange">
<rdfs:label xml:lang="en">Finding the range</rdfs:label>
<foaf:name>Finding the range</foaf:name>
<skos:prefLabel xml:lang="en">Finding the range</skos:prefLabel>
<skos:definition xml:lang="en">Ascertaining by instrument or by trial shots the distance from an enemy objective.</skos:definition>
<skos:inScheme rdf:resource="#OverTheTopDictionary"/>
<rdfs:isDefinedBy rdf:resource="http://rdf.muninn-project.org/ontologies/ott"/>
<rdf:type rdf:resource="http://dbpedia.org/resource/Irony"/>
<vs:term_status>Stable</vs:term_status>
</skos:Concept>
<skos:Concept rdf:ID="Fireworks">
<rdfs:label xml:lang="en">Fireworks</rdfs:label>
<foaf:name>Fireworks</foaf:name>
<skos:prefLabel xml:lang="en">Fireworks</skos:prefLabel>
<skos:definition xml:lang="en">A night bombardment.</skos:definition>
<skos:inScheme rdf:resource="#OverTheTopDictionary"/>
<rdfs:isDefinedBy rdf:resource="http://rdf.muninn-project.org/ontologies/ott"/>
<rdf:type rdf:resource="http://dbpedia.org/resource/Irony"/>
<vs:term_status>Stable</vs:term_status>
</skos:Concept>
<skos:Concept rdf:ID="FireSector">
<rdfs:label xml:lang="en">Fire Sector</rdfs:label>
<foaf:name>Fire Sector</foaf:name>
<skos:prefLabel xml:lang="en">Fire Sector</skos:prefLabel>
<skos:definition xml:lang="en">A certain space of ground which a machine gun is supposed to sweep with its fire. If the gun refuses to work, all of the enemy who cross this space are technically dead, according to the General&apos;s plans.</skos:definition>
<skos:inScheme rdf:resource="#OverTheTopDictionary"/>
<rdfs:isDefinedBy rdf:resource="http://rdf.muninn-project.org/ontologies/ott"/>
<rdf:type rdf:resource="http://dbpedia.org/resource/Irony"/>
<vs:term_status>Stable</vs:term_status>
</skos:Concept>
<skos:Concept rdf:ID="FiringSquad">
<rdfs:label xml:lang="en">Firing Squad</rdfs:label>
<foaf:name>Firing Squad</foaf:name>
<skos:prefLabel xml:lang="en">Firing Squad</skos:prefLabel>
<skos:definition xml:lang="en">Twelve men picked to shoot a soldier who has been sentenced to death by court-martial. Tommy has no comment to make on this.</skos:definition>
<skos:inScheme rdf:resource="#OverTheTopDictionary"/>
<rdfs:isDefinedBy rdf:resource="http://rdf.muninn-project.org/ontologies/ott"/>
<rdf:type rdf:resource="http://dbpedia.org/resource/Irony"/>
<vs:term_status>Stable</vs:term_status>
</skos:Concept>
<skos:Concept rdf:ID="FiringStep">
<rdfs:label xml:lang="en">Firing Step</rdfs:label>
<foaf:name>Firing Step</foaf:name>
<skos:prefLabel xml:lang="en">Firing Step</skos:prefLabel>
<skos:definition xml:lang="en">A ledge in the front trench which enables Tommy to fire &quot;over the top.&quot; In rainy weather you have to be an acrobat to even stand on it on account of the slippery mud.</skos:definition>
<skos:inScheme rdf:resource="#OverTheTopDictionary"/>
<rdfs:isDefinedBy rdf:resource="http://rdf.muninn-project.org/ontologies/ott"/>
<rdf:type rdf:resource="http://dbpedia.org/resource/Irony"/>
<vs:term_status>Stable</vs:term_status>
</skos:Concept>
<skos:Concept rdf:ID="FireTrench">
<rdfs:label xml:lang="en">Fire Trench</rdfs:label>
<foaf:name>Fire Trench</foaf:name>
<skos:prefLabel xml:lang="en">Fire Trench</skos:prefLabel>
<skos:definition xml:lang="en">The front-line trench. Another name is for Hell.</skos:definition>
<skos:inScheme rdf:resource="#OverTheTopDictionary"/>
<rdfs:isDefinedBy rdf:resource="http://rdf.muninn-project.org/ontologies/ott"/>
<rdf:type rdf:resource="http://dbpedia.org/resource/Irony"/>
<vs:term_status>Stable</vs:term_status>
</skos:Concept>
<skos:Concept rdf:ID="Fiveroundsrapid">
<rdfs:label xml:lang="en">Five rounds rapid</rdfs:label>
<foaf:name>Five rounds rapid</foaf:name>
<skos:prefLabel xml:lang="en">Five rounds rapid</skos:prefLabel>
<skos:definition xml:lang="en">Generally, just before daylight in the trenches, the order &quot;Five rounds rapid&quot; is given. Each man puts his rifle and head over the parapet and fires five shots as rapidly as possible in the direction of the German trenches and then ducks. A sort of &quot;Good morning, have you used Fears Soap?&quot;</skos:definition>
<skos:inScheme rdf:resource="#OverTheTopDictionary"/>
<rdfs:isDefinedBy rdf:resource="http://rdf.muninn-project.org/ontologies/ott"/>
<rdf:type rdf:resource="http://dbpedia.org/resource/Irony"/>
<vs:term_status>Stable</vs:term_status>
</skos:Concept>
<skos:Concept rdf:ID="Fivenine">
<rdfs:label xml:lang="en">Five nine</rdfs:label>
<foaf:name>Five nine</foaf:name>
<skos:prefLabel xml:lang="en">Five nine</skos:prefLabel>
<skos:definition xml:lang="en">A German shell 5.9 inches in diameter. It is their standard shell. Tommy has no special love for this brand, but they are like olives, all right when you get used to them.</skos:definition>
<skos:inScheme rdf:resource="#OverTheTopDictionary"/>
<rdfs:isDefinedBy rdf:resource="http://rdf.muninn-project.org/ontologies/ott"/>
<rdf:type rdf:resource="http://dbpedia.org/resource/Irony"/>
<vs:term_status>Stable</vs:term_status>
<rdf:type rdf:resource="http://dbpedia.org/resource/Slang"/>
</skos:Concept>
<skos:Concept rdf:ID="Flags">
<rdfs:label xml:lang="en">Flags</rdfs:label>
<foaf:name>Flags</foaf:name>
<skos:prefLabel xml:lang="en">Flags</skos:prefLabel>
<skos:definition xml:lang="en">Tommy&apos;s nickname for a Signaler.</skos:definition>
<skos:inScheme rdf:resource="#OverTheTopDictionary"/>
<rdfs:isDefinedBy rdf:resource="http://rdf.muninn-project.org/ontologies/ott"/>
<rdf:type rdf:resource="http://dbpedia.org/resource/Irony"/>
<vs:term_status>Stable</vs:term_status>
</skos:Concept>
<skos:Concept rdf:ID="Flare">
<rdfs:label xml:lang="en">Flare</rdfs:label>
<foaf:name>Flare</foaf:name>
<skos:prefLabel xml:lang="en">Flare</skos:prefLabel>
<skos:definition xml:lang="en">A rocket fired from a pistol which, at night, lights up the ground in front of your trench.</skos:definition>
<skos:inScheme rdf:resource="#OverTheTopDictionary"/>
<rdfs:isDefinedBy rdf:resource="http://rdf.muninn-project.org/ontologies/ott"/>
<rdf:type rdf:resource="http://dbpedia.org/resource/Irony"/>
<vs:term_status>Stable</vs:term_status>
</skos:Concept>
<skos:Concept rdf:ID="FlarePistol">
<rdfs:label xml:lang="en">Flare Pistol</rdfs:label>
<foaf:name>Flare Pistol</foaf:name>
<skos:prefLabel xml:lang="en">Flare Pistol</skos:prefLabel>
<skos:definition xml:lang="en">A large pistol, which looks like a sawed-off shotgun, from which flares are fired. When you need this pistol badly it has generally been left in your dugout.</skos:definition>
<skos:inScheme rdf:resource="#OverTheTopDictionary"/>
<rdfs:isDefinedBy rdf:resource="http://rdf.muninn-project.org/ontologies/ott"/>
<rdf:type rdf:resource="http://dbpedia.org/resource/Irony"/>
<vs:term_status>Stable</vs:term_status>
</skos:Concept>
<skos:Concept rdf:ID="FlyingColumn">
<rdfs:label xml:lang="en">Flying Column</rdfs:label>
<foaf:name>Flying Column</foaf:name>
<skos:prefLabel xml:lang="en">Flying Column</skos:prefLabel>
<skos:definition xml:lang="en">A flying column of troops that waits from one point of the line to another. In case of need they usually arrive at the wrong point.</skos:definition>
<skos:inScheme rdf:resource="#OverTheTopDictionary"/>
<rdfs:isDefinedBy rdf:resource="http://rdf.muninn-project.org/ontologies/ott"/>
<rdf:type rdf:resource="http://dbpedia.org/resource/Irony"/>
<vs:term_status>Stable</vs:term_status>
<rdf:type rdf:resource="http://dbpedia.org/resource/Slang"/>
</skos:Concept>
<skos:Concept rdf:ID="Fokker">
<rdfs:label xml:lang="en">Fokker</rdfs:label>
<foaf:name>Fokker</foaf:name>
<skos:prefLabel xml:lang="en">Fokker</skos:prefLabel>
<skos:definition xml:lang="en">A type of German aeroplane which the Boche claims to be the fastest in the world. Tommy believes this, because our airmen seldom catch them.</skos:definition>
<skos:inScheme rdf:resource="#OverTheTopDictionary"/>
<rdfs:isDefinedBy rdf:resource="http://rdf.muninn-project.org/ontologies/ott"/>
<rdf:type rdf:resource="http://dbpedia.org/resource/Irony"/>
<vs:term_status>Stable</vs:term_status>
</skos:Concept>
<skos:Concept rdf:ID="ForIt">
<rdfs:label xml:lang="en">For It</rdfs:label>
<foaf:name>For It</foaf:name>
<skos:prefLabel xml:lang="en">For It</skos:prefLabel>
<skos:definition xml:lang="en">On the crime sheet; up against a reprimand; on trial, in trouble.</skos:definition>
<skos:inScheme rdf:resource="#OverTheTopDictionary"/>
<rdfs:isDefinedBy rdf:resource="http://rdf.muninn-project.org/ontologies/ott"/>
<rdf:type rdf:resource="http://dbpedia.org/resource/Irony"/>
<rdf:type rdf:resource="http://dbpedia.org/resource/Slang"/>
<vs:term_status>Stable</vs:term_status>
</skos:Concept>
<skos:Concept rdf:ID="Fourbytwo">
<rdfs:label xml:lang="en">Four by two</rdfs:label>
<foaf:name>Four by two</foaf:name>
<skos:prefLabel xml:lang="en">Four by two</skos:prefLabel>
<skos:definition xml:lang="en">A piece of flannel four Inches by two issued by the Q. M. Sergeant with which to &quot;pull through.&quot;</skos:definition>
<skos:inScheme rdf:resource="#OverTheTopDictionary"/>
<rdfs:isDefinedBy rdf:resource="http://rdf.muninn-project.org/ontologies/ott"/>
<rdf:type rdf:resource="http://dbpedia.org/resource/Irony"/>
<rdf:type rdf:resource="http://dbpedia.org/resource/Slang"/>
<vs:term_status>Stable</vs:term_status>
</skos:Concept>
<skos:Concept rdf:ID="Fourpointfive">
<rdfs:label xml:lang="en">Four point five</rdfs:label>
<foaf:name>Four point five</foaf:name>
<skos:prefLabel xml:lang="en">Four point five</skos:prefLabel>
<skos:definition xml:lang="en">Another of ours. The Germans don&apos;t like this one.</skos:definition>
<skos:inScheme rdf:resource="#OverTheTopDictionary"/>
<rdfs:isDefinedBy rdf:resource="http://rdf.muninn-project.org/ontologies/ott"/>
<rdf:type rdf:resource="http://dbpedia.org/resource/Irony"/>
<rdf:type rdf:resource="http://dbpedia.org/resource/Slang"/>
<vs:term_status>Stable</vs:term_status>
</skos:Concept>
<skos:Concept rdf:ID="Fourpointseven">
<rdfs:label xml:lang="en">Four point seven</rdfs:label>
<foaf:name>Four point seven</foaf:name>
<skos:prefLabel xml:lang="en">Four point seven</skos:prefLabel>
<skos:definition xml:lang="en">One of our shells 4.7 inches in diameter. Tommy likes this kind.</skos:definition>
<skos:inScheme rdf:resource="#OverTheTopDictionary"/>
<rdfs:isDefinedBy rdf:resource="http://rdf.muninn-project.org/ontologies/ott"/>
<rdf:type rdf:resource="http://dbpedia.org/resource/Slang"/>
<rdf:type rdf:resource="http://dbpedia.org/resource/Irony"/>
<vs:term_status>Stable</vs:term_status>
</skos:Concept>
<skos:Concept rdf:ID="Fritz">
<rdfs:label xml:lang="en">Fritz</rdfs:label>
<foaf:name>Fritz</foaf:name>
<skos:prefLabel xml:lang="en">Fritz</skos:prefLabel>
<skos:definition xml:lang="en">Tommy&apos;s name for a German. He loves a German like poison.</skos:definition>
<skos:inScheme rdf:resource="#OverTheTopDictionary"/>
<rdfs:isDefinedBy rdf:resource="http://rdf.muninn-project.org/ontologies/ott"/>
<rdf:type rdf:resource="http://dbpedia.org/resource/Irony"/>
<rdf:type rdf:resource="http://dbpedia.org/resource/Slang"/>
<rdf:type rdf:resource="http://dbpedia.org/resource/Derogatory"/>
<vs:term_status>Stable</vs:term_status>
</skos:Concept>
<skos:Concept rdf:ID="FrontLine">
<rdfs:label xml:lang="en">Front Line</rdfs:label>
<foaf:name>Front Line</foaf:name>
<skos:prefLabel xml:lang="en">Front Line</skos:prefLabel>
<skos:definition xml:lang="en">The nearest trench to the enemy. No place for a conscientious objector.</skos:definition>
<skos:inScheme rdf:resource="#OverTheTopDictionary"/>
<rdfs:isDefinedBy rdf:resource="http://rdf.muninn-project.org/ontologies/ott"/>
<rdf:type rdf:resource="http://dbpedia.org/resource/Irony"/>
<vs:term_status>Stable</vs:term_status>
</skos:Concept>
<skos:Concept rdf:ID="Frostbite">
<rdfs:label xml:lang="en">Frostbite</rdfs:label>
<foaf:name>Frostbite</foaf:name>
<skos:prefLabel xml:lang="en">Frostbite</skos:prefLabel>
<skos:definition xml:lang="en">A quick road to Blighty, which Tommy used very often until frostbite became a court-martial offence. Now he keeps his feet warm.</skos:definition>
<skos:inScheme rdf:resource="#OverTheTopDictionary"/>
<rdfs:isDefinedBy rdf:resource="http://rdf.muninn-project.org/ontologies/ott"/>
<rdf:type rdf:resource="http://dbpedia.org/resource/Irony"/>
<vs:term_status>Stable</vs:term_status>
</skos:Concept>
<skos:Concept rdf:ID="Fullpack">
<rdfs:label xml:lang="en">Full pack</rdfs:label>
<foaf:name>Full pack</foaf:name>
<skos:prefLabel xml:lang="en">Full pack</skos:prefLabel>
<skos:definition xml:lang="en">A soldier carrying all of his equipment.</skos:definition>
<skos:inScheme rdf:resource="#OverTheTopDictionary"/>
<rdfs:isDefinedBy rdf:resource="http://rdf.muninn-project.org/ontologies/ott"/>
<rdf:type rdf:resource="http://dbpedia.org/resource/Irony"/>
<vs:term_status>Stable</vs:term_status>
</skos:Concept>
<skos:Concept rdf:ID="FullCorporal">
<rdfs:label xml:lang="en">Full Corporal</rdfs:label>
<foaf:name>Full Corporal</foaf:name>
<skos:prefLabel xml:lang="en">Full Corporal</skos:prefLabel>
<skos:definition xml:lang="en">A N.C.O. who sports two stripes on his arm and has more to say than the Colonel.</skos:definition>
<skos:inScheme rdf:resource="#OverTheTopDictionary"/>
<rdfs:isDefinedBy rdf:resource="http://rdf.muninn-project.org/ontologies/ott"/>
<rdf:type rdf:resource="http://dbpedia.org/resource/Irony"/>
<vs:term_status>Stable</vs:term_status>
</skos:Concept>
<skos:Concept rdf:ID="Fumigator">
<rdfs:label xml:lang="en">Fumigator</rdfs:label>
<foaf:name>Fumigator</foaf:name>
<skos:prefLabel xml:lang="en">Fumigator</skos:prefLabel>
<skos:definition xml:lang="en">An infernal device at a hospital which cooks Tommy&apos;s uniform and returns it to him two sizes too small.</skos:definition>
<skos:inScheme rdf:resource="#OverTheTopDictionary"/>
<rdfs:isDefinedBy rdf:resource="http://rdf.muninn-project.org/ontologies/ott"/>
<rdf:type rdf:resource="http://dbpedia.org/resource/Irony"/>
<vs:term_status>Stable</vs:term_status>
</skos:Concept>
<skos:Concept rdf:ID="FunkHole">
<rdfs:label xml:lang="en">Funk Hole</rdfs:label>
<foaf:name>Funk Hole</foaf:name>
<skos:prefLabel xml:lang="en">Funk Hole</skos:prefLabel>
<skos:definition xml:lang="en">Tommy&apos;s term for a dugout. A favorite spot for those of a nervous disposition.</skos:definition>
<skos:inScheme rdf:resource="#OverTheTopDictionary"/>
<rdfs:isDefinedBy rdf:resource="http://rdf.muninn-project.org/ontologies/ott"/>
<rdf:type rdf:resource="http://dbpedia.org/resource/Irony"/>
<rdf:type rdf:resource="http://dbpedia.org/resource/Slang"/>
<vs:term_status>Stable</vs:term_status>
</skos:Concept>
<skos:Concept rdf:ID="Fuse">
<rdfs:label xml:lang="en">Fuse</rdfs:label>
<foaf:name>Fuse</foaf:name>
<skos:prefLabel xml:lang="en">Fuse</skos:prefLabel>
<skos:definition xml:lang="en">A part of shell or bomb which burns in a set time and ignites the detonator.</skos:definition>
<skos:inScheme rdf:resource="#OverTheTopDictionary"/>
<rdfs:isDefinedBy rdf:resource="http://rdf.muninn-project.org/ontologies/ott"/>
<rdf:type rdf:resource="http://dbpedia.org/resource/Irony"/>
<vs:term_status>Stable</vs:term_status>
</skos:Concept>
<skos:Concept rdf:ID="Gas">
<rdfs:label xml:lang="en">Gas</rdfs:label>
<foaf:name>Gas</foaf:name>
<skos:prefLabel xml:lang="en">Gas</skos:prefLabel>
<skos:definition xml:lang="en">Poisonous fumes which the Germans send over to our trenches. When the wind is favorable this gas is discharged into the air from huge cylinders. The wind carries it over toward our lines. It appears like a huge yellowish-green cloud rolling along the ground. The alarm is sounded and Tommy promptly puts on his gas helmet and laughs at the Boches.</skos:definition>
<skos:inScheme rdf:resource="#OverTheTopDictionary"/>
<rdfs:isDefinedBy rdf:resource="http://rdf.muninn-project.org/ontologies/ott"/>
<rdf:type rdf:resource="http://dbpedia.org/resource/Irony"/>
<vs:term_status>Stable</vs:term_status>
</skos:Concept>
<skos:Concept rdf:ID="GasGong">
<rdfs:label xml:lang="en">Gas Gong</rdfs:label>
<foaf:name>Gas Gong</foaf:name>
<skos:prefLabel xml:lang="en">Gas Gong</skos:prefLabel>
<skos:definition xml:lang="en">An empty shell case hung up in the trenches and in billets. A sentry is posted near it, so that in case German poison gas comes over, he can give the alarm by striking this gong with an iron bar. If the sentry happens to be asleep we get &quot;gassed.&quot;</skos:definition>
<skos:inScheme rdf:resource="#OverTheTopDictionary"/>
<rdfs:isDefinedBy rdf:resource="http://rdf.muninn-project.org/ontologies/ott"/>
<rdf:type rdf:resource="http://dbpedia.org/resource/Irony"/>
<vs:term_status>Stable</vs:term_status>
</skos:Concept>
<skos:Concept rdf:ID="Gassed">
<rdfs:label xml:lang="en">Gassed</rdfs:label>
<foaf:name>Gassed</foaf:name>
<skos:prefLabel xml:lang="en">Gassed</skos:prefLabel>
<skos:definition xml:lang="en">A soldier who has been overcome from the fumes of German poison gas, or the hot air of a comrade.</skos:definition>
<skos:inScheme rdf:resource="#OverTheTopDictionary"/>
<rdfs:isDefinedBy rdf:resource="http://rdf.muninn-project.org/ontologies/ott"/>
<rdf:type rdf:resource="http://dbpedia.org/resource/Irony"/>
<vs:term_status>Stable</vs:term_status>
</skos:Concept>
<skos:Concept rdf:ID="Gassing">
<rdfs:label xml:lang="en">Gassing</rdfs:label>
<foaf:name>Gassing</foaf:name>
<skos:prefLabel xml:lang="en">Gassing</skos:prefLabel>
<skos:definition xml:lang="en">A term Tommy applies to &quot;shooting the bull.&quot;</skos:definition>
<skos:inScheme rdf:resource="#OverTheTopDictionary"/>
<rdfs:isDefinedBy rdf:resource="http://rdf.muninn-project.org/ontologies/ott"/>
<rdf:type rdf:resource="http://dbpedia.org/resource/Irony"/>
<vs:term_status>Stable</vs:term_status>
</skos:Concept>
<skos:Concept rdf:ID="Gettingasub">
<rdfs:label xml:lang="en">Getting a sub</rdfs:label>
<foaf:name>Getting a sub</foaf:name>
<skos:prefLabel xml:lang="en">Getting a sub</skos:prefLabel>
<skos:definition xml:lang="en">Touching an officer for money. To be taken out of soldier&apos;s pay on the next pay-day.</skos:definition>
<skos:inScheme rdf:resource="#OverTheTopDictionary"/>
<rdfs:isDefinedBy rdf:resource="http://rdf.muninn-project.org/ontologies/ott"/>
<rdf:type rdf:resource="http://dbpedia.org/resource/Irony"/>
<rdf:type rdf:resource="http://dbpedia.org/resource/Slang"/>
<vs:term_status>Stable</vs:term_status>
</skos:Concept>
<skos:Concept rdf:ID="Gettingthesparks">
<rdfs:label xml:lang="en">Getting the sparks</rdfs:label>
<foaf:name>Getting the sparks</foaf:name>
<skos:prefLabel xml:lang="en">Getting the sparks</skos:prefLabel>
<skos:definition xml:lang="en">Bullets from a machine gun cutting enemy barbed wire at night; when a bullet strikes wire it generally throws off a bluish spark. Machine gunners use this method at night to &quot;set&quot; their gun so that its fire will command the enemy&apos;s trench.</skos:definition>
<skos:inScheme rdf:resource="#OverTheTopDictionary"/>
<rdfs:isDefinedBy rdf:resource="http://rdf.muninn-project.org/ontologies/ott"/>
<rdf:type rdf:resource="http://dbpedia.org/resource/Irony"/>
<rdf:type rdf:resource="http://dbpedia.org/resource/Slang"/>
<vs:term_status>Stable</vs:term_status>
</skos:Concept>
<skos:Concept rdf:ID="Ginger">
<rdfs:label xml:lang="en">Ginger</rdfs:label>
<foaf:name>Ginger</foaf:name>
<skos:prefLabel xml:lang="en">Ginger</skos:prefLabel>
<skos:definition xml:lang="en">Nickname of a red-beaded soldier; courage; pep.</skos:definition>
<skos:inScheme rdf:resource="#OverTheTopDictionary"/>
<rdfs:isDefinedBy rdf:resource="http://rdf.muninn-project.org/ontologies/ott"/>
<rdf:type rdf:resource="http://dbpedia.org/resource/Irony"/>
<vs:term_status>Stable</vs:term_status>
</skos:Concept>
<skos:Concept rdf:ID="Gippo">
<rdfs:label xml:lang="en">Gippo</rdfs:label>
<foaf:name>Gippo</foaf:name>
<skos:prefLabel xml:lang="en">Gippo</skos:prefLabel>
<skos:definition xml:lang="en">Bacon grease; soup.</skos:definition>
<skos:inScheme rdf:resource="#OverTheTopDictionary"/>
<rdfs:isDefinedBy rdf:resource="http://rdf.muninn-project.org/ontologies/ott"/>
<rdf:type rdf:resource="http://dbpedia.org/resource/Irony"/>
<vs:term_status>Stable</vs:term_status>
<rdf:type rdf:resource="http://dbpedia.org/resource/Slang"/>
</skos:Concept>
<skos:Concept rdf:ID="GarrisonMilitaryPolice">
<rdfs:label xml:lang="en">Garrison Military Police</rdfs:label>
<muninn:acronym xml:lang="en">G.M.P.</muninn:acronym>
<foaf:name>Garrison Military Police</foaf:name>
<skos:prefLabel xml:lang="en">Garrison Military Police</skos:prefLabel>
<skos:definition xml:lang="en">Soldiers detailed to patrol the roads and regulate traffic behind the lines. Tommy&apos;s pet aversion.</skos:definition>
<skos:inScheme rdf:resource="#OverTheTopDictionary"/>
<rdfs:isDefinedBy rdf:resource="http://rdf.muninn-project.org/ontologies/ott"/>
<rdf:type rdf:resource="http://dbpedia.org/resource/Irony"/>
<vs:term_status>Stable</vs:term_status>
</skos:Concept>
<skos:Concept rdf:ID="GeneralOfficerCommanding">
<rdfs:label xml:lang="en">General Officer Commanding</rdfs:label>
<muninn:acronym xml:lang="en">G.O.C.</muninn:acronym>
<foaf:name>General Officer Commanding</foaf:name>
<skos:prefLabel xml:lang="en">General Officer Commanding</skos:prefLabel>
<skos:definition xml:lang="en">Tommy never sees him in the act of &quot;commanding,&quot; but has the opportunity of reading many an order signed &quot;G.O.C.&quot;</skos:definition>
<skos:inScheme rdf:resource="#OverTheTopDictionary"/>
<rdfs:isDefinedBy rdf:resource="http://rdf.muninn-project.org/ontologies/ott"/>
<rdf:type rdf:resource="http://dbpedia.org/resource/Irony"/>
<vs:term_status>Stable</vs:term_status>
</skos:Concept>
<skos:Concept rdf:ID="Goggles">
<rdfs:label xml:lang="en">Goggles</rdfs:label>
<foaf:name>Goggles</foaf:name>
<skos:prefLabel xml:lang="en">Goggles</skos:prefLabel>
<skos:definition xml:lang="en">An apparatus made of canvas and mica which is worn over the eyes for protection from the gases of German &quot;tear shells.&quot; The only time Tommy cries is when he forgets his goggles or misses the mm issue.</skos:definition>
<skos:inScheme rdf:resource="#OverTheTopDictionary"/>
<rdfs:isDefinedBy rdf:resource="http://rdf.muninn-project.org/ontologies/ott"/>
<rdf:type rdf:resource="http://dbpedia.org/resource/Irony"/>
<vs:term_status>Stable</vs:term_status>
</skos:Concept>
<skos:Concept rdf:ID="Goingin">
<rdfs:label xml:lang="en">Going in</rdfs:label>
<foaf:name>Going in</foaf:name>
<skos:prefLabel xml:lang="en">Going in</skos:prefLabel>
<skos:definition xml:lang="en">Taking over trenches.</skos:definition>
<skos:inScheme rdf:resource="#OverTheTopDictionary"/>
<rdfs:isDefinedBy rdf:resource="http://rdf.muninn-project.org/ontologies/ott"/>
<rdf:type rdf:resource="http://dbpedia.org/resource/Irony"/>
<rdf:type rdf:resource="http://dbpedia.org/resource/Slang"/>
<vs:term_status>Stable</vs:term_status>
</skos:Concept>
<skos:Concept rdf:ID="Goingout">
<rdfs:label xml:lang="en">Going out</rdfs:label>
<foaf:name>Going out</foaf:name>
<skos:prefLabel xml:lang="en">Going out</skos:prefLabel>
<skos:definition xml:lang="en">Relieved from the trenches.</skos:definition>
<skos:inScheme rdf:resource="#OverTheTopDictionary"/>
<rdfs:isDefinedBy rdf:resource="http://rdf.muninn-project.org/ontologies/ott"/>
<rdf:type rdf:resource="http://dbpedia.org/resource/Irony"/>
<vs:term_status>Stable</vs:term_status>
<rdf:type rdf:resource="http://dbpedia.org/resource/Slang"/>
</skos:Concept>
<skos:Concept rdf:ID="GoneWest">
<rdfs:label xml:lang="en">Gone West</rdfs:label>
<foaf:name>Gone West</foaf:name>
<skos:prefLabel xml:lang="en">Gone West</skos:prefLabel>
<skos:definition xml:lang="en">Killed; died.</skos:definition>
<skos:inScheme rdf:resource="#OverTheTopDictionary"/>
<rdfs:isDefinedBy rdf:resource="http://rdf.muninn-project.org/ontologies/ott"/>
<rdf:type rdf:resource="http://dbpedia.org/resource/Irony"/>
<vs:term_status>Stable</vs:term_status>
<rdf:type rdf:resource="http://dbpedia.org/resource/Slang"/>
</skos:Concept>
<skos:Concept rdf:ID="Gooseberries">
<rdfs:label xml:lang="en">Gooseberries</rdfs:label>
<foaf:name>Gooseberries</foaf:name>
<skos:prefLabel xml:lang="en">Gooseberries</skos:prefLabel>
<skos:definition xml:lang="en">A wooden frame in the shape of a cask wrapped round with barbed wire. These gooseberries are thrown into the barbed-wire entanglements to help make them impassable.</skos:definition>
<skos:inScheme rdf:resource="#OverTheTopDictionary"/>
<rdfs:isDefinedBy rdf:resource="http://rdf.muninn-project.org/ontologies/ott"/>
<rdf:type rdf:resource="http://dbpedia.org/resource/Irony"/>
<vs:term_status>Stable</vs:term_status>
<rdf:type rdf:resource="http://dbpedia.org/resource/Slang"/>
</skos:Concept>
<skos:Concept rdf:ID="GottheCrown">
<rdfs:label xml:lang="en">Got the Crown</rdfs:label>
<foaf:name>Got the Crown</foaf:name>
<skos:prefLabel xml:lang="en">Got the Crown</skos:prefLabel>
<skos:definition xml:lang="en">Promoted to Sergeant-Major.</skos:definition>
<skos:inScheme rdf:resource="#OverTheTopDictionary"/>
<rdfs:isDefinedBy rdf:resource="http://rdf.muninn-project.org/ontologies/ott"/>
<rdf:type rdf:resource="http://dbpedia.org/resource/Irony"/>
<vs:term_status>Stable</vs:term_status>
<rdf:type rdf:resource="http://dbpedia.org/resource/Slang"/>
</skos:Concept>
<skos:Concept rdf:ID="GreenEnvelope">
<rdfs:label xml:lang="en">Green Envelope</rdfs:label>
<foaf:name>Green Envelope</foaf:name>
<skos:prefLabel xml:lang="en">Green Envelope</skos:prefLabel>
<skos:definition xml:lang="en">An envelope of a green color issued to Tommy once a week. The contents will not be censored regimentally, but are liable to censor at the base. On the outside of envelope appears the following certificate, which Tommy must sign: &quot;I certify on my honor that the contents of this envelope refer to nothing but private and family matters.&quot; After signing this certificate Tommy immediately writes about everything but family and private matters.</skos:definition>
<skos:inScheme rdf:resource="#OverTheTopDictionary"/>
<rdfs:isDefinedBy rdf:resource="http://rdf.muninn-project.org/ontologies/ott"/>
<rdf:type rdf:resource="http://dbpedia.org/resource/Irony"/>
<vs:term_status>Stable</vs:term_status>
</skos:Concept>
<skos:Concept rdf:ID="Groom">
<rdfs:label xml:lang="en">Groom</rdfs:label>
<foaf:name>Groom</foaf:name>
<skos:prefLabel xml:lang="en">Groom</skos:prefLabel>
<skos:definition xml:lang="en">A soldier who looks after an officer&apos;s horse and who robs said horse of its hay. He makes his own bed comfortable with this hay.</skos:definition>
<skos:inScheme rdf:resource="#OverTheTopDictionary"/>
<rdfs:isDefinedBy rdf:resource="http://rdf.muninn-project.org/ontologies/ott"/>
<rdf:type rdf:resource="http://dbpedia.org/resource/Irony"/>
<vs:term_status>Stable</vs:term_status>
</skos:Concept>
<skos:Concept rdf:ID="Grousing">
<rdfs:label xml:lang="en">Grousing</rdfs:label>
<foaf:name>Grousing</foaf:name>
<skos:prefLabel xml:lang="en">Grousing</skos:prefLabel>
<skos:definition xml:lang="en">A scientific grumbling in which Tommy cusses everything in general and offends no one.</skos:definition>
<skos:inScheme rdf:resource="#OverTheTopDictionary"/>
<rdfs:isDefinedBy rdf:resource="http://rdf.muninn-project.org/ontologies/ott"/>
<rdf:type rdf:resource="http://dbpedia.org/resource/Irony"/>
<vs:term_status>Stable</vs:term_status>
</skos:Concept>
<skos:Concept rdf:ID="Gunshotwound">
<rdfs:label xml:lang="en">Gunshot wound</rdfs:label>
<muninn:acronym xml:lang="en">G.S.W.</muninn:acronym>
<foaf:name>Gunshot wound</foaf:name>
<skos:prefLabel xml:lang="en">Gunshot wound</skos:prefLabel>
<skos:definition xml:lang="en">When Tommy is wounded he does not care whether it is a G.S.W. or a kick from a mule, just so he gets back to Blighty.</skos:definition>
<skos:inScheme rdf:resource="#OverTheTopDictionary"/>
<rdfs:isDefinedBy rdf:resource="http://rdf.muninn-project.org/ontologies/ott"/>
<rdf:type rdf:resource="http://dbpedia.org/resource/Irony"/>
<vs:term_status>Stable</vs:term_status>
</skos:Concept>
<skos:Concept rdf:ID="GSWagon">
<rdfs:label xml:lang="en">G.S. Wagon</rdfs:label>
<foaf:name>G.S. Wagon</foaf:name>
<skos:prefLabel xml:lang="en">G.S. Wagon</skos:prefLabel>
<skos:definition xml:lang="en">A four-wheeled wagon driven by an A.S.C. driver. It carries supplies, such as food, ammunition, trench tools, and timber tor dugouts. When Tommy gets sore feet he is allowed to ride on this wagon and fills the ears of the driver with tales of his wonderful exploits. Occasionally one of these drivers believes him.</skos:definition>
<skos:inScheme rdf:resource="#OverTheTopDictionary"/>
<rdfs:isDefinedBy rdf:resource="http://rdf.muninn-project.org/ontologies/ott"/>
<rdf:type rdf:resource="http://dbpedia.org/resource/Irony"/>
<vs:term_status>Stable</vs:term_status>
<rdf:type rdf:resource="http://dbpedia.org/resource/Slang"/>
</skos:Concept>
<skos:Concept rdf:ID="GumBoots">
<rdfs:label xml:lang="en">Gum Boots</rdfs:label>
<foaf:name>Gum Boots</foaf:name>
<skos:prefLabel xml:lang="en">Gum Boots</skos:prefLabel>
<skos:definition xml:lang="en">Rubber boots issued to Tommy for wet trenches. They are used to keep his feet dry; they do, when he is lucky enough to get a pair.</skos:definition>
<skos:inScheme rdf:resource="#OverTheTopDictionary"/>
<rdfs:isDefinedBy rdf:resource="http://rdf.muninn-project.org/ontologies/ott"/>
<rdf:type rdf:resource="http://dbpedia.org/resource/Irony"/>
<vs:term_status>Stable</vs:term_status>
<rdf:type rdf:resource="http://dbpedia.org/resource/Slang"/>
</skos:Concept>
<skos:Concept rdf:ID="Gummingthegame">
<rdfs:label xml:lang="en">Gumming the game</rdfs:label>
<foaf:name>Gumming the game</foaf:name>
<skos:prefLabel xml:lang="en">Gumming the game</skos:prefLabel>
<skos:definition xml:lang="en">Spoiling anything, interfering.</skos:definition>
<skos:inScheme rdf:resource="#OverTheTopDictionary"/>
<rdfs:isDefinedBy rdf:resource="http://rdf.muninn-project.org/ontologies/ott"/>
<rdf:type rdf:resource="http://dbpedia.org/resource/Irony"/>
<vs:term_status>Stable</vs:term_status>
<rdf:type rdf:resource="http://dbpedia.org/resource/Slang"/>
</skos:Concept>
<skos:Concept rdf:ID="Hairbrush">
<rdfs:label xml:lang="en">Hair brush</rdfs:label>
<foaf:name>Hair brush</foaf:name>
<skos:prefLabel xml:lang="en">Hair brush</skos:prefLabel>
<skos:definition xml:lang="en">Name of a bomb used in the earlier stages of the war. It is shaped like a hair brush and is thrown by the handle. Tommy used to throw them over to the Germans for their morning toilette.</skos:definition>
<skos:inScheme rdf:resource="#OverTheTopDictionary"/>
<rdfs:isDefinedBy rdf:resource="http://rdf.muninn-project.org/ontologies/ott"/>
<rdf:type rdf:resource="http://dbpedia.org/resource/Irony"/>
<vs:term_status>Stable</vs:term_status>
<rdf:type rdf:resource="http://dbpedia.org/resource/Slang"/>
</skos:Concept>
<skos:Concept rdf:ID="Handgrenade">
<rdfs:label xml:lang="en">Hand grenade</rdfs:label>
<foaf:name>Hand grenade</foaf:name>
<skos:prefLabel xml:lang="en">Hand grenade</skos:prefLabel>
<skos:definition xml:lang="en">A general term for a bomb which is thrown by hand. Tommy looks upon all bombs with grave suspicion; from long experience he has learned not to trust them, even if the detonator has been removed.</skos:definition>
<skos:inScheme rdf:resource="#OverTheTopDictionary"/>
<rdfs:isDefinedBy rdf:resource="http://rdf.muninn-project.org/ontologies/ott"/>
<rdf:type rdf:resource="http://dbpedia.org/resource/Irony"/>
<vs:term_status>Stable</vs:term_status>
</skos:Concept>
<skos:Concept rdf:ID="Hardtails">
<rdfs:label xml:lang="en">Hard tails</rdfs:label>
<foaf:name>Hard tails</foaf:name>
<skos:prefLabel xml:lang="en">Hard tails</skos:prefLabel>
<skos:definition xml:lang="en">Mules.</skos:definition>
<skos:inScheme rdf:resource="#OverTheTopDictionary"/>
<rdfs:isDefinedBy rdf:resource="http://rdf.muninn-project.org/ontologies/ott"/>
<rdf:type rdf:resource="http://dbpedia.org/resource/Irony"/>
<vs:term_status>Stable</vs:term_status>
<rdf:type rdf:resource="http://dbpedia.org/resource/Slang"/>
</skos:Concept>
<skos:Concept rdf:ID="Haversack">
<rdfs:label xml:lang="en">Haversack</rdfs:label>
<foaf:name>Haversack</foaf:name>
<skos:prefLabel xml:lang="en">Haversack</skos:prefLabel>
<skos:definition xml:lang="en">A canvas bag forming part of Tommy&apos;s equipment, carried on the left side. Its original use was intended for the carrying of emergency rations and small kit. It is generally filled with a miscellaneous assortment of tobacco, pipes, bread crumbs, letters, and a lot of useless souvenirs.</skos:definition>
<skos:inScheme rdf:resource="#OverTheTopDictionary"/>
<rdfs:isDefinedBy rdf:resource="http://rdf.muninn-project.org/ontologies/ott"/>
<rdf:type rdf:resource="http://dbpedia.org/resource/Irony"/>
<vs:term_status>Stable</vs:term_status>
</skos:Concept>
<skos:Concept rdf:ID="Havingadoss">
<rdfs:label xml:lang="en">Having a doss</rdfs:label>
<foaf:name>Having a doss</foaf:name>
<skos:prefLabel xml:lang="en">Having a doss</skos:prefLabel>
<skos:definition xml:lang="en">Having a sleep.</skos:definition>
<skos:inScheme rdf:resource="#OverTheTopDictionary"/>
<rdfs:isDefinedBy rdf:resource="http://rdf.muninn-project.org/ontologies/ott"/>
<rdf:type rdf:resource="http://dbpedia.org/resource/Irony"/>
<vs:term_status>Stable</vs:term_status>
<rdf:type rdf:resource="http://dbpedia.org/resource/Slang"/>
</skos:Concept>
<skos:Concept rdf:ID="HoldAll">
<rdfs:label xml:lang="en">Hold-all</rdfs:label>
<foaf:name>Hold-all</foaf:name>
<skos:prefLabel xml:lang="en">Hold-all</skos:prefLabel>
<skos:definition xml:lang="en">A small canvas roll in which you are supposed to carry your razor, comb, knife, fork, spoon, mirror, soap, tooth brush, etc. Tommy takes great care of the above, because it means extra pack drill to come on parade unshaven.</skos:definition>
<skos:inScheme rdf:resource="#OverTheTopDictionary"/>
<rdfs:isDefinedBy rdf:resource="http://rdf.muninn-project.org/ontologies/ott"/>
<rdf:type rdf:resource="http://dbpedia.org/resource/Irony"/>
<vs:term_status>Stable</vs:term_status>
<rdf:type rdf:resource="http://dbpedia.org/resource/Slang"/>
</skos:Concept>
<skos:Concept rdf:ID="HolyJoe">
<rdfs:label xml:lang="en">Holy Joe</rdfs:label>
<foaf:name>Holy Joe</foaf:name>
<skos:prefLabel xml:lang="en">Holy Joe</skos:prefLabel>
<skos:definition xml:lang="en">Tommy&apos;s familiar but not necessarily irreverent same for the Chaplain. He really has a great admiration for this officer, who although not a fighting man, so often risks his life to save a wounded Tommy.</skos:definition>
<rdf:type rdf:resource="http://dbpedia.org/resource/Nickname"/>
<skos:inScheme rdf:resource="#OverTheTopDictionary"/>
<rdfs:isDefinedBy rdf:resource="http://rdf.muninn-project.org/ontologies/ott"/>
<rdf:type rdf:resource="http://dbpedia.org/resource/Irony"/>
<vs:term_status>Stable</vs:term_status>
<rdf:type rdf:resource="http://dbpedia.org/resource/Slang"/>
</skos:Concept>
<skos:Concept rdf:ID="Housewife">
<rdfs:label xml:lang="en">Housewife</rdfs:label>
<foaf:name>Housewife</foaf:name>
<skos:prefLabel xml:lang="en">Housewife</skos:prefLabel>
<skos:definition xml:lang="en">A neat little package of needles, thread, extra shoelaces, and buttons. When a button comes off Tommy&apos;s trousers, instead of going to his housewife he looks around for a nail.</skos:definition>
<skos:inScheme rdf:resource="#OverTheTopDictionary"/>
<rdfs:isDefinedBy rdf:resource="http://rdf.muninn-project.org/ontologies/ott"/>
<rdf:type rdf:resource="http://dbpedia.org/resource/Irony"/>
<vs:term_status>Stable</vs:term_status>
</skos:Concept>
<skos:Concept rdf:ID="Hun">
<rdfs:label xml:lang="en">Hun</rdfs:label>
<foaf:name>Hun</foaf:name>
<skos:prefLabel xml:lang="en">Hun</skos:prefLabel>
<skos:definition xml:lang="en">Another term for a German, mostly used by war correspondents.</skos:definition>
<skos:inScheme rdf:resource="#OverTheTopDictionary"/>
<rdfs:isDefinedBy rdf:resource="http://rdf.muninn-project.org/ontologies/ott"/>
<rdf:type rdf:resource="http://dbpedia.org/resource/Irony"/>
<vs:term_status>Stable</vs:term_status>
<rdf:type rdf:resource="http://dbpedia.org/resource/Slang"/>
</skos:Concept>
<skos:Concept rdf:ID="Hunpinching">
<rdfs:label xml:lang="en">Hun pinching</rdfs:label>
<foaf:name>Hun pinching</foaf:name>
<skos:prefLabel xml:lang="en">Hun pinching</skos:prefLabel>
<skos:definition xml:lang="en">Raiding German trenches for prisoners.</skos:definition>
<skos:inScheme rdf:resource="#OverTheTopDictionary"/>
<rdfs:isDefinedBy rdf:resource="http://rdf.muninn-project.org/ontologies/ott"/>
<rdf:type rdf:resource="http://dbpedia.org/resource/Irony"/>
<vs:term_status>Stable</vs:term_status>
<rdf:type rdf:resource="http://dbpedia.org/resource/Slang"/>
</skos:Concept>
<skos:Concept rdf:ID="IdentificationDisk">
<rdfs:label xml:lang="en">Identification Disk</rdfs:label>
<foaf:name>Identification Disk</foaf:name>
<skos:prefLabel xml:lang="en">Identification Disk</skos:prefLabel>
<skos:definition xml:lang="en">A little fiber disk which is worn around the neck by means of a string. On one side is stamped your name, rank, regimental number, and regiment, while on the other side is stamped your religion. If at any time Tommy is doubtful of his identity he looks at his disk to reassure himself.</skos:definition>
<skos:inScheme rdf:resource="#OverTheTopDictionary"/>
<rdfs:isDefinedBy rdf:resource="http://rdf.muninn-project.org/ontologies/ott"/>
<rdf:type rdf:resource="http://dbpedia.org/resource/Irony"/>
<vs:term_status>Stable</vs:term_status>
</skos:Concept>
<skos:Concept rdf:ID="Imsorry">
<rdfs:label xml:lang="en">I&apos;m sorry</rdfs:label>
<foaf:name>I&apos;m sorry</foaf:name>
<skos:prefLabel xml:lang="en">I&apos;m sorry</skos:prefLabel>
<skos:definition xml:lang="en">Tommy&apos;s apology. If he pokes your eye out with his bayonet he says, &quot;I&apos;m sorry,&quot; and the matter is ended so far as he is concerned.</skos:definition>
<skos:inScheme rdf:resource="#OverTheTopDictionary"/>
<rdfs:isDefinedBy rdf:resource="http://rdf.muninn-project.org/ontologies/ott"/>
<rdf:type rdf:resource="http://dbpedia.org/resource/Irony"/>
<vs:term_status>Stable</vs:term_status>
</skos:Concept>
<skos:Concept rdf:ID="Infront">
<rdfs:label xml:lang="en">In front</rdfs:label>
<foaf:name>In front</foaf:name>
<skos:prefLabel xml:lang="en">In front</skos:prefLabel>
<skos:definition xml:lang="en">Over the top; in front of the front-line trench, in No Man&apos;s Land.</skos:definition>
<skos:inScheme rdf:resource="#OverTheTopDictionary"/>
<rdfs:isDefinedBy rdf:resource="http://rdf.muninn-project.org/ontologies/ott"/>
<rdf:type rdf:resource="http://dbpedia.org/resource/Irony"/>
<vs:term_status>Stable</vs:term_status>
</skos:Concept>
<skos:Concept rdf:ID="Inreserve">
<rdfs:label xml:lang="en">In reserve</rdfs:label>
<foaf:name>In reserve</foaf:name>
<skos:prefLabel xml:lang="en">In reserve</skos:prefLabel>
<skos:definition xml:lang="en">Troops occupying positions, billets, or dugouts, immediately in rear of the front line, who in case of an attack will support the firing line.</skos:definition>
<skos:inScheme rdf:resource="#OverTheTopDictionary"/>
<rdfs:isDefinedBy rdf:resource="http://rdf.muninn-project.org/ontologies/ott"/>
<rdf:type rdf:resource="http://dbpedia.org/resource/Irony"/>
<vs:term_status>Stable</vs:term_status>
</skos:Concept>
<skos:Concept rdf:ID="IntelligenceDepartment">
<rdfs:label xml:lang="en">Intelligence Department</rdfs:label>
<foaf:name>Intelligence Department</foaf:name>
<skos:prefLabel xml:lang="en">Intelligence Department</skos:prefLabel>
<skos:definition xml:lang="en">Secret service men who are supposed to catch spies or be spies as the occasion demands.</skos:definition>
<skos:inScheme rdf:resource="#OverTheTopDictionary"/>
<rdfs:isDefinedBy rdf:resource="http://rdf.muninn-project.org/ontologies/ott"/>
<rdf:type rdf:resource="http://dbpedia.org/resource/Irony"/>
<vs:term_status>Stable</vs:term_status>
</skos:Concept>
<skos:Concept rdf:ID="Interpreter">
<rdfs:label xml:lang="en">Interpreter</rdfs:label>
<foaf:name>Interpreter</foaf:name>
<skos:prefLabel xml:lang="en">Interpreter</skos:prefLabel>
<skos:definition xml:lang="en">A fat job with a &quot;return ticket,&quot; held by a soldier who thinks he can speak a couple of languages. He questions prisoners as to the color of their grandmothers&apos; eyes and why they joined the army. Just imagine asking a German &quot;why&quot; he joined the army.</skos:definition>
<skos:inScheme rdf:resource="#OverTheTopDictionary"/>
<rdfs:isDefinedBy rdf:resource="http://rdf.muninn-project.org/ontologies/ott"/>
<rdf:type rdf:resource="http://dbpedia.org/resource/Irony"/>
<vs:term_status>Stable</vs:term_status>
</skos:Concept>
<skos:Concept rdf:ID="Invalided">
<rdfs:label xml:lang="en">Invalided</rdfs:label>
<foaf:name>Invalided</foaf:name>
<skos:prefLabel xml:lang="en">Invalided</skos:prefLabel>
<skos:definition xml:lang="en">Sent to England on account of sickness.</skos:definition>
<skos:inScheme rdf:resource="#OverTheTopDictionary"/>
<rdfs:isDefinedBy rdf:resource="http://rdf.muninn-project.org/ontologies/ott"/>
<rdf:type rdf:resource="http://dbpedia.org/resource/Irony"/>
<vs:term_status>Stable</vs:term_status>
</skos:Concept>
<skos:Concept rdf:ID="IronRations">
<rdfs:label xml:lang="en">Iron Rations</rdfs:label>
<foaf:name>Iron Rations</foaf:name>
<skos:prefLabel xml:lang="en">Iron Rations</skos:prefLabel>
<skos:definition xml:lang="en">A tin of bully beef, two biscuits, and a tin containing tea, sugar, and Oxo cubes. These are not supposed to be eaten until you die of starvation.</skos:definition>
<skos:inScheme rdf:resource="#OverTheTopDictionary"/>
<rdfs:isDefinedBy rdf:resource="http://rdf.muninn-project.org/ontologies/ott"/>
<rdf:type rdf:resource="http://dbpedia.org/resource/Irony"/>
<vs:term_status>Stable</vs:term_status>
<rdf:type rdf:resource="http://dbpedia.org/resource/Slang"/>
</skos:Concept>
<skos:Concept rdf:ID="IsolatedPost">
<rdfs:label xml:lang="en">Isolated Post</rdfs:label>
<foaf:name>Isolated Post</foaf:name>
<skos:prefLabel xml:lang="en">Isolated Post</skos:prefLabel>
<skos:definition xml:lang="en">An advanced part of a trench or position where one or two sentries are posted to guard against a surprise attack. While in this post Tommy is constantly wondering what the Germans will do with his body.</skos:definition>
<skos:inScheme rdf:resource="#OverTheTopDictionary"/>
<rdfs:isDefinedBy rdf:resource="http://rdf.muninn-project.org/ontologies/ott"/>
<rdf:type rdf:resource="http://dbpedia.org/resource/Irony"/>
<vs:term_status>Stable</vs:term_status>
</skos:Concept>
<skos:Concept rdf:ID="ItsgoodwehaveaNavy">
<rdfs:label xml:lang="en">It&apos;s good we have a Navy</rdfs:label>
<foaf:name>It&apos;s good we have a Navy</foaf:name>
<skos:prefLabel xml:lang="en">It&apos;s good we have a Navy</skos:prefLabel>
<skos:definition xml:lang="en">One of Tommy&apos;s expressions when he is disgusted with the army and its work.</skos:definition>
<skos:inScheme rdf:resource="#OverTheTopDictionary"/>
<rdfs:isDefinedBy rdf:resource="http://rdf.muninn-project.org/ontologies/ott"/>
<rdf:type rdf:resource="http://dbpedia.org/resource/Irony"/>
<rdf:type rdf:resource="http://dbpedia.org/resource/Slang"/>
<vs:term_status>Stable</vs:term_status>
</skos:Concept>
<skos:Concept rdf:ID="JackJohnson">
<rdfs:label xml:lang="en">Jack Johnson</rdfs:label>
<foaf:name>Jack Johnson</foaf:name>
<skos:prefLabel xml:lang="en">Jack Johnson</skos:prefLabel>
<skos:definition xml:lang="en">A seventeen-inch German shell. Probably called &quot;Jack Johnson&quot; because the Germans thought that with it they could lick the world.</skos:definition>
<skos:inScheme rdf:resource="#OverTheTopDictionary"/>
<rdfs:isDefinedBy rdf:resource="http://rdf.muninn-project.org/ontologies/ott"/>
<rdf:type rdf:resource="http://dbpedia.org/resource/Irony"/>
<rdf:type rdf:resource="http://dbpedia.org/resource/Slang"/>
<vs:term_status>Stable</vs:term_status>
</skos:Concept>
<skos:Concept rdf:ID="Jackknife">
<rdfs:label xml:lang="en">Jackknife</rdfs:label>
<foaf:name>Jackknife</foaf:name>
<skos:prefLabel xml:lang="en">Jackknife</skos:prefLabel>
<skos:definition xml:lang="en">A knife, issued to Tommy, which weighs a stone and won&apos;t cut. Its only virtue is the fact that it has a tin-opener attachment which won&apos;t open tins.</skos:definition>
<skos:inScheme rdf:resource="#OverTheTopDictionary"/>
<rdfs:isDefinedBy rdf:resource="http://rdf.muninn-project.org/ontologies/ott"/>
<rdf:type rdf:resource="http://dbpedia.org/resource/Irony"/>
<vs:term_status>Stable</vs:term_status>
</skos:Concept>
<skos:Concept rdf:ID="Jam">
<rdfs:label xml:lang="en">Jam</rdfs:label>
<foaf:name>Jam</foaf:name>
<skos:prefLabel xml:lang="en">Jam</skos:prefLabel>
<skos:definition xml:lang="en">A horrible mess of fruit and sugar which Tommy spreads on his bread. It all tastes the same no matter whether labelled &quot;Strawberry &quot; or &quot;Green Gage.&quot;</skos:definition>
<skos:inScheme rdf:resource="#OverTheTopDictionary"/>
<rdfs:isDefinedBy rdf:resource="http://rdf.muninn-project.org/ontologies/ott"/>
<rdf:type rdf:resource="http://dbpedia.org/resource/Irony"/>
<vs:term_status>Stable</vs:term_status>
</skos:Concept>
<skos:Concept rdf:ID="JamTin">
<rdfs:label xml:lang="en">Jam Tin</rdfs:label>
<foaf:name>Jam Tin</foaf:name>
<skos:prefLabel xml:lang="en">Jam Tin</skos:prefLabel>
<skos:definition xml:lang="en">A crude sort of hand grenade which, in the early stages of the war. Tommy used to manufacture out of jam tins, ammonal, and mud. The manufacturer generally would receive a little wooden cross in recognition of the fact that he died for King and Country.</skos:definition>
<skos:inScheme rdf:resource="#OverTheTopDictionary"/>
<rdfs:isDefinedBy rdf:resource="http://rdf.muninn-project.org/ontologies/ott"/>
<rdf:type rdf:resource="http://dbpedia.org/resource/Irony"/>
<vs:term_status>Stable</vs:term_status>
</skos:Concept>
<skos:Concept rdf:ID="Jock">
<rdfs:label xml:lang="en">Jock</rdfs:label>
<foaf:name>Jock</foaf:name>
<skos:prefLabel xml:lang="en">Jock</skos:prefLabel>
<skos:definition xml:lang="en">Universal name for a Scotchman.</skos:definition>
<skos:inScheme rdf:resource="#OverTheTopDictionary"/>
<rdfs:isDefinedBy rdf:resource="http://rdf.muninn-project.org/ontologies/ott"/>
<rdf:type rdf:resource="http://dbpedia.org/resource/Irony"/>
<rdf:type rdf:resource="http://dbpedia.org/resource/Slang"/>
<vs:term_status>Stable</vs:term_status>
</skos:Concept>
<skos:Concept rdf:ID="Kickedthebucket">
<rdfs:label xml:lang="en">Kicked the bucket</rdfs:label>
<foaf:name>Kicked the bucket</foaf:name>
<skos:prefLabel xml:lang="en">Kicked the bucket</skos:prefLabel>
<skos:definition xml:lang="en">Died.</skos:definition>
<skos:inScheme rdf:resource="#OverTheTopDictionary"/>
<rdfs:isDefinedBy rdf:resource="http://rdf.muninn-project.org/ontologies/ott"/>
<rdf:type rdf:resource="http://dbpedia.org/resource/Irony"/>
<rdf:type rdf:resource="http://dbpedia.org/resource/Slang"/>
<vs:term_status>Stable</vs:term_status>
</skos:Concept>
<skos:Concept rdf:ID="Kilo">
<rdfs:label xml:lang="en">Kilo</rdfs:label>
<foaf:name>Kilo</foaf:name>
<skos:prefLabel xml:lang="en">Kilo</skos:prefLabel>
<skos:definition xml:lang="en">Five eighths of a mile. Ten &quot;kilos&quot; generally means a trek of fifteen miles.</skos:definition>
<skos:inScheme rdf:resource="#OverTheTopDictionary"/>
<rdfs:isDefinedBy rdf:resource="http://rdf.muninn-project.org/ontologies/ott"/>
<rdf:type rdf:resource="http://dbpedia.org/resource/Irony"/>
<vs:term_status>Stable</vs:term_status>
</skos:Concept>
<skos:Concept rdf:ID="KingShilling">
<rdfs:label xml:lang="en">King&apos;s Shilling</rdfs:label>
<foaf:name>King&apos;s Shilling</foaf:name>
<skos:prefLabel xml:lang="en">King&apos;s Shilling</skos:prefLabel>
<skos:definition xml:lang="en">Tommy&apos;s rate of pay per day, perhaps.</skos:definition>
<skos:inScheme rdf:resource="#OverTheTopDictionary"/>
<rdfs:isDefinedBy rdf:resource="http://rdf.muninn-project.org/ontologies/ott"/>
<rdf:type rdf:resource="http://dbpedia.org/resource/Irony"/>
<vs:term_status>Stable</vs:term_status>
<rdf:type rdf:resource="http://dbpedia.org/resource/Slang"/>
</skos:Concept>
<skos:Concept rdf:ID="TakingtheKingShilling">
<rdfs:label xml:lang="en">Taking the King&apos;s Shilling</rdfs:label>
<foaf:name>Taking the King&apos;s Shilling</foaf:name>
<skos:prefLabel xml:lang="en">Taking the King&apos;s Shilling</skos:prefLabel>
<skos:definition xml:lang="en">Means enlisting.</skos:definition>
<skos:inScheme rdf:resource="#OverTheTopDictionary"/>
<rdfs:isDefinedBy rdf:resource="http://rdf.muninn-project.org/ontologies/ott"/>
<rdf:type rdf:resource="http://dbpedia.org/resource/Irony"/>
<vs:term_status>Stable</vs:term_status>
<rdf:type rdf:resource="http://dbpedia.org/resource/Slang"/>
</skos:Concept>
<skos:Concept rdf:ID="Kip">
<rdfs:label xml:lang="en">Kip</rdfs:label>
<foaf:name>Kip</foaf:name>
<skos:prefLabel xml:lang="en">Kip</skos:prefLabel>
<skos:definition xml:lang="en">Tommy&apos;s term for &quot;sleep.&quot; He also calls his bed his &quot;kip.&quot; It is on guard that Tommy most desires to kip.</skos:definition>
<skos:inScheme rdf:resource="#OverTheTopDictionary"/>
<rdfs:isDefinedBy rdf:resource="http://rdf.muninn-project.org/ontologies/ott"/>
<rdf:type rdf:resource="http://dbpedia.org/resource/Irony"/>
<vs:term_status>Stable</vs:term_status>
<rdf:type rdf:resource="http://dbpedia.org/resource/Slang"/>
</skos:Concept>
<skos:Concept rdf:ID="KitBag">
<rdfs:label xml:lang="en">Kit Bag</rdfs:label>
<foaf:name>Kit Bag</foaf:name>
<skos:prefLabel xml:lang="en">Kit Bag</skos:prefLabel>
<skos:definition xml:lang="en">A part of Tommy&apos;s equipment in which he is supposed to pack up his troubles and smile, according to the words of a popular song (the composer was never in a trench).</skos:definition>
<skos:inScheme rdf:resource="#OverTheTopDictionary"/>
<rdfs:isDefinedBy rdf:resource="http://rdf.muninn-project.org/ontologies/ott"/>
<rdf:type rdf:resource="http://dbpedia.org/resource/Irony"/>
<vs:term_status>Stable</vs:term_status>
</skos:Concept>
<skos:Concept rdf:ID="KitchenerArmy">
<rdfs:label xml:lang="en">Kitchener&apos;s Army</rdfs:label>
<foaf:name>Kitchener&apos;s Army</foaf:name>
<skos:prefLabel xml:lang="en">Kitchener&apos;s Army</skos:prefLabel>
<skos:definition xml:lang="en">The volunteer army raised by Lord Kitchener, the members of which signed for duration of war. They are commonly called the &quot;New Army&quot; or &quot;Kitchener&apos;s Mob.&quot; At first the Regulars and Territorials looked down on them, but now accept them as welcome mates.</skos:definition>
<skos:inScheme rdf:resource="#OverTheTopDictionary"/>
<rdfs:isDefinedBy rdf:resource="http://rdf.muninn-project.org/ontologies/ott"/>
<rdf:type rdf:resource="http://dbpedia.org/resource/Irony"/>
<vs:term_status>Stable</vs:term_status>
<rdf:type rdf:resource="http://dbpedia.org/resource/Slang"/>
</skos:Concept>
<skos:Concept rdf:ID="LaborBattalion">
<rdfs:label xml:lang="en">Labor Battalion</rdfs:label>
<foaf:name>Labor Battalion</foaf:name>
<skos:prefLabel xml:lang="en">Labor Battalion</skos:prefLabel>
<skos:definition xml:lang="en">An organization which is &quot;too proud to fight.&quot; They would sooner use a pick and shovel.</skos:definition>
<skos:inScheme rdf:resource="#OverTheTopDictionary"/>
<rdfs:isDefinedBy rdf:resource="http://rdf.muninn-project.org/ontologies/ott"/>
<rdf:type rdf:resource="http://dbpedia.org/resource/Irony"/>
<vs:term_status>Stable</vs:term_status>
</skos:Concept>
<skos:Concept rdf:ID="LanceCorporal">
<rdfs:label xml:lang="en">Lance-corporal</rdfs:label>
<foaf:name>Lance-corporal</foaf:name>
<skos:prefLabel xml:lang="en">Lance-corporal</skos:prefLabel>
<skos:definition xml:lang="en">A N.C.O. one grade above a private who wears a shoestring stripe on his arm and thinks the war should be run according to his ideas.</skos:definition>
<skos:inScheme rdf:resource="#OverTheTopDictionary"/>
<rdfs:isDefinedBy rdf:resource="http://rdf.muninn-project.org/ontologies/ott"/>
<rdf:type rdf:resource="http://dbpedia.org/resource/Irony"/>
<vs:term_status>Stable</vs:term_status>
</skos:Concept>
<skos:Concept rdf:ID="lead">
<rdfs:label xml:lang="en">lead</rdfs:label>
<foaf:name>lead</foaf:name>
<skos:prefLabel xml:lang="en">lead</skos:prefLabel>
<skos:definition xml:lang="en">The leading pair of horses or mules on a limber. Their only fault is that they won&apos;t lead (if they happen to be mules).</skos:definition>
<skos:inScheme rdf:resource="#OverTheTopDictionary"/>
<rdfs:isDefinedBy rdf:resource="http://rdf.muninn-project.org/ontologies/ott"/>
<rdf:type rdf:resource="http://dbpedia.org/resource/Irony"/>
<vs:term_status>Stable</vs:term_status>
</skos:Concept>
<skos:Concept rdf:ID="LeaveTrain">
<rdfs:label xml:lang="en">Leave Train</rdfs:label>
<foaf:name>Leave Train</foaf:name>
<skos:prefLabel xml:lang="en">Leave Train</skos:prefLabel>
<skos:definition xml:lang="en">The train which takes Tommy to one of the seaports on the Channel en route to Blighty when granted leave. The worst part of going on leave is coming back.</skos:definition>
<skos:inScheme rdf:resource="#OverTheTopDictionary"/>
<rdfs:isDefinedBy rdf:resource="http://rdf.muninn-project.org/ontologies/ott"/>
<rdf:type rdf:resource="http://dbpedia.org/resource/Irony"/>
<vs:term_status>Stable</vs:term_status>
</skos:Concept>
<skos:Concept rdf:ID="LeeEnfield">
<rdfs:label xml:lang="en">Lee Enfield</rdfs:label>
<foaf:name>Lee Enfield</foaf:name>
<skos:prefLabel xml:lang="en">Lee Enfield</skos:prefLabel>
<skos:definition xml:lang="en">Name of the rifle used by the British Army. Its caliber is .303 and the magazine holds ten rounds. When dirty it has a tasty habit of getting Tommy&apos;s name on the crime sheet.</skos:definition>
<skos:inScheme rdf:resource="#OverTheTopDictionary"/>
<rdfs:isDefinedBy rdf:resource="http://rdf.muninn-project.org/ontologies/ott"/>
<rdf:type rdf:resource="http://dbpedia.org/resource/Irony"/>
<vs:term_status>Stable</vs:term_status>
</skos:Concept>
<skos:Concept rdf:ID="Leggingit">
<rdfs:label xml:lang="en">Legging it</rdfs:label>
<foaf:name>Legging it</foaf:name>
<skos:prefLabel xml:lang="en">Legging it</skos:prefLabel>
<skos:definition xml:lang="en">Running away.</skos:definition>
<skos:inScheme rdf:resource="#OverTheTopDictionary"/>
<rdfs:isDefinedBy rdf:resource="http://rdf.muninn-project.org/ontologies/ott"/>
<rdf:type rdf:resource="http://dbpedia.org/resource/Irony"/>
<vs:term_status>Stable</vs:term_status>
<rdf:type rdf:resource="http://dbpedia.org/resource/Slang"/>
</skos:Concept>
<skos:Concept rdf:ID="LewisGun">
<rdfs:label xml:lang="en">Lewis Gun</rdfs:label>
<foaf:name>Lewis Gun</foaf:name>
<skos:prefLabel xml:lang="en">Lewis Gun</skos:prefLabel>
<skos:definition xml:lang="en">A rifle-like machine gun, air cooled, which only carries 47 rounds in its &quot;pie-plate&quot; magazine. Under fire when this magazine is emptied you shout for &quot;ammo&quot; but perhaps No. 2, the ammo carrier, is lying in the rear with a bullet through his napper. Then it&apos;s &quot;napoo-fini&quot; (Tommy&apos;s French) for Mr. Lewis.</skos:definition>
<skos:inScheme rdf:resource="#OverTheTopDictionary"/>
<rdfs:isDefinedBy rdf:resource="http://rdf.muninn-project.org/ontologies/ott"/>
<rdf:type rdf:resource="http://dbpedia.org/resource/Irony"/>
<vs:term_status>Stable</vs:term_status>
</skos:Concept>
<skos:Concept rdf:ID="LightDuty">
<rdfs:label xml:lang="en">Light Duty</rdfs:label>
<foaf:name>Light Duty</foaf:name>
<skos:prefLabel xml:lang="en">Light Duty</skos:prefLabel>
<skos:definition xml:lang="en">What the doctor marks on the sick report opposite a Tommy&apos;s name when he has doubts as to whether said Tommy is putting one over on him. Usually Tommy is.</skos:definition>
<skos:inScheme rdf:resource="#OverTheTopDictionary"/>
<rdfs:isDefinedBy rdf:resource="http://rdf.muninn-project.org/ontologies/ott"/>
<rdf:type rdf:resource="http://dbpedia.org/resource/Irony"/>
<vs:term_status>Stable</vs:term_status>
</skos:Concept>
<skos:Concept rdf:ID="LightRailway">
<rdfs:label xml:lang="en">Light Railway</rdfs:label>
<foaf:name>Light Railway</foaf:name>
<skos:prefLabel xml:lang="en">Light Railway</skos:prefLabel>
<skos:definition xml:lang="en">Two thin iron tracks on which small flat cars full of ammunition and supplies are pushed. These railways afford Tommy great sport in the loading, pushing, and unloading of cars.</skos:definition>
<skos:inScheme rdf:resource="#OverTheTopDictionary"/>
<rdfs:isDefinedBy rdf:resource="http://rdf.muninn-project.org/ontologies/ott"/>
<rdf:type rdf:resource="http://dbpedia.org/resource/Irony"/>
<vs:term_status>Stable</vs:term_status>
</skos:Concept>
<skos:Concept rdf:ID="Limber">
<rdfs:label xml:lang="en">Limber</rdfs:label>
<foaf:name>Limber</foaf:name>
<skos:prefLabel xml:lang="en">Limber</skos:prefLabel>
<skos:definition xml:lang="en">A match box on two wheels which gives the Army mule a job. It also carries officer&apos;s packs.</skos:definition>
<skos:inScheme rdf:resource="#OverTheTopDictionary"/>
<rdfs:isDefinedBy rdf:resource="http://rdf.muninn-project.org/ontologies/ott"/>
<rdf:type rdf:resource="http://dbpedia.org/resource/Irony"/>
<vs:term_status>Stable</vs:term_status>
</skos:Concept>
<skos:Concept rdf:ID="LiquidFire">
<rdfs:label xml:lang="en">Liquid Fire</rdfs:label>
<foaf:name>Liquid Fire</foaf:name>
<skos:prefLabel xml:lang="en">Liquid Fire</skos:prefLabel>
<skos:definition xml:lang="en">Another striking example of German &quot;Kultur.&quot; According to the Germans it is supposed to annihilate whole brigades, but Tommy refuses to be annihilated.</skos:definition>
<skos:inScheme rdf:resource="#OverTheTopDictionary"/>
<rdfs:isDefinedBy rdf:resource="http://rdf.muninn-project.org/ontologies/ott"/>
<rdf:type rdf:resource="http://dbpedia.org/resource/Irony"/>
<rdf:type rdf:resource="http://dbpedia.org/resource/Slang"/>
<vs:term_status>Stable</vs:term_status>
</skos:Concept>
<skos:Concept rdf:ID="ListeningPost">
<rdfs:label xml:lang="en">Listening Post</rdfs:label>
<foaf:name>Listening Post</foaf:name>
<skos:prefLabel xml:lang="en">Listening Post</skos:prefLabel>
<skos:definition xml:lang="en">Two or three men detailed to go out &quot;in front&quot; at night, to lie on the ground and listen for any undue activity in the German lines. They also listen for the digging of mines. It is nervous work and when Tommy returns he generally writes for a bos of &quot;Phosperine Tablets,&quot; a widely advertised nerve tonic.</skos:definition>
<skos:inScheme rdf:resource="#OverTheTopDictionary"/>
<rdfs:isDefinedBy rdf:resource="http://rdf.muninn-project.org/ontologies/ott"/>
<rdf:type rdf:resource="http://dbpedia.org/resource/Irony"/>
<vs:term_status>Stable</vs:term_status>
</skos:Concept>
<skos:Concept rdf:ID="LittleWillie">
<rdfs:label xml:lang="en">Little Willie</rdfs:label>
<foaf:name>Little Willie</foaf:name>
<skos:prefLabel xml:lang="en">Little Willie</skos:prefLabel>
<skos:definition xml:lang="en">Tommy&apos;s nickname for the German Crown. Prince. They are not on speaking terms.</skos:definition>
<skos:inScheme rdf:resource="#OverTheTopDictionary"/>
<rdfs:isDefinedBy rdf:resource="http://rdf.muninn-project.org/ontologies/ott"/>
<rdf:type rdf:resource="http://dbpedia.org/resource/Irony"/>
<rdf:type rdf:resource="http://dbpedia.org/resource/Nickname"/>
<vs:term_status>Stable</vs:term_status>
</skos:Concept>
<skos:Concept rdf:ID="LloydGeorgePets">
<rdfs:label xml:lang="en">Lloyd George&apos;s Pets</rdfs:label>
<foaf:name>Lloyd George&apos;s Pets</foaf:name>
<skos:prefLabel xml:lang="en">Lloyd George&apos;s Pets</skos:prefLabel>
<skos:definition xml:lang="en">Munition workers in England.</skos:definition>
<skos:inScheme rdf:resource="#OverTheTopDictionary"/>
<rdfs:isDefinedBy rdf:resource="http://rdf.muninn-project.org/ontologies/ott"/>
<rdf:type rdf:resource="http://dbpedia.org/resource/Irony"/>
<vs:term_status>Stable</vs:term_status>
<rdf:type rdf:resource="http://dbpedia.org/resource/Slang"/>
</skos:Concept>
<skos:Concept rdf:ID="LonelySoldier">
<rdfs:label xml:lang="en">Lonely Soldier</rdfs:label>
<foaf:name>Lonely Soldier</foaf:name>
<skos:prefLabel xml:lang="en">Lonely Soldier</skos:prefLabel>
<skos:definition xml:lang="en">A soldier who advertises himself as &quot;lonely&quot; through the medium of some English newspaper. If he is clever and diplomatic by this method he generally receives two or three parcels a week, but he must be careful not to write to two girls living on the same block or his parcel post mail will diminish.</skos:definition>
<skos:inScheme rdf:resource="#OverTheTopDictionary"/>
<rdf:type rdf:resource="http://dbpedia.org/resource/Slang"/>
<rdfs:isDefinedBy rdf:resource="http://rdf.muninn-project.org/ontologies/ott"/>
<rdf:type rdf:resource="http://dbpedia.org/resource/Irony"/>
<vs:term_status>Stable</vs:term_status>
</skos:Concept>
<skos:Concept rdf:ID="LonelyStab">
<rdfs:label xml:lang="en">Lonely Stab</rdfs:label>
<foaf:name>Lonely Stab</foaf:name>
<skos:prefLabel xml:lang="en">Lonely Stab</skos:prefLabel>
<skos:definition xml:lang="en">A girl who writes and sends parcels to Tommy. She got his name from the &quot;Lonely Soldier Column&quot; of some newspaper.</skos:definition>
<skos:inScheme rdf:resource="#OverTheTopDictionary"/>
<rdfs:isDefinedBy rdf:resource="http://rdf.muninn-project.org/ontologies/ott"/>
<rdf:type rdf:resource="http://dbpedia.org/resource/Irony"/>
<vs:term_status>Stable</vs:term_status>
<rdf:type rdf:resource="http://dbpedia.org/resource/Slang"/>
</skos:Concept>
<skos:Concept rdf:ID="Loophole">
<rdfs:label xml:lang="en">Loophole</rdfs:label>
<foaf:name>Loophole</foaf:name>
<skos:prefLabel xml:lang="en">Loophole</skos:prefLabel>
<skos:definition xml:lang="en">A disguised aperture in a trench through which to &quot;snipe&quot; at Germans.</skos:definition>
<skos:inScheme rdf:resource="#OverTheTopDictionary"/>
<rdfs:isDefinedBy rdf:resource="http://rdf.muninn-project.org/ontologies/ott"/>
<rdf:type rdf:resource="http://dbpedia.org/resource/Irony"/>
<vs:term_status>Stable</vs:term_status>
</skos:Concept>
<skos:Concept rdf:ID="Lyddite">
<rdfs:label xml:lang="en">Lyddite</rdfs:label>
<foaf:name>Lyddite</foaf:name>
<skos:prefLabel xml:lang="en">Lyddite</skos:prefLabel>
<skos:definition xml:lang="en">A high explosive used in shells. Has a habit of scattering bits of anatomy over the landscape.</skos:definition>
<skos:inScheme rdf:resource="#OverTheTopDictionary"/>
<rdfs:isDefinedBy rdf:resource="http://rdf.muninn-project.org/ontologies/ott"/>
<rdf:type rdf:resource="http://dbpedia.org/resource/Irony"/>
<vs:term_status>Stable</vs:term_status>
</skos:Concept>
<skos:Concept rdf:ID="MachineGunCorps">
<rdfs:label xml:lang="en">Machine Gun Corps</rdfs:label>
<muninn:acronym xml:lang="en">M.G.C.</muninn:acronym>
<foaf:name>Machine Gun Corps</foaf:name>
<skos:prefLabel xml:lang="en">Machine Gun Corps</skos:prefLabel>
<skos:definition xml:lang="en">A collection of machine gunners who think they are the deciding factor of the war, and that artillery is unnecessary.</skos:definition>
<skos:inScheme rdf:resource="#OverTheTopDictionary"/>
<rdfs:isDefinedBy rdf:resource="http://rdf.muninn-project.org/ontologies/ott"/>
<rdf:type rdf:resource="http://dbpedia.org/resource/Irony"/>
<vs:term_status>Stable</vs:term_status>
</skos:Concept>
<skos:Concept rdf:ID="MachineGunner">
<rdfs:label xml:lang="en">Machine Gunner</rdfs:label>
<muninn:acronym xml:lang="en">M.G.</muninn:acronym>
<foaf:name>Machine Gunner</foaf:name>
<skos:prefLabel xml:lang="en">Machine Gunner</skos:prefLabel>
<skos:definition xml:lang="en">A man who, like an American policeman, is never there when he is badly wanted.</skos:definition>
<skos:inScheme rdf:resource="#OverTheTopDictionary"/>
<rdfs:isDefinedBy rdf:resource="http://rdf.muninn-project.org/ontologies/ott"/>
<rdf:type rdf:resource="http://dbpedia.org/resource/Irony"/>
<vs:term_status>Stable</vs:term_status>
</skos:Concept>
<skos:Concept rdf:ID="Maconochie">
<rdfs:label xml:lang="en">Maconochie</rdfs:label>
<foaf:name>Maconochie</foaf:name>
<skos:prefLabel xml:lang="en">Maconochie</skos:prefLabel>
<skos:definition xml:lang="en">A ration of meat, vegetables, and soapy water, contained in a tin. Mr. Maconochie, the chemist who compounded this mess, intends to commit &quot;hari kari&quot; before the boys return from the front. He is wise.</skos:definition>
<skos:inScheme rdf:resource="#OverTheTopDictionary"/>
<rdfs:isDefinedBy rdf:resource="http://rdf.muninn-project.org/ontologies/ott"/>
<rdf:type rdf:resource="http://dbpedia.org/resource/Irony"/>
<rdf:type rdf:resource="http://dbpedia.org/resource/Slang"/>
<vs:term_status>Stable</vs:term_status>
</skos:Concept>
<skos:Concept rdf:ID="MadMinute">
<rdfs:label xml:lang="en">Mad Minute</rdfs:label>
<foaf:name>Mad Minute</foaf:name>
<skos:prefLabel xml:lang="en">Mad Minute</skos:prefLabel>
<skos:definition xml:lang="en">Firing fifteen rounds from your rifle in sixty seconds. A man is mad to attempt it, especially with a stiff bolt.</skos:definition>
<skos:inScheme rdf:resource="#OverTheTopDictionary"/>
<rdf:type rdf:resource="http://dbpedia.org/resource/Slang"/>
<rdfs:isDefinedBy rdf:resource="http://rdf.muninn-project.org/ontologies/ott"/>
<rdf:type rdf:resource="http://dbpedia.org/resource/Irony"/>
<vs:term_status>Stable</vs:term_status>
</skos:Concept>
<skos:Concept rdf:ID="MailBag">
<rdfs:label xml:lang="en">Mail Bag</rdfs:label>
<foaf:name>Mail Bag</foaf:name>
<skos:prefLabel xml:lang="en">Mail Bag</skos:prefLabel>
<skos:definition xml:lang="en">A canvas bag which is used to bring the other fellow&apos;s mail around.</skos:definition>
<skos:inScheme rdf:resource="#OverTheTopDictionary"/>
<rdfs:isDefinedBy rdf:resource="http://rdf.muninn-project.org/ontologies/ott"/>
<rdf:type rdf:resource="http://dbpedia.org/resource/Irony"/>
<vs:term_status>Stable</vs:term_status>
</skos:Concept>
<skos:Concept rdf:ID="Major">
<rdfs:label xml:lang="en">Major</rdfs:label>
<foaf:name>Major</foaf:name>
<skos:prefLabel xml:lang="en">Major</skos:prefLabel>
<skos:definition xml:lang="en">An officer in a Battalion who wears a crown on his uniform, is in command of two companies, and corrects said companies in the second position of &quot;present arms.&quot; He also resides in a dugout.</skos:definition>
<skos:inScheme rdf:resource="#OverTheTopDictionary"/>
<rdfs:isDefinedBy rdf:resource="http://rdf.muninn-project.org/ontologies/ott"/>
<rdf:type rdf:resource="http://dbpedia.org/resource/Irony"/>
<vs:term_status>Stable</vs:term_status>
</skos:Concept>
<skos:Concept rdf:ID="Maneuvers">
<rdfs:label xml:lang="en">Maneuvers</rdfs:label>
<foaf:name>Maneuvers</foaf:name>
<skos:prefLabel xml:lang="en">Maneuvers</skos:prefLabel>
<skos:definition xml:lang="en">Useless evolutions of troops conceived by someone higher up to show Tommy how brave his officers are and how battles should be fought. The enemy never attend these maneuvers to prove they&apos;re right.</skos:definition>
<skos:inScheme rdf:resource="#OverTheTopDictionary"/>
<rdfs:isDefinedBy rdf:resource="http://rdf.muninn-project.org/ontologies/ott"/>
<rdf:type rdf:resource="http://dbpedia.org/resource/Irony"/>
<vs:term_status>Stable</vs:term_status>
</skos:Concept>
<skos:Concept rdf:ID="MassFormation">
<rdfs:label xml:lang="en">Mass Formation</rdfs:label>
<foaf:name>Mass Formation</foaf:name>
<skos:prefLabel xml:lang="en">Mass Formation</skos:prefLabel>
<skos:definition xml:lang="en">A dose order formation in which the Germans attack. It gives them a sort of &quot;Come on, I&apos;m with you&quot; feeling. They would &quot;hold hands&quot; only for the fact that they have to carry their rifles. Tommy takes great delight in &quot;busting up&quot; these gatherings.</skos:definition>
<skos:inScheme rdf:resource="#OverTheTopDictionary"/>
<rdfs:isDefinedBy rdf:resource="http://rdf.muninn-project.org/ontologies/ott"/>
<rdf:type rdf:resource="http://dbpedia.org/resource/Irony"/>
<vs:term_status>Stable</vs:term_status>
</skos:Concept>
<skos:Concept rdf:ID="Mate">
<rdfs:label xml:lang="en">Mate</rdfs:label>
<foaf:name>Mate</foaf:name>
<skos:prefLabel xml:lang="en">Mate</skos:prefLabel>
<skos:definition xml:lang="en">A soldier with whom Tommy is especially &quot;chummy.&quot; Generally picked because this soldier receives a parcel from home every week.</skos:definition>
<skos:inScheme rdf:resource="#OverTheTopDictionary"/>
<rdfs:isDefinedBy rdf:resource="http://rdf.muninn-project.org/ontologies/ott"/>
<rdf:type rdf:resource="http://dbpedia.org/resource/Irony"/>
<vs:term_status>Stable</vs:term_status>
</skos:Concept>
<skos:Concept rdf:ID="Maxim">
<rdfs:label xml:lang="en">Maxim</rdfs:label>
<foaf:name>Maxim</foaf:name>
<skos:prefLabel xml:lang="en">Maxim</skos:prefLabel>
<skos:definition xml:lang="en">Type of machine gun which has been supplanted by the Vickers in order to make Tommy unlearn what he has been taught about the Maxim.</skos:definition>
<skos:inScheme rdf:resource="#OverTheTopDictionary"/>
<rdfs:isDefinedBy rdf:resource="http://rdf.muninn-project.org/ontologies/ott"/>
<rdf:type rdf:resource="http://dbpedia.org/resource/Irony"/>
<vs:term_status>Stable</vs:term_status>
</skos:Concept>
<skos:Concept rdf:ID="MechanicalTransport">
<rdfs:label xml:lang="en">Mechanical Transport</rdfs:label>
<muninn:acronym xml:lang="en">M.T.</muninn:acronym>
<foaf:name>Mechanical Transport</foaf:name>
<skos:prefLabel xml:lang="en">Mechanical Transport</skos:prefLabel>
<skos:definition xml:lang="en">The members of which are ex-taxi drivers. No wonder Tommy&apos;s rations melt away when the M. T. carries them.</skos:definition>
<skos:inScheme rdf:resource="#OverTheTopDictionary"/>
<rdfs:isDefinedBy rdf:resource="http://rdf.muninn-project.org/ontologies/ott"/>
<rdf:type rdf:resource="http://dbpedia.org/resource/Irony"/>
<vs:term_status>Stable</vs:term_status>
</skos:Concept>
<skos:Concept rdf:ID="MedicalOfficer">
<rdfs:label xml:lang="en">Medical Officer</rdfs:label>
<muninn:acronym xml:lang="en">M.O.</muninn:acronym>
<foaf:name>Medical Officer</foaf:name>
<skos:prefLabel xml:lang="en">Medical Officer</skos:prefLabel>
<skos:definition xml:lang="en">A doctor specially detailed to tell Tommy that he is not sick.</skos:definition>
<skos:inScheme rdf:resource="#OverTheTopDictionary"/>
<rdfs:isDefinedBy rdf:resource="http://rdf.muninn-project.org/ontologies/ott"/>
<rdf:type rdf:resource="http://dbpedia.org/resource/Irony"/>
<vs:term_status>Stable</vs:term_status>
</skos:Concept>
<skos:Concept rdf:ID="MedicineandDuty">
<rdfs:label xml:lang="en">Medicine and Duty</rdfs:label>
<muninn:acronym xml:lang="en">M. and D.</muninn:acronym>
<foaf:name>Medicine and Duty</foaf:name>
<skos:prefLabel xml:lang="en">Medicine and Duty</skos:prefLabel>
<skos:definition xml:lang="en">What the doctor marks on the &quot;sicker&quot; or side report when he thinks Tommy is faking sickness. It means medicine and duty.</skos:definition>
<skos:inScheme rdf:resource="#OverTheTopDictionary"/>
<rdfs:isDefinedBy rdf:resource="http://rdf.muninn-project.org/ontologies/ott"/>
<rdf:type rdf:resource="http://dbpedia.org/resource/Irony"/>
<vs:term_status>Stable</vs:term_status>
</skos:Concept>
<skos:Concept rdf:ID="MentionedinDespatches">
<rdfs:label xml:lang="en">Mentioned in Despatches</rdfs:label>
<foaf:name>Mentioned in Despatches</foaf:name>
<skos:prefLabel xml:lang="en">Mentioned in Despatches</skos:prefLabel>
<skos:definition xml:lang="en">Recommended for bravery. Tommy would sooner be recommended for leave.</skos:definition>
<skos:inScheme rdf:resource="#OverTheTopDictionary"/>
<rdfs:isDefinedBy rdf:resource="http://rdf.muninn-project.org/ontologies/ott"/>
<rdf:type rdf:resource="http://dbpedia.org/resource/Irony"/>
<vs:term_status>Stable</vs:term_status>
</skos:Concept>
<skos:Concept rdf:ID="MercyKamerad">
<rdfs:label xml:lang="en">Mercy Kamerad</rdfs:label>
<foaf:name>Mercy Kamerad</foaf:name>
<skos:prefLabel xml:lang="en">Mercy Kamerad</skos:prefLabel>
<skos:definition xml:lang="en">What Fritz says when he has had a bellyful of fighting and wants to surrender. Of late this has been quite a popular phrase with him, replacing the Hymn of Hate.</skos:definition>
<skos:inScheme rdf:resource="#OverTheTopDictionary"/>
<rdfs:isDefinedBy rdf:resource="http://rdf.muninn-project.org/ontologies/ott"/>
<rdf:type rdf:resource="http://dbpedia.org/resource/Irony"/>
<vs:term_status>Stable</vs:term_status>
<rdf:type rdf:resource="http://dbpedia.org/resource/Slang"/>
</skos:Concept>
<skos:Concept rdf:ID="MessOrderly">
<rdfs:label xml:lang="en">Mess Orderly</rdfs:label>
<foaf:name>Mess Orderly</foaf:name>
<skos:prefLabel xml:lang="en">Mess Orderly</skos:prefLabel>
<skos:definition xml:lang="en">A soldier detailed daily to carry Tommy&apos;s meals to and from the cook-house.</skos:definition>
<skos:inScheme rdf:resource="#OverTheTopDictionary"/>
<rdfs:isDefinedBy rdf:resource="http://rdf.muninn-project.org/ontologies/ott"/>
<rdf:type rdf:resource="http://dbpedia.org/resource/Irony"/>
<vs:term_status>Stable</vs:term_status>
</skos:Concept>
<skos:Concept rdf:ID="MessTin">
<rdfs:label xml:lang="en">Mess Tin</rdfs:label>
<foaf:name>Mess Tin</foaf:name>
<skos:prefLabel xml:lang="en">Mess Tin</skos:prefLabel>
<skos:definition xml:lang="en">An article of equipment used as a tea-kettle and dinner-set.</skos:definition>
<skos:inScheme rdf:resource="#OverTheTopDictionary"/>
<rdfs:isDefinedBy rdf:resource="http://rdf.muninn-project.org/ontologies/ott"/>
<rdf:type rdf:resource="http://dbpedia.org/resource/Irony"/>
<vs:term_status>Stable</vs:term_status>
</skos:Concept>
<skos:Concept rdf:ID="MikeandGeorge">
<rdfs:label xml:lang="en">Mike and George</rdfs:label>
<muninn:acronym xml:lang="en">K. C. M. G.</muninn:acronym>
<foaf:name>Mike and George</foaf:name>
<skos:prefLabel xml:lang="en">Mike and George</skos:prefLabel>
<skos:definition xml:lang="en">Knight Commander of the Order of St. Michael and St. George. An award for bravery in the field.</skos:definition>
<skos:inScheme rdf:resource="#OverTheTopDictionary"/>
<rdfs:isDefinedBy rdf:resource="http://rdf.muninn-project.org/ontologies/ott"/>
<rdf:type rdf:resource="http://dbpedia.org/resource/Irony"/>
<vs:term_status>Stable</vs:term_status>
<rdf:type rdf:resource="http://dbpedia.org/resource/Slang"/>
</skos:Concept>
<skos:Concept rdf:ID="MilitaryCross">
<rdfs:label xml:lang="en">Military Cross</rdfs:label>
<foaf:name>Military Cross</foaf:name>
<skos:prefLabel xml:lang="en">Military Cross</skos:prefLabel>
<skos:definition xml:lang="en">A badge of honor dished out to officers for bravery. Tommy insists they throw dice to see which is the bravest. The winner gets the medal.</skos:definition>
<skos:inScheme rdf:resource="#OverTheTopDictionary"/>
<rdfs:isDefinedBy rdf:resource="http://rdf.muninn-project.org/ontologies/ott"/>
<rdf:type rdf:resource="http://dbpedia.org/resource/Irony"/>
<vs:term_status>Stable</vs:term_status>
</skos:Concept>
<skos:Concept rdf:ID="MilitaryMedal">
<rdfs:label xml:lang="en">Military Medal</rdfs:label>
<foaf:name>Military Medal</foaf:name>
<skos:prefLabel xml:lang="en">Military Medal</skos:prefLabel>
<skos:definition xml:lang="en">A piece of Junk issued to Tommy who has done something that is not exactly brave but still is not cowardly. When it is presented he takes it and goes back wondering why the Army picks on him.</skos:definition>
<skos:inScheme rdf:resource="#OverTheTopDictionary"/>
<rdfs:isDefinedBy rdf:resource="http://rdf.muninn-project.org/ontologies/ott"/>
<rdf:type rdf:resource="http://dbpedia.org/resource/Irony"/>
<vs:term_status>Stable</vs:term_status>
</skos:Concept>
<skos:Concept rdf:ID="MilitaryPolice">
<rdfs:label xml:lang="en">Military Police</rdfs:label>
<muninn:acronym xml:lang="en">M.P.</muninn:acronym>
<foaf:name>Military Police</foaf:name>
<skos:prefLabel xml:lang="en">Military Police</skos:prefLabel>
<skos:definition xml:lang="en">Soldiers with whom it is unsafe to argue.</skos:definition>
<skos:inScheme rdf:resource="#OverTheTopDictionary"/>
<rdfs:isDefinedBy rdf:resource="http://rdf.muninn-project.org/ontologies/ott"/>
<rdf:type rdf:resource="http://dbpedia.org/resource/Irony"/>
<vs:term_status>Stable</vs:term_status>
</skos:Concept>
<skos:Concept rdf:ID="Mills">
<rdfs:label xml:lang="en">Mills</rdfs:label>
<foaf:name>Mills</foaf:name>
<skos:prefLabel xml:lang="en">Mills</skos:prefLabel>
<skos:definition xml:lang="en">Name of a bomb invented by Mills. The only bomb in which Tommy has full confidence, -- and he mistrusts even that.</skos:definition>
<skos:inScheme rdf:resource="#OverTheTopDictionary"/>
<rdfs:isDefinedBy rdf:resource="http://rdf.muninn-project.org/ontologies/ott"/>
<rdf:type rdf:resource="http://dbpedia.org/resource/Irony"/>
<vs:term_status>Stable</vs:term_status>
</skos:Concept>
<skos:Concept rdf:ID="Mine">
<rdfs:label xml:lang="en">Mine</rdfs:label>
<foaf:name>Mine</foaf:name>
<skos:prefLabel xml:lang="en">Mine</skos:prefLabel>
<skos:definition xml:lang="en">An underground tunnel dug by sappers of the Royal Engineer Corps. This tunnel leads from your trench to that of the enemy&apos;s. At the end or head of the tunnel a great quantity of explosives are stored which at a given time are exploded. It is Tommy&apos;s job to then go &quot;over the top&quot; and occupy the crater caused by the explosion.</skos:definition>
<skos:inScheme rdf:resource="#OverTheTopDictionary"/>
<rdfs:isDefinedBy rdf:resource="http://rdf.muninn-project.org/ontologies/ott"/>
<rdf:type rdf:resource="http://dbpedia.org/resource/Irony"/>
<vs:term_status>Stable</vs:term_status>
</skos:Concept>
<skos:Concept rdf:ID="MineShaft">
<rdfs:label xml:lang="en">Mine Shaft</rdfs:label>
<foaf:name>Mine Shaft</foaf:name>
<skos:prefLabel xml:lang="en">Mine Shaft</skos:prefLabel>
<skos:definition xml:lang="en">A shaft leading down to the &quot;gallery&quot; or tunnel of a mine. Sometimes Tommy, as a reward, is given the Job of helping the R. E.&apos;s dig this shaft.</skos:definition>
<skos:inScheme rdf:resource="#OverTheTopDictionary"/>
<rdfs:isDefinedBy rdf:resource="http://rdf.muninn-project.org/ontologies/ott"/>
<rdf:type rdf:resource="http://dbpedia.org/resource/Irony"/>
<vs:term_status>Stable</vs:term_status>
</skos:Concept>
<skos:Concept rdf:ID="Minnenwerfer">
<rdfs:label xml:lang="en">Minnenwerfer</rdfs:label>
<foaf:name>Minnenwerfer</foaf:name>
<skos:prefLabel xml:lang="en">Minnenwerfer</skos:prefLabel>
<skos:definition xml:lang="en">A high-power trench mortar shell of the Germans, which makes no noise coming through the air. It was invented by Professor Kultur. Tommy does not know what is near until it bites him; after that nothing worries him. Tommy nicknames them &quot;Minnies.&quot;</skos:definition>
<skos:inScheme rdf:resource="#OverTheTopDictionary"/>
<rdfs:isDefinedBy rdf:resource="http://rdf.muninn-project.org/ontologies/ott"/>
<rdf:type rdf:resource="http://dbpedia.org/resource/Irony"/>
<rdf:type rdf:resource="http://dbpedia.org/resource/Slang"/>
<vs:term_status>Stable</vs:term_status>
</skos:Concept>
<skos:Concept rdf:ID="MouthOrgan">
<rdfs:label xml:lang="en">Mouth Organ</rdfs:label>
<foaf:name>Mouth Organ</foaf:name>
<skos:prefLabel xml:lang="en">Mouth Organ</skos:prefLabel>
<skos:definition xml:lang="en">An instrument with which a vindictive Tommy causes misery to the rest of his platoon. Some authorities define it as a &quot;musical instrument.&quot;</skos:definition>
<skos:inScheme rdf:resource="#OverTheTopDictionary"/>
<rdfs:isDefinedBy rdf:resource="http://rdf.muninn-project.org/ontologies/ott"/>
<rdf:type rdf:resource="http://dbpedia.org/resource/Irony"/>
<vs:term_status>Stable</vs:term_status>
</skos:Concept>
<skos:Concept rdf:ID="Mud">
<rdfs:label xml:lang="en">Mud</rdfs:label>
<foaf:name>Mud</foaf:name>
<skos:prefLabel xml:lang="en">Mud</skos:prefLabel>
<skos:definition xml:lang="en">A brownish, sticky substance found in the trenches after the frequent rains. A true friend to Tommy, which sticks to him like glue, even though at times Tommy resents this affection and roundly curses said mud.</skos:definition>
<skos:inScheme rdf:resource="#OverTheTopDictionary"/>
<rdfs:isDefinedBy rdf:resource="http://rdf.muninn-project.org/ontologies/ott"/>
<rdf:type rdf:resource="http://dbpedia.org/resource/Irony"/>
<vs:term_status>Stable</vs:term_status>
</skos:Concept>
<skos:Concept rdf:ID="Mufti">
<rdfs:label xml:lang="en">Mufti</rdfs:label>
<foaf:name>Mufti</foaf:name>
<skos:prefLabel xml:lang="en">Mufti</skos:prefLabel>
<skos:definition xml:lang="en">The term Tommy gives to civilian clothes. Mufti looks good to him now.</skos:definition>
<skos:inScheme rdf:resource="#OverTheTopDictionary"/>
<rdfs:isDefinedBy rdf:resource="http://rdf.muninn-project.org/ontologies/ott"/>
<rdf:type rdf:resource="http://dbpedia.org/resource/Irony"/>
<vs:term_status>Stable</vs:term_status>
<rdf:type rdf:resource="http://dbpedia.org/resource/Slang"/>
</skos:Concept>
<skos:Concept rdf:ID="Nap">
<rdfs:label xml:lang="en">Nap</rdfs:label>
<foaf:name>Nap</foaf:name>
<skos:prefLabel xml:lang="en">Nap</skos:prefLabel>
<skos:definition xml:lang="en">A card game of Tommy&apos;s in which the one who stays awake the longest grabs the pot. If all the players fall asleep, the pot goes to the &quot;Wounded Soldiers&apos; Fund.&quot;</skos:definition>
<skos:inScheme rdf:resource="#OverTheTopDictionary"/>
<rdfs:isDefinedBy rdf:resource="http://rdf.muninn-project.org/ontologies/ott"/>
<rdf:type rdf:resource="http://dbpedia.org/resource/Irony"/>
<vs:term_status>Stable</vs:term_status>
<rdf:type rdf:resource="http://dbpedia.org/resource/Slang"/>
</skos:Concept>
<skos:Concept rdf:ID="NapooFini">
<rdfs:label xml:lang="en">Napoo-Fini</rdfs:label>
<foaf:name>Napoo-Fini</foaf:name>
<skos:prefLabel xml:lang="en">Napoo-Fini</skos:prefLabel>
<skos:definition xml:lang="en">Tommy&apos;s French for gone, through with, finished, disappeared.</skos:definition>
<skos:inScheme rdf:resource="#OverTheTopDictionary"/>
<rdfs:isDefinedBy rdf:resource="http://rdf.muninn-project.org/ontologies/ott"/>
<rdf:type rdf:resource="http://dbpedia.org/resource/Irony"/>
<rdf:type rdf:resource="http://dbpedia.org/resource/Slang"/>
<vs:term_status>Stable</vs:term_status>
</skos:Concept>
<skos:Concept rdf:ID="Napper">
<rdfs:label xml:lang="en">Napper</rdfs:label>
<foaf:name>Napper</foaf:name>
<skos:prefLabel xml:lang="en">Napper</skos:prefLabel>
<skos:definition xml:lang="en">Tommy&apos;s term for bead.</skos:definition>
<skos:inScheme rdf:resource="#OverTheTopDictionary"/>
<rdfs:isDefinedBy rdf:resource="http://rdf.muninn-project.org/ontologies/ott"/>
<rdf:type rdf:resource="http://dbpedia.org/resource/Irony"/>
<vs:term_status>Stable</vs:term_status>
</skos:Concept>
<skos:Concept rdf:ID="Neutral">
<rdfs:label xml:lang="en">Neutral</rdfs:label>
<foaf:name>Neutral</foaf:name>
<skos:prefLabel xml:lang="en">Neutral</skos:prefLabel>
<skos:definition xml:lang="en">Tommy says it means &quot;afraid to fight.&quot;</skos:definition>
<skos:inScheme rdf:resource="#OverTheTopDictionary"/>
<rdfs:isDefinedBy rdf:resource="http://rdf.muninn-project.org/ontologies/ott"/>
<rdf:type rdf:resource="http://dbpedia.org/resource/Irony"/>
<vs:term_status>Stable</vs:term_status>
</skos:Concept>
<skos:Concept rdf:ID="NextofKin">
<rdfs:label xml:lang="en">Next of Kin</rdfs:label>
<foaf:name>Next of Kin</foaf:name>
<skos:prefLabel xml:lang="en">Next of Kin</skos:prefLabel>
<skos:definition xml:lang="en">Nearest relative. A young and ambitious platoon officer bothers his men two or three times a month taking a record of their &quot;next of kin,&quot; because he thinks that Tommy&apos;s grandmother may have changed to his uncle.</skos:definition>
<skos:inScheme rdf:resource="#OverTheTopDictionary"/>
<rdfs:isDefinedBy rdf:resource="http://rdf.muninn-project.org/ontologies/ott"/>
<rdf:type rdf:resource="http://dbpedia.org/resource/Irony"/>
<vs:term_status>Stable</vs:term_status>
</skos:Concept>
<skos:Concept rdf:ID="Nightops">
<rdfs:label xml:lang="en">Night ops</rdfs:label>
<foaf:name>Night ops</foaf:name>
<skos:prefLabel xml:lang="en">Night ops</skos:prefLabel>
<skos:definition xml:lang="en">Slang for night operations or maneuvers.</skos:definition>
<skos:inScheme rdf:resource="#OverTheTopDictionary"/>
<rdfs:isDefinedBy rdf:resource="http://rdf.muninn-project.org/ontologies/ott"/>
<rdf:type rdf:resource="http://dbpedia.org/resource/Irony"/>
<vs:term_status>Stable</vs:term_status>
</skos:Concept>
<skos:Concept rdf:ID="NinePointTwo">
<rdfs:label xml:lang="en">Nine-point-two</rdfs:label>
<foaf:name>Nine-point-two</foaf:name>
<skos:prefLabel xml:lang="en">Nine-point-two</skos:prefLabel>
<skos:definition xml:lang="en">A howitzer which fires a shell 9.2 inches in diameter, and knocks the tiles off the roof of Tommy&apos;s billet through the force of its concussion.</skos:definition>
<skos:inScheme rdf:resource="#OverTheTopDictionary"/>
<rdfs:isDefinedBy rdf:resource="http://rdf.muninn-project.org/ontologies/ott"/>
<rdf:type rdf:resource="http://dbpedia.org/resource/Slang"/>
<rdf:type rdf:resource="http://dbpedia.org/resource/Irony"/>
<vs:term_status>Stable</vs:term_status>
</skos:Concept>
<skos:Concept rdf:ID="NoMansLand">
<rdfs:label xml:lang="en">No Man&apos;s Land</rdfs:label>
<foaf:name>No Man&apos;s Land</foaf:name>
<skos:prefLabel xml:lang="en">No Man&apos;s Land</skos:prefLabel>
<skos:definition xml:lang="en">The space between the hostile trenches called &quot;No Man&apos;s Land&quot; because no one owns it and no one wants to. In France you could not give it away.</skos:definition>
<skos:inScheme rdf:resource="#OverTheTopDictionary"/>
<rdfs:isDefinedBy rdf:resource="http://rdf.muninn-project.org/ontologies/ott"/>
<rdf:type rdf:resource="http://dbpedia.org/resource/Irony"/>
<rdf:type rdf:resource="http://dbpedia.org/resource/Slang"/>
<vs:term_status>Stable</vs:term_status>
</skos:Concept>
<skos:Concept rdf:ID="NonCombatantCorps">
<rdfs:label xml:lang="en">Non-Combatant Corps</rdfs:label>
<muninn:acronym xml:lang="en">N.C.C.</muninn:acronym>
<foaf:name>Non-Combatant Corps</foaf:name>
<skos:prefLabel xml:lang="en">Non-Combatant Corps</skos:prefLabel>
<skos:definition xml:lang="en">Men who joined the Army under the stipulation that the only thing they would fight for would be their meals. They have no &quot;King and Country.&quot;</skos:definition>
<skos:inScheme rdf:resource="#OverTheTopDictionary"/>
<rdfs:isDefinedBy rdf:resource="http://rdf.muninn-project.org/ontologies/ott"/>
<rdf:type rdf:resource="http://dbpedia.org/resource/Irony"/>
<vs:term_status>Stable</vs:term_status>
</skos:Concept>
<skos:Concept rdf:ID="NonCommissionedOfficer">
<rdfs:label xml:lang="en">Non-commissioned officer</rdfs:label>
<muninn:acronym xml:lang="en">N.C.O.</muninn:acronym>
<foaf:name>Non-commissioned officer</foaf:name>
<skos:prefLabel xml:lang="en">Non-commissioned officer</skos:prefLabel>
<skos:definition xml:lang="en">A person hated more than the Germans. Tommy says his stripes are issued out with the rations, and he ought to know.</skos:definition>
<skos:inScheme rdf:resource="#OverTheTopDictionary"/>
<rdfs:isDefinedBy rdf:resource="http://rdf.muninn-project.org/ontologies/ott"/>
<rdf:type rdf:resource="http://dbpedia.org/resource/Irony"/>
<vs:term_status>Stable</vs:term_status>
</skos:Concept>
<skos:Concept rdf:ID="No9">
<rdfs:label xml:lang="en">No. 9.</rdfs:label>
<foaf:name>No. 9.</foaf:name>
<skos:prefLabel xml:lang="en">No. 9.</skos:prefLabel>
<skos:definition xml:lang="en">A pill the doctor gives you if you are suffering with corns or barber&apos;s itch or any disease at all. If none are in stock, he gives you a No. 6 and No. 3, or a No. 5 and No. 4, anything to make nine.</skos:definition>
<skos:inScheme rdf:resource="#OverTheTopDictionary"/>
<rdfs:isDefinedBy rdf:resource="http://rdf.muninn-project.org/ontologies/ott"/>
<rdf:type rdf:resource="http://dbpedia.org/resource/Irony"/>
<vs:term_status>Stable</vs:term_status>
</skos:Concept>
<skos:Concept rdf:ID="Nosecap">
<rdfs:label xml:lang="en">Nosecap</rdfs:label>
<foaf:name>Nosecap</foaf:name>
<skos:prefLabel xml:lang="en">Nosecap</skos:prefLabel>
<skos:definition xml:lang="en">That part of a shell which unscrews and contains the device and scale for setting the time fuse. Some Tommies are ardent souvenir hunters. As soon as a shell bursts in the ground you will see them out with picks and shovels digging in the shell hole for the nose cap. If the shell bursts too near them they don&apos;t dig.</skos:definition>
<skos:inScheme rdf:resource="#OverTheTopDictionary"/>
<rdfs:isDefinedBy rdf:resource="http://rdf.muninn-project.org/ontologies/ott"/>
<rdf:type rdf:resource="http://dbpedia.org/resource/Irony"/>
<vs:term_status>Stable</vs:term_status>
</skos:Concept>
<skos:Concept rdf:ID="ObservationBalloon">
<rdfs:label xml:lang="en">Observation Balloon</rdfs:label>
<foaf:name>Observation Balloon</foaf:name>
<skos:prefLabel xml:lang="en">Observation Balloon</skos:prefLabel>
<skos:definition xml:lang="en">A captive balloon behind the lines which observes the enemy. The enemy doesn&apos;t mind being observed, so takes no notice of it. It gives someone a job hauling it down at night, so it has one good point.</skos:definition>
<skos:inScheme rdf:resource="#OverTheTopDictionary"/>
<rdfs:isDefinedBy rdf:resource="http://rdf.muninn-project.org/ontologies/ott"/>
<rdf:type rdf:resource="http://dbpedia.org/resource/Irony"/>
<vs:term_status>Stable</vs:term_status>
</skos:Concept>
<skos:Concept rdf:ID="ObservationPost">
<rdfs:label xml:lang="en">Observation Post</rdfs:label>
<foaf:name>Observation Post</foaf:name>
<skos:prefLabel xml:lang="en">Observation Post</skos:prefLabel>
<skos:definition xml:lang="en">A position in the front line where an artillery officer observes the fire of our guns. He keeps on observing until a German shell observes him. After this there is generally a new officer and a new observation post.</skos:definition>
<skos:inScheme rdf:resource="#OverTheTopDictionary"/>
<rdfs:isDefinedBy rdf:resource="http://rdf.muninn-project.org/ontologies/ott"/>
<rdf:type rdf:resource="http://dbpedia.org/resource/Irony"/>
<vs:term_status>Stable</vs:term_status>
</skos:Concept>
<skos:Concept rdf:ID="Officercommanding">
<rdfs:label xml:lang="en">Officer commanding.</rdfs:label>
<muninn:acronym xml:lang="en">O.C.</muninn:acronym>
<foaf:name>Officer commanding.</foaf:name>
<skos:prefLabel xml:lang="en">Officer commanding.</skos:prefLabel>
<skos:definition xml:lang="en"></skos:definition>
<skos:inScheme rdf:resource="#OverTheTopDictionary"/>
<rdfs:isDefinedBy rdf:resource="http://rdf.muninn-project.org/ontologies/ott"/>
<rdf:type rdf:resource="http://dbpedia.org/resource/Irony"/>
<vs:term_status>Stable</vs:term_status>
</skos:Concept>
<skos:Concept rdf:ID="OfficersMess">
<rdfs:label xml:lang="en">Officers&apos; Mess</rdfs:label>
<foaf:name>Officers&apos; Mess</foaf:name>
<skos:prefLabel xml:lang="en">Officers&apos; Mess</skos:prefLabel>
<skos:definition xml:lang="en">Where the officers eat the mess that the O. S. have cooked.</skos:definition>
<skos:inScheme rdf:resource="#OverTheTopDictionary"/>
<rdfs:isDefinedBy rdf:resource="http://rdf.muninn-project.org/ontologies/ott"/>
<rdf:type rdf:resource="http://dbpedia.org/resource/Irony"/>
<vs:term_status>Stable</vs:term_status>
</skos:Concept>
<skos:Concept rdf:ID="Officersservants">
<rdfs:label xml:lang="en">Officers&apos; servants</rdfs:label>
<muninn:acronym xml:lang="en">O.S.</muninn:acronym>
<foaf:name>Officers&apos; servants</foaf:name>
<skos:prefLabel xml:lang="en">Officers&apos; servants</skos:prefLabel>
<skos:definition xml:lang="en">The lowest ranking private in the Army, who feeds better than the officers he waits on.</skos:definition>
<skos:inScheme rdf:resource="#OverTheTopDictionary"/>
<rdfs:isDefinedBy rdf:resource="http://rdf.muninn-project.org/ontologies/ott"/>
<rdf:type rdf:resource="http://dbpedia.org/resource/Irony"/>
<vs:term_status>Stable</vs:term_status>
</skos:Concept>
<skos:Concept rdf:ID="OilCans">
<rdfs:label xml:lang="en">Oil Cans</rdfs:label>
<foaf:name>Oil Cans</foaf:name>
<skos:prefLabel xml:lang="en">Oil Cans</skos:prefLabel>
<skos:definition xml:lang="en">Tommy&apos;s term for a German trench mortar shell, which is an old tin filled with explosive and junk that the Boches have no further use for.</skos:definition>
<skos:inScheme rdf:resource="#OverTheTopDictionary"/>
<rdfs:isDefinedBy rdf:resource="http://rdf.muninn-project.org/ontologies/ott"/>
<rdf:type rdf:resource="http://dbpedia.org/resource/Irony"/>
<vs:term_status>Stable</vs:term_status>
</skos:Concept>
<skos:Concept rdf:ID="Oneup">
<rdfs:label xml:lang="en">One up</rdfs:label>
<foaf:name>One up</foaf:name>
<skos:prefLabel xml:lang="en">One up</skos:prefLabel>
<skos:definition xml:lang="en">Tommy&apos;s term for a lance-corporal who wears one stripe. The private always wonders why he was overlooked when promotions were in order.</skos:definition>
<skos:inScheme rdf:resource="#OverTheTopDictionary"/>
<rdfs:isDefinedBy rdf:resource="http://rdf.muninn-project.org/ontologies/ott"/>
<rdf:type rdf:resource="http://dbpedia.org/resource/Irony"/>
<vs:term_status>Stable</vs:term_status>
</skos:Concept>
<skos:Concept rdf:ID="Onthemat">
<rdfs:label xml:lang="en">On the mat</rdfs:label>
<foaf:name>On the mat</foaf:name>
<skos:prefLabel xml:lang="en">On the mat</skos:prefLabel>
<skos:definition xml:lang="en">When Tommy is haled before his commanding officer to explain why he has broken one of the seven million King&apos;s regulations for the government of the Army. His &quot;explanation&quot; never gets him anywhere unless it is on the wheel of a Umber.</skos:definition>
<skos:inScheme rdf:resource="#OverTheTopDictionary"/>
<rdfs:isDefinedBy rdf:resource="http://rdf.muninn-project.org/ontologies/ott"/>
<rdf:type rdf:resource="http://dbpedia.org/resource/Irony"/>
<rdf:type rdf:resource="http://dbpedia.org/resource/Slang"/>
<vs:term_status>Stable</vs:term_status>
</skos:Concept>
<skos:Concept rdf:ID="Onyourown">
<rdfs:label xml:lang="en">On your own</rdfs:label>
<foaf:name>On your own</foaf:name>
<skos:prefLabel xml:lang="en">On your own</skos:prefLabel>
<skos:definition xml:lang="en">Another famous or infamous phrase which means Tommy is allowed to do as he pleases. An officer generally puts Tommy &quot;on his own&quot; when he gets Tommy into a dangerous position and sees no way to extricate him.</skos:definition>
<skos:inScheme rdf:resource="#OverTheTopDictionary"/>
<rdfs:isDefinedBy rdf:resource="http://rdf.muninn-project.org/ontologies/ott"/>
<rdf:type rdf:resource="http://dbpedia.org/resource/Irony"/>
<vs:term_status>Stable</vs:term_status>
</skos:Concept>
<skos:Concept rdf:ID="OrderlyCorporal">
<rdfs:label xml:lang="en">Orderly-Corporal</rdfs:label>
<foaf:name>Orderly-Corporal</foaf:name>
<skos:prefLabel xml:lang="en">Orderly-Corporal</skos:prefLabel>
<skos:definition xml:lang="en">A non-commissioned officer who takes the names of the sick every morning and who keeps his own candle burning after he has ordered &quot;Lights out&quot; at night.</skos:definition>
<skos:inScheme rdf:resource="#OverTheTopDictionary"/>
<rdfs:isDefinedBy rdf:resource="http://rdf.muninn-project.org/ontologies/ott"/>
<rdf:type rdf:resource="http://dbpedia.org/resource/Irony"/>
<vs:term_status>Stable</vs:term_status>
</skos:Concept>
<skos:Concept rdf:ID="OrderlyOfficer">
<rdfs:label xml:lang="en">Orderly-Officer</rdfs:label>
<foaf:name>Orderly-Officer</foaf:name>
<skos:prefLabel xml:lang="en">Orderly-Officer</skos:prefLabel>
<skos:definition xml:lang="en">An officer who, for a week, goes around and asks if there are &quot;any complaints&quot; and gives the name of the complaining soldier to the Orderly-Sergeant for extra pack drill.</skos:definition>
<skos:inScheme rdf:resource="#OverTheTopDictionary"/>
<rdfs:isDefinedBy rdf:resource="http://rdf.muninn-project.org/ontologies/ott"/>
<rdf:type rdf:resource="http://dbpedia.org/resource/Irony"/>
<vs:term_status>Stable</vs:term_status>
</skos:Concept>
<skos:Concept rdf:ID="OrderlyRoom">
<rdfs:label xml:lang="en">Orderly Room</rdfs:label>
<foaf:name>Orderly Room</foaf:name>
<skos:prefLabel xml:lang="en">Orderly Room</skos:prefLabel>
<skos:definition xml:lang="en">The Captain&apos;s office where everything is disorderly.</skos:definition>
<skos:inScheme rdf:resource="#OverTheTopDictionary"/>
<rdfs:isDefinedBy rdf:resource="http://rdf.muninn-project.org/ontologies/ott"/>
<rdf:type rdf:resource="http://dbpedia.org/resource/Irony"/>
<vs:term_status>Stable</vs:term_status>
</skos:Concept>
<skos:Concept rdf:ID="OrderlySergeant">
<rdfs:label xml:lang="en">Orderly-Sergeant</rdfs:label>
<foaf:name>Orderly-Sergeant</foaf:name>
<skos:prefLabel xml:lang="en">Orderly-Sergeant</skos:prefLabel>
<skos:definition xml:lang="en">A sergeant who, for a week, is supposed to do the work of the Orderly-Officer.</skos:definition>
<skos:inScheme rdf:resource="#OverTheTopDictionary"/>
<rdfs:isDefinedBy rdf:resource="http://rdf.muninn-project.org/ontologies/ott"/>
<rdf:type rdf:resource="http://dbpedia.org/resource/Irony"/>
<vs:term_status>Stable</vs:term_status>
</skos:Concept>
<skos:Concept rdf:ID="Outofbounds">
<rdfs:label xml:lang="en">Out of bounds</rdfs:label>
<foaf:name>Out of bounds</foaf:name>
<skos:prefLabel xml:lang="en">Out of bounds</skos:prefLabel>
<skos:definition xml:lang="en">The official Army term meaning that Tommy is not allowed to trespass where this sign is displayed. He never wished to until the sign made its appearance.</skos:definition>
<skos:inScheme rdf:resource="#OverTheTopDictionary"/>
<rdfs:isDefinedBy rdf:resource="http://rdf.muninn-project.org/ontologies/ott"/>
<rdf:type rdf:resource="http://dbpedia.org/resource/Irony"/>
<vs:term_status>Stable</vs:term_status>
</skos:Concept>
<skos:Concept rdf:ID="Outthere">
<rdfs:label xml:lang="en">Out there</rdfs:label>
<foaf:name>Out there</foaf:name>
<skos:prefLabel xml:lang="en">Out there</skos:prefLabel>
<skos:definition xml:lang="en">A term used in Blighty which means &quot;in France.&quot; Conscientious objectors object to going &quot;out there.&quot;</skos:definition>
<skos:inScheme rdf:resource="#OverTheTopDictionary"/>
<rdfs:isDefinedBy rdf:resource="http://rdf.muninn-project.org/ontologies/ott"/>
<rdf:type rdf:resource="http://dbpedia.org/resource/Irony"/>
<vs:term_status>Stable</vs:term_status>
</skos:Concept>
<skos:Concept rdf:ID="OvertheTop">
<rdfs:label xml:lang="en">Over the Top</rdfs:label>
<foaf:name>Over the Top</foaf:name>
<skos:prefLabel xml:lang="en">Over the Top</skos:prefLabel>
<skos:definition xml:lang="en">A famous phrase of the trenches. It is generally the order for the men to charge the German lines. Nearly always it is accompanied by the Jonah wish, &quot;With the best o&apos; luck and give them hell.&quot;</skos:definition>
<skos:inScheme rdf:resource="#OverTheTopDictionary"/>
<rdfs:isDefinedBy rdf:resource="http://rdf.muninn-project.org/ontologies/ott"/>
<rdf:type rdf:resource="http://dbpedia.org/resource/Irony"/>
<vs:term_status>Stable</vs:term_status>
</skos:Concept>
<skos:Concept rdf:ID="Oxo">
<rdfs:label xml:lang="en">Oxo</rdfs:label>
<foaf:name>Oxo</foaf:name>
<skos:prefLabel xml:lang="en">Oxo</skos:prefLabel>
<skos:definition xml:lang="en">Concentrated beef cubes that a fond mother sends out to Tommy because they are advertised as &quot;British to the Backbone.&quot;</skos:definition>
<skos:inScheme rdf:resource="#OverTheTopDictionary"/>
<rdfs:isDefinedBy rdf:resource="http://rdf.muninn-project.org/ontologies/ott"/>
<rdf:type rdf:resource="http://dbpedia.org/resource/Irony"/>
<vs:term_status>Stable</vs:term_status>
</skos:Concept>
<skos:Concept rdf:ID="Packing">
<rdfs:label xml:lang="en">Packing</rdfs:label>
<foaf:name>Packing</foaf:name>
<skos:prefLabel xml:lang="en">Packing</skos:prefLabel>
<skos:definition xml:lang="en">Asbestos wrapping around the barrel of a machine gun to keep the water from leaking out of the barrel casing. Also slang for rations.</skos:definition>
<skos:inScheme rdf:resource="#OverTheTopDictionary"/>
<rdfs:isDefinedBy rdf:resource="http://rdf.muninn-project.org/ontologies/ott"/>
<rdf:type rdf:resource="http://dbpedia.org/resource/Irony"/>
<vs:term_status>Stable</vs:term_status>
</skos:Concept>
<skos:Concept rdf:ID="PackDrill">
<rdfs:label xml:lang="en">Pack Drill</rdfs:label>
<foaf:name>Pack Drill</foaf:name>
<skos:prefLabel xml:lang="en">Pack Drill</skos:prefLabel>
<skos:definition xml:lang="en">Punishment for a misdemeanor. Sometimes Tommy gets caught when he fills his pack with straw to lighten it for this drill.</skos:definition>
<skos:inScheme rdf:resource="#OverTheTopDictionary"/>
<rdfs:isDefinedBy rdf:resource="http://rdf.muninn-project.org/ontologies/ott"/>
<rdf:type rdf:resource="http://dbpedia.org/resource/Irony"/>
<vs:term_status>Stable</vs:term_status>
</skos:Concept>
<skos:Concept rdf:ID="Parados">
<rdfs:label xml:lang="en">Parados</rdfs:label>
<foaf:name>Parados</foaf:name>
<skos:prefLabel xml:lang="en">Parados</skos:prefLabel>
<skos:definition xml:lang="en">The rear wall of a trench which the Germans continually fill with bits of shell and rifle bullets. Tommy doesn&apos;t mind how many they put in the parados.</skos:definition>
<skos:inScheme rdf:resource="#OverTheTopDictionary"/>
<rdfs:isDefinedBy rdf:resource="http://rdf.muninn-project.org/ontologies/ott"/>
<rdf:type rdf:resource="http://dbpedia.org/resource/Irony"/>
<rdf:type rdf:resource="http://dbpedia.org/resource/Slang"/>
<vs:term_status>Stable</vs:term_status>
</skos:Concept>
<skos:Concept rdf:ID="Parapet">
<rdfs:label xml:lang="en">Parapet</rdfs:label>
<foaf:name>Parapet</foaf:name>
<skos:prefLabel xml:lang="en">Parapet</skos:prefLabel>
<skos:definition xml:lang="en">The top part of a front trench which Tommy constantly builds up and the Germans just as constantly knock down.</skos:definition>
<skos:inScheme rdf:resource="#OverTheTopDictionary"/>
<rdfs:isDefinedBy rdf:resource="http://rdf.muninn-project.org/ontologies/ott"/>
<rdf:type rdf:resource="http://dbpedia.org/resource/Irony"/>
<vs:term_status>Stable</vs:term_status>
</skos:Concept>
<skos:Concept rdf:ID="Patrol">
<rdfs:label xml:lang="en">Patrol</rdfs:label>
<foaf:name>Patrol</foaf:name>
<skos:prefLabel xml:lang="en">Patrol</skos:prefLabel>
<skos:definition xml:lang="en">A few soldiers detailed to go out in &quot;No Man&apos;s Land,&quot; at night and return without any information. Usually these patrols are successful.</skos:definition>
<skos:inScheme rdf:resource="#OverTheTopDictionary"/>
<rdfs:isDefinedBy rdf:resource="http://rdf.muninn-project.org/ontologies/ott"/>
<rdf:type rdf:resource="http://dbpedia.org/resource/Irony"/>
<vs:term_status>Stable</vs:term_status>
</skos:Concept>
<skos:Concept rdf:ID="PayBook">
<rdfs:label xml:lang="en">Pay Book</rdfs:label>
<foaf:name>Pay Book</foaf:name>
<skos:prefLabel xml:lang="en">Pay Book</skos:prefLabel>
<skos:definition xml:lang="en">A little book in which is entered the amount of pay Tommy draws. In the back of same there is also a space for his &quot;will and last testament&quot;; this to remind Tommy that he is liable to be killed. (As if he needed any reminder.)</skos:definition>
<skos:inScheme rdf:resource="#OverTheTopDictionary"/>
<rdfs:isDefinedBy rdf:resource="http://rdf.muninn-project.org/ontologies/ott"/>
<rdf:type rdf:resource="http://dbpedia.org/resource/Irony"/>
<vs:term_status>Stable</vs:term_status>
</skos:Concept>
<skos:Concept rdf:ID="PayParade">
<rdfs:label xml:lang="en">Pay Parade</rdfs:label>
<foaf:name>Pay Parade</foaf:name>
<skos:prefLabel xml:lang="en">Pay Parade</skos:prefLabel>
<skos:definition xml:lang="en">A formation at which Tommy lines up for pay. When his turn comes the paying-officer asks, &quot;How much?&quot; and Tommy answers, &quot;Fifteen francs, sir.&quot; He gets five.</skos:definition>
<skos:inScheme rdf:resource="#OverTheTopDictionary"/>
<rdfs:isDefinedBy rdf:resource="http://rdf.muninn-project.org/ontologies/ott"/>
<rdf:type rdf:resource="http://dbpedia.org/resource/Irony"/>
<vs:term_status>Stable</vs:term_status>
</skos:Concept>
<skos:Concept rdf:ID="Periscope">
<rdfs:label xml:lang="en">Periscope</rdfs:label>
<foaf:name>Periscope</foaf:name>
<skos:prefLabel xml:lang="en">Periscope</skos:prefLabel>
<skos:definition xml:lang="en">A thing in the trenches which you look through. After looking through it, you look over the top to really see something.</skos:definition>
<skos:inScheme rdf:resource="#OverTheTopDictionary"/>
<rdfs:isDefinedBy rdf:resource="http://rdf.muninn-project.org/ontologies/ott"/>
<rdf:type rdf:resource="http://dbpedia.org/resource/Irony"/>
<vs:term_status>Stable</vs:term_status>
</skos:Concept>
<skos:Concept rdf:ID="Physicaltorture">
<rdfs:label xml:lang="en">Physical torture</rdfs:label>
<foaf:name>Physical torture</foaf:name>
<skos:prefLabel xml:lang="en">Physical torture</skos:prefLabel>
<skos:definition xml:lang="en">The nickname for physical training. It is torture, especially to a recruit.</skos:definition>
<skos:inScheme rdf:resource="#OverTheTopDictionary"/>
<rdfs:isDefinedBy rdf:resource="http://rdf.muninn-project.org/ontologies/ott"/>
<rdf:type rdf:resource="http://dbpedia.org/resource/Irony"/>
<vs:term_status>Stable</vs:term_status>
</skos:Concept>
<skos:Concept rdf:ID="Pick">
<rdfs:label xml:lang="en">Pick</rdfs:label>
<foaf:name>Pick</foaf:name>
<skos:prefLabel xml:lang="en">Pick</skos:prefLabel>
<skos:definition xml:lang="en">A tool shaped like an anchor which is being constantly handed to Tommy with the terse command, &quot;get busy.&quot;</skos:definition>
<skos:inScheme rdf:resource="#OverTheTopDictionary"/>
<rdfs:isDefinedBy rdf:resource="http://rdf.muninn-project.org/ontologies/ott"/>
<rdf:type rdf:resource="http://dbpedia.org/resource/Irony"/>
<vs:term_status>Stable</vs:term_status>
</skos:Concept>
<skos:Concept rdf:ID="Pioneer">
<rdfs:label xml:lang="en">Pioneer</rdfs:label>
<foaf:name>Pioneer</foaf:name>
<skos:prefLabel xml:lang="en">Pioneer</skos:prefLabel>
<skos:definition xml:lang="en">A soldier detailed in each company to keep the space around the billets clean. He sleeps all day and only gets busy when an officer comes round. He also sleeps at night.</skos:definition>
<skos:inScheme rdf:resource="#OverTheTopDictionary"/>
<rdfs:isDefinedBy rdf:resource="http://rdf.muninn-project.org/ontologies/ott"/>
<rdf:type rdf:resource="http://dbpedia.org/resource/Irony"/>
<vs:term_status>Stable</vs:term_status>
</skos:Concept>
<skos:Concept rdf:ID="Pipsqueak">
<rdfs:label xml:lang="en">Pip squeak</rdfs:label>
<foaf:name>Pip squeak</foaf:name>
<skos:prefLabel xml:lang="en">Pip squeak</skos:prefLabel>
<skos:definition xml:lang="en">Tommy&apos;s term for a small German shell which makes a &quot;pip&quot; and then a &quot;squeak,&quot; when it comes over.</skos:definition>
<skos:inScheme rdf:resource="#OverTheTopDictionary"/>
<rdfs:isDefinedBy rdf:resource="http://rdf.muninn-project.org/ontologies/ott"/>
<rdf:type rdf:resource="http://dbpedia.org/resource/Irony"/>
<vs:term_status>Stable</vs:term_status>
</skos:Concept>
<skos:Concept rdf:ID="Pontoon">
<rdfs:label xml:lang="en">Pontoon</rdfs:label>
<foaf:name>Pontoon</foaf:name>
<skos:prefLabel xml:lang="en">Pontoon</skos:prefLabel>
<skos:definition xml:lang="en">A card game, in America known as &quot;Black Jack&quot; or &quot;Twenty One.&quot; The banker is the only winner.</skos:definition>
<skos:inScheme rdf:resource="#OverTheTopDictionary"/>
<rdfs:isDefinedBy rdf:resource="http://rdf.muninn-project.org/ontologies/ott"/>
<rdf:type rdf:resource="http://dbpedia.org/resource/Irony"/>
<vs:term_status>Stable</vs:term_status>
</skos:Concept>
<skos:Concept rdf:ID="ProvostSergeant">
<rdfs:label xml:lang="en">Provost-Sergeant</rdfs:label>
<foaf:name>Provost-Sergeant</foaf:name>
<skos:prefLabel xml:lang="en">Provost-Sergeant</skos:prefLabel>
<skos:definition xml:lang="en">A sergeant detailed to oversee prisoners, their work, etc. Each prisoner solemnly swears that when he gets out of &quot;dink&quot; he is going to shoot this sergeant and when he does get out he buys him a drink.</skos:definition>
<skos:inScheme rdf:resource="#OverTheTopDictionary"/>
<rdfs:isDefinedBy rdf:resource="http://rdf.muninn-project.org/ontologies/ott"/>
<rdf:type rdf:resource="http://dbpedia.org/resource/Irony"/>
<vs:term_status>Stable</vs:term_status>
</skos:Concept>
<skos:Concept rdf:ID="PullThrough">
<rdfs:label xml:lang="en">Pull Through</rdfs:label>
<foaf:name>Pull Through</foaf:name>
<skos:prefLabel xml:lang="en">Pull Through</skos:prefLabel>
<skos:definition xml:lang="en">A stout cord with a weight on one end, and a loop on the other for an oily rag. The weighted end is dropped through the bore of the rifle and the rag on the other end is &quot;pulled through.&quot;</skos:definition>
<skos:inScheme rdf:resource="#OverTheTopDictionary"/>
<rdfs:isDefinedBy rdf:resource="http://rdf.muninn-project.org/ontologies/ott"/>
<rdf:type rdf:resource="http://dbpedia.org/resource/Irony"/>
<vs:term_status>Stable</vs:term_status>
</skos:Concept>
<skos:Concept rdf:ID="Pump">
<rdfs:label xml:lang="en">Pump</rdfs:label>
<foaf:name>Pump</foaf:name>
<skos:prefLabel xml:lang="en">Pump</skos:prefLabel>
<skos:definition xml:lang="en">A useless contrivance for emptying the trenches of water. &quot;Useless&quot; because the trenches refuse to be emptied.</skos:definition>
<skos:inScheme rdf:resource="#OverTheTopDictionary"/>
<rdfs:isDefinedBy rdf:resource="http://rdf.muninn-project.org/ontologies/ott"/>
<rdf:type rdf:resource="http://dbpedia.org/resource/Irony"/>
<vs:term_status>Stable</vs:term_status>
</skos:Concept>
<skos:Concept rdf:ID="PushinguptheDaisies">
<rdfs:label xml:lang="en">Pushing up the Daisies</rdfs:label>
<foaf:name>Pushing up the Daisies</foaf:name>
<skos:prefLabel xml:lang="en">Pushing up the Daisies</skos:prefLabel>
<skos:definition xml:lang="en">Tommy&apos;s term for a soldier who has been killed and buried in France.</skos:definition>
<skos:inScheme rdf:resource="#OverTheTopDictionary"/>
<rdfs:isDefinedBy rdf:resource="http://rdf.muninn-project.org/ontologies/ott"/>
<rdf:type rdf:resource="http://dbpedia.org/resource/Irony"/>
<vs:term_status>Stable</vs:term_status>
</skos:Concept>
<skos:Concept rdf:ID="Queer">
<rdfs:label xml:lang="en">Queer</rdfs:label>
<foaf:name>Queer</foaf:name>
<skos:prefLabel xml:lang="en">Queer</skos:prefLabel>
<skos:definition xml:lang="en">Tommy&apos;s term for being sick. The doctor immediately informs him that there is nothing queer about him, and Tommy doesn&apos;t know whether to feel insulted or complimented.</skos:definition>
<skos:inScheme rdf:resource="#OverTheTopDictionary"/>
<rdfs:isDefinedBy rdf:resource="http://rdf.muninn-project.org/ontologies/ott"/>
<rdf:type rdf:resource="http://dbpedia.org/resource/Irony"/>
<vs:term_status>Stable</vs:term_status>
</skos:Concept>
<skos:Concept rdf:ID="Quid">
<rdfs:label xml:lang="en">Quid</rdfs:label>
<foaf:name>Quid</foaf:name>
<skos:prefLabel xml:lang="en">Quid</skos:prefLabel>
<skos:definition xml:lang="en">Tommy&apos;s term for a pound or twenty shillings (about $4.80). He is not on very good terms with this amount as you never see the two together.</skos:definition>
<skos:inScheme rdf:resource="#OverTheTopDictionary"/>
<rdfs:isDefinedBy rdf:resource="http://rdf.muninn-project.org/ontologies/ott"/>
<rdf:type rdf:resource="http://dbpedia.org/resource/Irony"/>
<vs:term_status>Stable</vs:term_status>
</skos:Concept>
<skos:Concept rdf:ID="QuartermasterSergeant">
<rdfs:label xml:lang="en">Quartermaster-Sergeant</rdfs:label>
<muninn:acronym xml:lang="en">Q. M. Sergeant</muninn:acronym>
<foaf:name>Quartermaster-Sergeant</foaf:name>
<skos:prefLabel xml:lang="en">Quartermaster-Sergeant</skos:prefLabel>
<skos:definition xml:lang="en">Quartermaster-Sergeant, or &quot;Quarter&quot; as he is called. A non-commissioned officer in a company who wears three stripes and a crown, and takes charge of the company stores, with the emphasis on the &quot;takes.&quot; In civil life he was a politician or burglar.</skos:definition>
<skos:inScheme rdf:resource="#OverTheTopDictionary"/>
<rdfs:isDefinedBy rdf:resource="http://rdf.muninn-project.org/ontologies/ott"/>
<rdf:type rdf:resource="http://dbpedia.org/resource/Irony"/>
<vs:term_status>Stable</vs:term_status>
</skos:Concept>
<skos:Concept rdf:ID="RangeFinder">
<rdfs:label xml:lang="en">Range Finder</rdfs:label>
<foaf:name>Range Finder</foaf:name>
<skos:prefLabel xml:lang="en">Range Finder</skos:prefLabel>
<skos:definition xml:lang="en">An instrument for ascertaining the distance between two objects, using the instrument as one object. It is very accurate only you get a different result each time you use it, says Tommy.</skos:definition>
<skos:inScheme rdf:resource="#OverTheTopDictionary"/>
<rdfs:isDefinedBy rdf:resource="http://rdf.muninn-project.org/ontologies/ott"/>
<rdf:type rdf:resource="http://dbpedia.org/resource/Irony"/>
<vs:term_status>Stable</vs:term_status>
</skos:Concept>
<skos:Concept rdf:ID="RapidFire">
<rdfs:label xml:lang="en">Rapid Fire</rdfs:label>
<foaf:name>Rapid Fire</foaf:name>
<skos:prefLabel xml:lang="en">Rapid Fire</skos:prefLabel>
<skos:definition xml:lang="en">Means to stick year head &quot;over the top&quot; at night, aim at the moon, and empty your magazine. It there is no moon, aim at the spot where it should be.</skos:definition>
<skos:inScheme rdf:resource="#OverTheTopDictionary"/>
<rdfs:isDefinedBy rdf:resource="http://rdf.muninn-project.org/ontologies/ott"/>
<rdf:type rdf:resource="http://dbpedia.org/resource/Irony"/>
<vs:term_status>Stable</vs:term_status>
</skos:Concept>
<skos:Concept rdf:ID="RationBag">
<rdfs:label xml:lang="en">Ration Bag</rdfs:label>
<foaf:name>Ration Bag</foaf:name>
<skos:prefLabel xml:lang="en">Ration Bag</skos:prefLabel>
<skos:definition xml:lang="en">A small, very small bag for carrying rations. Sometimes it is really useful for lugging souvenirs.</skos:definition>
<skos:inScheme rdf:resource="#OverTheTopDictionary"/>
<rdfs:isDefinedBy rdf:resource="http://rdf.muninn-project.org/ontologies/ott"/>
<rdf:type rdf:resource="http://dbpedia.org/resource/Irony"/>
<vs:term_status>Stable</vs:term_status>
</skos:Concept>
<skos:Concept rdf:ID="Rations">
<rdfs:label xml:lang="en">Rations</rdfs:label>
<foaf:name>Rations</foaf:name>
<skos:prefLabel xml:lang="en">Rations</skos:prefLabel>
<skos:definition xml:lang="en">Various kinds of tasteless food issued by the Government to Tommy, to kid him into thinking that he is living in luxury, while the Germans are starving.</skos:definition>
<skos:inScheme rdf:resource="#OverTheTopDictionary"/>
<rdfs:isDefinedBy rdf:resource="http://rdf.muninn-project.org/ontologies/ott"/>
<rdf:type rdf:resource="http://dbpedia.org/resource/Irony"/>
<vs:term_status>Stable</vs:term_status>
</skos:Concept>
<skos:Concept rdf:ID="RationParty">
<rdfs:label xml:lang="en">Ration Party</rdfs:label>
<foaf:name>Ration Party</foaf:name>
<skos:prefLabel xml:lang="en">Ration Party</skos:prefLabel>
<skos:definition xml:lang="en">Men detailed to carry rations to the front line; pick out a black, cold, and rainy night; put a fifty-pound box on your shoulder; sling your rifle and carry one hundred twenty rounds of ammunition. Then go through a communication trench, with the mud up to your knees, down this trench for a half-mile, and then find your mates swearing in seven different languages; duck a few shells and bullets, and then ask Tommy for his definition of a &quot;ration party.&quot; You will be surprised to learn that it is the same as yours.</skos:definition>
<skos:inScheme rdf:resource="#OverTheTopDictionary"/>
<rdfs:isDefinedBy rdf:resource="http://rdf.muninn-project.org/ontologies/ott"/>
<rdf:type rdf:resource="http://dbpedia.org/resource/Irony"/>
<vs:term_status>Stable</vs:term_status>
</skos:Concept>
<skos:Concept rdf:ID="Rats">
<rdfs:label xml:lang="en">Rats</rdfs:label>
<foaf:name>Rats</foaf:name>
<skos:prefLabel xml:lang="en">Rats</skos:prefLabel>
<skos:definition xml:lang="en">The main inhabitants of the trenches and dugouts. Very useful for chewing up leather equipment and running over your face when asleep. A British rat resembles a bull-dog, while a German one, through a course of Kultur, resembles a dachshund.</skos:definition>
<skos:inScheme rdf:resource="#OverTheTopDictionary"/>
<rdfs:isDefinedBy rdf:resource="http://rdf.muninn-project.org/ontologies/ott"/>
<rdf:type rdf:resource="http://dbpedia.org/resource/Irony"/>
<vs:term_status>Stable</vs:term_status>
</skos:Concept>
<skos:Concept rdf:ID="RedCap">
<rdfs:label xml:lang="en">Red Cap</rdfs:label>
<foaf:name>Red Cap</foaf:name>
<skos:prefLabel xml:lang="en">Red Cap</skos:prefLabel>
<skos:definition xml:lang="en">Tommy&apos;s nickname for a Staff Officer because he wears a red band around his cap.</skos:definition>
<skos:inScheme rdf:resource="#OverTheTopDictionary"/>
<rdfs:isDefinedBy rdf:resource="http://rdf.muninn-project.org/ontologies/ott"/>
<rdf:type rdf:resource="http://dbpedia.org/resource/Irony"/>
<rdf:type rdf:resource="http://dbpedia.org/resource/Slang"/>
<vs:term_status>Stable</vs:term_status>
</skos:Concept>
<skos:Concept rdf:ID="RedTape">
<rdfs:label xml:lang="en">Red Tape</rdfs:label>
<foaf:name>Red Tape</foaf:name>
<skos:prefLabel xml:lang="en">Red Tape</skos:prefLabel>
<skos:definition xml:lang="en">A useless sort of procedure. The main object of this is to prolong the war and give a lot of fat jobs to Army politicians.</skos:definition>
<skos:inScheme rdf:resource="#OverTheTopDictionary"/>
<rdfs:isDefinedBy rdf:resource="http://rdf.muninn-project.org/ontologies/ott"/>
<rdf:type rdf:resource="http://dbpedia.org/resource/Irony"/>
<vs:term_status>Stable</vs:term_status>
</skos:Concept>
<skos:Concept rdf:ID="RegimentalNumber">
<rdfs:label xml:lang="en">Regimental Number</rdfs:label>
<foaf:name>Regimental Number</foaf:name>
<skos:prefLabel xml:lang="en">Regimental Number</skos:prefLabel>
<skos:definition xml:lang="en">Each soldier has a number whether or not he was a convict in civil life. Tommy never forgets his number when he sees it on &quot;orders for leave.&quot;</skos:definition>
<skos:inScheme rdf:resource="#OverTheTopDictionary"/>
<rdfs:isDefinedBy rdf:resource="http://rdf.muninn-project.org/ontologies/ott"/>
<rdf:type rdf:resource="http://dbpedia.org/resource/Irony"/>
<vs:term_status>Stable</vs:term_status>
</skos:Concept>
<skos:Concept rdf:ID="RegimentalPolice">
<rdfs:label xml:lang="en">Regimental Police</rdfs:label>
<muninn:acronym xml:lang="en">R.P.</muninn:acronym>
<foaf:name>Regimental Police</foaf:name>
<skos:prefLabel xml:lang="en">Regimental Police</skos:prefLabel>
<skos:definition xml:lang="en">Men detailed in a Battalion to annoy Tommy and to prevent him from doing what he most desires.</skos:definition>
<skos:inScheme rdf:resource="#OverTheTopDictionary"/>
<rdfs:isDefinedBy rdf:resource="http://rdf.muninn-project.org/ontologies/ott"/>
<rdf:type rdf:resource="http://dbpedia.org/resource/Irony"/>
<vs:term_status>Stable</vs:term_status>
</skos:Concept>
<skos:Concept rdf:ID="Reinforcements">
<rdfs:label xml:lang="en">Reinforcements</rdfs:label>
<foaf:name>Reinforcements</foaf:name>
<skos:prefLabel xml:lang="en">Reinforcements</skos:prefLabel>
<skos:definition xml:lang="en">A lot of new men sent out from England who think that the war will be over a week after they enter the trenches.</skos:definition>
<skos:inScheme rdf:resource="#OverTheTopDictionary"/>
<rdfs:isDefinedBy rdf:resource="http://rdf.muninn-project.org/ontologies/ott"/>
<rdf:type rdf:resource="http://dbpedia.org/resource/Irony"/>
<vs:term_status>Stable</vs:term_status>
</skos:Concept>
<skos:Concept rdf:ID="Relaying">
<rdfs:label xml:lang="en">Relaying</rdfs:label>
<foaf:name>Relaying</foaf:name>
<skos:prefLabel xml:lang="en">Relaying</skos:prefLabel>
<skos:definition xml:lang="en">A term used by the artillery. After a gun is fired it is &quot;relayed &quot; or aimed at something out of sight.</skos:definition>
<skos:inScheme rdf:resource="#OverTheTopDictionary"/>
<rdfs:isDefinedBy rdf:resource="http://rdf.muninn-project.org/ontologies/ott"/>
<rdf:type rdf:resource="http://dbpedia.org/resource/Irony"/>
<vs:term_status>Stable</vs:term_status>
</skos:Concept>
<skos:Concept rdf:ID="Respirator">
<rdfs:label xml:lang="en">Respirator</rdfs:label>
<foaf:name>Respirator</foaf:name>
<skos:prefLabel xml:lang="en">Respirator</skos:prefLabel>
<skos:definition xml:lang="en">A cloth helmet, chemically treated, with glass eye-holes, which Tommy puts over his head as a protection against, poison gas. This helmet never leaves Tommy&apos;s person, he even sleeps with it.</skos:definition>
<skos:inScheme rdf:resource="#OverTheTopDictionary"/>
<rdfs:isDefinedBy rdf:resource="http://rdf.muninn-project.org/ontologies/ott"/>
<rdf:type rdf:resource="http://dbpedia.org/resource/Irony"/>
<vs:term_status>Stable</vs:term_status>
</skos:Concept>
<skos:Concept rdf:ID="Rest">
<rdfs:label xml:lang="en">Rest</rdfs:label>
<foaf:name>Rest</foaf:name>
<skos:prefLabel xml:lang="en">Rest</skos:prefLabel>
<skos:definition xml:lang="en">A period of time for rest allotted to Tommy upon being relieved from the trenches. He uses this &quot;rest&quot; to mend roads, dig trenches, and make himself generally useful while behind the lines.</skos:definition>
<skos:inScheme rdf:resource="#OverTheTopDictionary"/>
<rdfs:isDefinedBy rdf:resource="http://rdf.muninn-project.org/ontologies/ott"/>
<rdf:type rdf:resource="http://dbpedia.org/resource/Irony"/>
<vs:term_status>Stable</vs:term_status>
</skos:Concept>
<skos:Concept rdf:ID="RestBillets">
<rdfs:label xml:lang="en">Rest Billets</rdfs:label>
<foaf:name>Rest Billets</foaf:name>
<skos:prefLabel xml:lang="en">Rest Billets</skos:prefLabel>
<skos:definition xml:lang="en">Shell shattered houses, generally barns, in which Tommy &quot;rests,&quot; when relieved from the firing line.</skos:definition>
<skos:inScheme rdf:resource="#OverTheTopDictionary"/>
<rdfs:isDefinedBy rdf:resource="http://rdf.muninn-project.org/ontologies/ott"/>
<rdf:type rdf:resource="http://dbpedia.org/resource/Irony"/>
<vs:term_status>Stable</vs:term_status>
</skos:Concept>
<skos:Concept rdf:ID="Ricco">
<rdfs:label xml:lang="en">Ricco</rdfs:label>
<foaf:name>Ricco</foaf:name>
<skos:prefLabel xml:lang="en">Ricco</skos:prefLabel>
<skos:definition xml:lang="en">Term for a ricochet bullet. It makes a whining noise and Tommy always ducks when a &quot;ricco&quot; passes him.</skos:definition>
<skos:inScheme rdf:resource="#OverTheTopDictionary"/>
<rdfs:isDefinedBy rdf:resource="http://rdf.muninn-project.org/ontologies/ott"/>
<rdf:type rdf:resource="http://dbpedia.org/resource/Irony"/>
<vs:term_status>Stable</vs:term_status>
<rdf:type rdf:resource="http://dbpedia.org/resource/Slang"/>
</skos:Concept>
<skos:Concept rdf:ID="Rifle">
<rdfs:label xml:lang="en">Rifle</rdfs:label>
<foaf:name>Rifle</foaf:name>
<skos:prefLabel xml:lang="en">Rifle</skos:prefLabel>
<skos:definition xml:lang="en">A part of Tommy&apos;s armament. Its main use is to be cleaned. Sometimes it is fired, when you are not using a pick or shovel. You also &quot;present arms by numbers&quot; with it. This is a very fascinating exercise to Tommy. Ask him.</skos:definition>
<skos:inScheme rdf:resource="#OverTheTopDictionary"/>
<rdfs:isDefinedBy rdf:resource="http://rdf.muninn-project.org/ontologies/ott"/>
<rdf:type rdf:resource="http://dbpedia.org/resource/Irony"/>
<vs:term_status>Stable</vs:term_status>
</skos:Concept>
<skos:Concept rdf:ID="RifleGrenade">
<rdfs:label xml:lang="en">Rifle Grenade</rdfs:label>
<foaf:name>Rifle Grenade</foaf:name>
<skos:prefLabel xml:lang="en">Rifle Grenade</skos:prefLabel>
<skos:definition xml:lang="en">A bomb on the end of a rod. This rod is inserted into the barrel of a specially designed rifle.</skos:definition>
<skos:inScheme rdf:resource="#OverTheTopDictionary"/>
<rdfs:isDefinedBy rdf:resource="http://rdf.muninn-project.org/ontologies/ott"/>
<rdf:type rdf:resource="http://dbpedia.org/resource/Irony"/>
<vs:term_status>Stable</vs:term_status>
</skos:Concept>
<skos:Concept rdf:ID="Requiscatinpace">
<rdfs:label xml:lang="en">Requiscat in pace</rdfs:label>
<muninn:acronym xml:lang="en">R.I.P.</muninn:acronym>
<foaf:name>Requiscat in pace</foaf:name>
<skos:prefLabel xml:lang="en">Requiscat in pace</skos:prefLabel>
<skos:definition xml:lang="en">In monk&apos;s highbrow, &quot;Requiscat in pace,&quot; put on little wooden crosses over soldier&apos;s graves. It means &quot;Rest in peace,&quot; but Tommy says like as not it means &quot;Rest in pieces,&quot; especially if the man under the cross has been sent West by a bomb or shell explosion.</skos:definition>
<skos:inScheme rdf:resource="#OverTheTopDictionary"/>
<rdfs:isDefinedBy rdf:resource="http://rdf.muninn-project.org/ontologies/ott"/>
<rdf:type rdf:resource="http://dbpedia.org/resource/Irony"/>
<vs:term_status>Stable</vs:term_status>
</skos:Concept>
<skos:Concept rdf:ID="RoadDangerousUseTrench">
<rdfs:label xml:lang="en">Road Dangerous, Use Trench</rdfs:label>
<foaf:name>Road Dangerous, Use Trench</foaf:name>
<skos:prefLabel xml:lang="en">Road Dangerous, Use Trench</skos:prefLabel>
<skos:definition xml:lang="en">A familiar sign on roads immediately in rear of the firing line. It is to warn soldiers that it is within sight of Fritz. Tommy never believes these signs and swanks up the road. Later on he tells the Red Cross nurse that the sign told the truth.</skos:definition>
<skos:inScheme rdf:resource="#OverTheTopDictionary"/>
<rdfs:isDefinedBy rdf:resource="http://rdf.muninn-project.org/ontologies/ott"/>
<rdf:type rdf:resource="http://dbpedia.org/resource/Irony"/>
<vs:term_status>Stable</vs:term_status>
</skos:Concept>
<skos:Concept rdf:ID="RollofHonor">
<rdfs:label xml:lang="en">Roll of Honor</rdfs:label>
<foaf:name>Roll of Honor</foaf:name>
<skos:prefLabel xml:lang="en">Roll of Honor</skos:prefLabel>
<skos:definition xml:lang="en">The name given to the published casualty lists of the war. Tommy has no ambition for his name to appear on the &quot;Roll of Honor&quot; unless it comes under the heading &quot;Slightly Wounded.&quot;</skos:definition>
<skos:inScheme rdf:resource="#OverTheTopDictionary"/>
<rdfs:isDefinedBy rdf:resource="http://rdf.muninn-project.org/ontologies/ott"/>
<rdf:type rdf:resource="http://dbpedia.org/resource/Irony"/>
<vs:term_status>Stable</vs:term_status>
</skos:Concept>
<skos:Concept rdf:ID="RomanCatholic">
<rdfs:label xml:lang="en">Roman Catholic</rdfs:label>
<muninn:acronym xml:lang="en">R.C.</muninn:acronym>
<foaf:name>Roman Catholic</foaf:name>
<skos:prefLabel xml:lang="en">Roman Catholic</skos:prefLabel>
<skos:definition xml:lang="en">One of the advantages of being a R.C. is that &quot;Church Parade&quot; is not compulsory.</skos:definition>
<skos:inScheme rdf:resource="#OverTheTopDictionary"/>
<rdfs:isDefinedBy rdf:resource="http://rdf.muninn-project.org/ontologies/ott"/>
<rdf:type rdf:resource="http://dbpedia.org/resource/Irony"/>
<vs:term_status>Stable</vs:term_status>
</skos:Concept>
<skos:Concept rdf:ID="Rooty">
<rdfs:label xml:lang="en">Rooty</rdfs:label>
<foaf:name>Rooty</foaf:name>
<skos:prefLabel xml:lang="en">Rooty</skos:prefLabel>
<skos:definition xml:lang="en">Tommy&apos;s nickname for bread.</skos:definition>
<skos:inScheme rdf:resource="#OverTheTopDictionary"/>
<rdfs:isDefinedBy rdf:resource="http://rdf.muninn-project.org/ontologies/ott"/>
<rdf:type rdf:resource="http://dbpedia.org/resource/Irony"/>
<vs:term_status>Stable</vs:term_status>
<rdf:type rdf:resource="http://dbpedia.org/resource/Slang"/>
</skos:Concept>
<skos:Concept rdf:ID="RouteMarch">
<rdfs:label xml:lang="en">Route March</rdfs:label>
<foaf:name>Route March</foaf:name>
<skos:prefLabel xml:lang="en">Route March</skos:prefLabel>
<skos:definition xml:lang="en">A useless expenditure of leather and energy. These marches teach Tommy to be kind to overloaded beasts of burden.</skos:definition>
<skos:inScheme rdf:resource="#OverTheTopDictionary"/>
<rdfs:isDefinedBy rdf:resource="http://rdf.muninn-project.org/ontologies/ott"/>
<rdf:type rdf:resource="http://dbpedia.org/resource/Irony"/>
<vs:term_status>Stable</vs:term_status>
</skos:Concept>
<skos:Concept rdf:ID="RoyalArmyMedicalCorps">
<rdfs:label xml:lang="en">Royal Army Medical Corps</rdfs:label>
<muninn:acronym xml:lang="en">R.A.M.C.</muninn:acronym>
<foaf:name>Royal Army Medical Corps</foaf:name>
<skos:prefLabel xml:lang="en">Royal Army Medical Corps</skos:prefLabel>
<skos:definition xml:lang="en">Tommy says it means &quot;Rob All My Comrades.&quot;</skos:definition>
<skos:inScheme rdf:resource="#OverTheTopDictionary"/>
<rdfs:isDefinedBy rdf:resource="http://rdf.muninn-project.org/ontologies/ott"/>
<rdf:type rdf:resource="http://dbpedia.org/resource/Irony"/>
<vs:term_status>Stable</vs:term_status>
</skos:Concept>
<skos:Concept rdf:ID="RoyalEngineers">
<rdfs:label xml:lang="en">Royal Engineers</rdfs:label>
<muninn:acronym xml:lang="en">R.E.</muninn:acronym>
<foaf:name>Royal Engineers</foaf:name>
<skos:prefLabel xml:lang="en">Royal Engineers</skos:prefLabel>
<skos:definition xml:lang="en"></skos:definition>
<skos:inScheme rdf:resource="#OverTheTopDictionary"/>
<rdfs:isDefinedBy rdf:resource="http://rdf.muninn-project.org/ontologies/ott"/>
<rdf:type rdf:resource="http://dbpedia.org/resource/Irony"/>
<vs:term_status>Stable</vs:term_status>
</skos:Concept>
<skos:Concept rdf:ID="RoyalFieldArtillery">
<rdfs:label xml:lang="en">Royal Field Artillery</rdfs:label>
<muninn:acronym xml:lang="en">R.F.A.</muninn:acronym>
<foaf:name>Royal Field Artillery</foaf:name>
<skos:prefLabel xml:lang="en">Royal Field Artillery</skos:prefLabel>
<skos:definition xml:lang="en"></skos:definition>
<skos:inScheme rdf:resource="#OverTheTopDictionary"/>
<rdfs:isDefinedBy rdf:resource="http://rdf.muninn-project.org/ontologies/ott"/>
<rdf:type rdf:resource="http://dbpedia.org/resource/Irony"/>
<vs:term_status>Stable</vs:term_status>
</skos:Concept>
<skos:Concept rdf:ID="RoyalPlyingCorps">
<rdfs:label xml:lang="en">Royal Plying Corps</rdfs:label>
<muninn:acronym xml:lang="en">R.F.C.</muninn:acronym>
<foaf:name>Royal Plying Corps</foaf:name>
<skos:prefLabel xml:lang="en">Royal Plying Corps</skos:prefLabel>
<skos:definition xml:lang="en"></skos:definition>
<skos:inScheme rdf:resource="#OverTheTopDictionary"/>
<rdfs:isDefinedBy rdf:resource="http://rdf.muninn-project.org/ontologies/ott"/>
<rdf:type rdf:resource="http://dbpedia.org/resource/Irony"/>
<vs:term_status>Stable</vs:term_status>
</skos:Concept>
<skos:Concept rdf:ID="Rum">
<rdfs:label xml:lang="en">Rum</rdfs:label>
<foaf:name>Rum</foaf:name>
<skos:prefLabel xml:lang="en">Rum</skos:prefLabel>
<skos:definition xml:lang="en">A nectar of the gods issued in the early morning to Tommy.</skos:definition>
<skos:inScheme rdf:resource="#OverTheTopDictionary"/>
<rdfs:isDefinedBy rdf:resource="http://rdf.muninn-project.org/ontologies/ott"/>
<rdf:type rdf:resource="http://dbpedia.org/resource/Irony"/>
<vs:term_status>Stable</vs:term_status>
</skos:Concept>
<skos:Concept rdf:ID="Rumissue">
<rdfs:label xml:lang="en">Rum issue</rdfs:label>
<foaf:name>Rum issue</foaf:name>
<skos:prefLabel xml:lang="en">Rum issue</skos:prefLabel>
<skos:definition xml:lang="en">A daily formation at which Tommy receives a spoonful of rum; that is if any is left over from the Sergeant&apos;s Mess.</skos:definition>
<skos:inScheme rdf:resource="#OverTheTopDictionary"/>
<rdfs:isDefinedBy rdf:resource="http://rdf.muninn-project.org/ontologies/ott"/>
<rdf:type rdf:resource="http://dbpedia.org/resource/Irony"/>
<vs:term_status>Stable</vs:term_status>
</skos:Concept>
<skos:Concept rdf:ID="Runner">
<rdfs:label xml:lang="en">Runner</rdfs:label>
<foaf:name>Runner</foaf:name>
<skos:prefLabel xml:lang="en">Runner</skos:prefLabel>
<skos:definition xml:lang="en">A soldier who is detailed or picked as an orderly for an officer while in the trenches. His real job is to take messages under fire, asking how many tins of jam are required for 1917.</skos:definition>
<skos:inScheme rdf:resource="#OverTheTopDictionary"/>
<rdfs:isDefinedBy rdf:resource="http://rdf.muninn-project.org/ontologies/ott"/>
<rdf:type rdf:resource="http://dbpedia.org/resource/Irony"/>
<vs:term_status>Stable</vs:term_status>
</skos:Concept>
<skos:Concept rdf:ID="SmallArmsAmmunition">
<rdfs:label xml:lang="en">Small Arms Ammunition</rdfs:label>
<muninn:acronym xml:lang="en">S.A.A.</muninn:acronym>
<foaf:name>Small Arms Ammunition</foaf:name>
<skos:prefLabel xml:lang="en">Small Arms Ammunition</skos:prefLabel>
<skos:definition xml:lang="en">Small steel pellets which have a bad habit of drilling holes in the anatomy of Tommy and Fritz.</skos:definition>
<skos:inScheme rdf:resource="#OverTheTopDictionary"/>
<rdfs:isDefinedBy rdf:resource="http://rdf.muninn-project.org/ontologies/ott"/>
<rdf:type rdf:resource="http://dbpedia.org/resource/Irony"/>
<vs:term_status>Stable</vs:term_status>
</skos:Concept>
<skos:Concept rdf:ID="Salvo">
<rdfs:label xml:lang="en">Salvo</rdfs:label>
<foaf:name>Salvo</foaf:name>
<skos:prefLabel xml:lang="en">Salvo</skos:prefLabel>
<skos:definition xml:lang="en">Battery firing four guns simultaneously.</skos:definition>
<skos:inScheme rdf:resource="#OverTheTopDictionary"/>
<rdfs:isDefinedBy rdf:resource="http://rdf.muninn-project.org/ontologies/ott"/>
<rdf:type rdf:resource="http://dbpedia.org/resource/Irony"/>
<vs:term_status>Stable</vs:term_status>
</skos:Concept>
<skos:Concept rdf:ID="Sandbag">
<rdfs:label xml:lang="en">Sandbag</rdfs:label>
<foaf:name>Sandbag</foaf:name>
<skos:prefLabel xml:lang="en">Sandbag</skos:prefLabel>
<skos:definition xml:lang="en">A jute bag which is constantly being filled with earth. Its main uses are to provide Tommy with material for a comfortable kip and to strengthen parapets.</skos:definition>
<skos:inScheme rdf:resource="#OverTheTopDictionary"/>
<rdfs:isDefinedBy rdf:resource="http://rdf.muninn-project.org/ontologies/ott"/>
<rdf:type rdf:resource="http://dbpedia.org/resource/Irony"/>
<vs:term_status>Stable</vs:term_status>
</skos:Concept>
<skos:Concept rdf:ID="Sap">
<rdfs:label xml:lang="en">Sap</rdfs:label>
<foaf:name>Sap</foaf:name>
<skos:prefLabel xml:lang="en">Sap</skos:prefLabel>
<skos:definition xml:lang="en">A small ditch, or trench, dug from the front line and leading out into &quot;No Man&apos;s Land &quot; in the direction of the German trenches.</skos:definition>
<skos:inScheme rdf:resource="#OverTheTopDictionary"/>
<rdfs:isDefinedBy rdf:resource="http://rdf.muninn-project.org/ontologies/ott"/>
<rdf:type rdf:resource="http://dbpedia.org/resource/Irony"/>
<vs:term_status>Stable</vs:term_status>
</skos:Concept>
<skos:Concept rdf:ID="Sapper">
<rdfs:label xml:lang="en">Sapper</rdfs:label>
<foaf:name>Sapper</foaf:name>
<skos:prefLabel xml:lang="en">Sapper</skos:prefLabel>
<skos:definition xml:lang="en">A man who saps or digs mines. He thinks he is thirty-three degrees above an ordinary soldier, while in fact he is generally beneath him.</skos:definition>
<skos:inScheme rdf:resource="#OverTheTopDictionary"/>
<rdfs:isDefinedBy rdf:resource="http://rdf.muninn-project.org/ontologies/ott"/>
<rdf:type rdf:resource="http://dbpedia.org/resource/Irony"/>
<vs:term_status>Stable</vs:term_status>
</skos:Concept>
<skos:Concept rdf:ID="StretcherBearer">
<rdfs:label xml:lang="en">Stretcher Bearer</rdfs:label>
<muninn:acronym xml:lang="en">S.B.</muninn:acronym>
<foaf:name>Stretcher Bearer</foaf:name>
<skos:prefLabel xml:lang="en">Stretcher Bearer</skos:prefLabel>
<skos:definition xml:lang="en">The motive power of a stretcher. He is generally looking the other way when a fourteen-stone Tommy gets hit.</skos:definition>
<skos:inScheme rdf:resource="#OverTheTopDictionary"/>
<rdfs:isDefinedBy rdf:resource="http://rdf.muninn-project.org/ontologies/ott"/>
<rdf:type rdf:resource="http://dbpedia.org/resource/Irony"/>
<vs:term_status>Stable</vs:term_status>
</skos:Concept>
<skos:Concept rdf:ID="Scalingladder">
<rdfs:label xml:lang="en">Scaling ladder</rdfs:label>
<foaf:name>Scaling ladder</foaf:name>
<skos:prefLabel xml:lang="en">Scaling ladder</skos:prefLabel>
<skos:definition xml:lang="en">Small wooden ladders used by Tommy for climbing out of the front trench when he goes &quot;over the top.&quot; When Tommy sees these ladders being brought into the trench, he sits down and writes his will in his little pay-book.</skos:definition>
<skos:inScheme rdf:resource="#OverTheTopDictionary"/>
<rdfs:isDefinedBy rdf:resource="http://rdf.muninn-project.org/ontologies/ott"/>
<rdf:type rdf:resource="http://dbpedia.org/resource/Irony"/>
<vs:term_status>Stable</vs:term_status>
</skos:Concept>
<skos:Concept rdf:ID="SentryGo">
<rdfs:label xml:lang="en">Sentry Go</rdfs:label>
<foaf:name>Sentry Go</foaf:name>
<skos:prefLabel xml:lang="en">Sentry Go</skos:prefLabel>
<skos:definition xml:lang="en">Time on guard. It means &quot;sentry come.&quot;</skos:definition>
<skos:inScheme rdf:resource="#OverTheTopDictionary"/>
<rdfs:isDefinedBy rdf:resource="http://rdf.muninn-project.org/ontologies/ott"/>
<rdf:type rdf:resource="http://dbpedia.org/resource/Irony"/>
<vs:term_status>Stable</vs:term_status>
</skos:Concept>
<skos:Concept rdf:ID="SergeantMess">
<rdfs:label xml:lang="en">Sergeant&apos;s Mess</rdfs:label>
<foaf:name>Sergeant&apos;s Mess</foaf:name>
<skos:prefLabel xml:lang="en">Sergeant&apos;s Mess</skos:prefLabel>
<skos:definition xml:lang="en">Where the sergeants eat. Nearly all of the rum has a habit of disappearing into the Sergeant&apos;s Mess.</skos:definition>
<skos:inScheme rdf:resource="#OverTheTopDictionary"/>
<rdfs:isDefinedBy rdf:resource="http://rdf.muninn-project.org/ontologies/ott"/>
<rdf:type rdf:resource="http://dbpedia.org/resource/Irony"/>
<vs:term_status>Stable</vs:term_status>
</skos:Concept>
<skos:Concept rdf:ID="SeventyFives">
<rdfs:label xml:lang="en">Seventy-fives</rdfs:label>
<foaf:name>Seventy-fives</foaf:name>
<skos:prefLabel xml:lang="en">Seventy-fives</skos:prefLabel>
<skos:definition xml:lang="en">A very efficient field-gun of the French, which can fire thirty shells per minute. The gun needs no relaying due to the recoil which throws the him back to its original position. The gun that knocked out &quot;Jack Johnson,&quot; therefore called &quot;Jess Willard.&quot;</skos:definition>
<skos:inScheme rdf:resource="#OverTheTopDictionary"/>
<rdfs:isDefinedBy rdf:resource="http://rdf.muninn-project.org/ontologies/ott"/>
<rdf:type rdf:resource="http://dbpedia.org/resource/Irony"/>
<vs:term_status>Stable</vs:term_status>
</skos:Concept>
<skos:Concept rdf:ID="Sewedinablanket">
<rdfs:label xml:lang="en">Sewed in a blanket</rdfs:label>
<foaf:name>Sewed in a blanket</foaf:name>
<skos:prefLabel xml:lang="en">Sewed in a blanket</skos:prefLabel>
<skos:definition xml:lang="en">Term for a soldier who has been buried. His remains are generally sewn in a blanket and the piece of blanket is generally deducted from his pay that is due.</skos:definition>
<skos:inScheme rdf:resource="#OverTheTopDictionary"/>
<rdfs:isDefinedBy rdf:resource="http://rdf.muninn-project.org/ontologies/ott"/>
<rdf:type rdf:resource="http://dbpedia.org/resource/Irony"/>
<vs:term_status>Stable</vs:term_status>
<rdf:type rdf:resource="http://dbpedia.org/resource/Slang"/>
</skos:Concept>
<skos:Concept rdf:ID="Shag">
<rdfs:label xml:lang="en">Shag</rdfs:label>
<foaf:name>Shag</foaf:name>
<skos:prefLabel xml:lang="en">Shag</skos:prefLabel>
<skos:definition xml:lang="en">Cigarette tobacco which an American can never learn to use. Even the mules object to the smell of it.</skos:definition>
<skos:inScheme rdf:resource="#OverTheTopDictionary"/>
<rdfs:isDefinedBy rdf:resource="http://rdf.muninn-project.org/ontologies/ott"/>
<rdf:type rdf:resource="http://dbpedia.org/resource/Irony"/>
<vs:term_status>Stable</vs:term_status>
<rdf:type rdf:resource="http://dbpedia.org/resource/Slang"/>
</skos:Concept>
<skos:Concept rdf:ID="Shell">
<rdfs:label xml:lang="en">Shell</rdfs:label>
<foaf:name>Shell</foaf:name>
<skos:prefLabel xml:lang="en">Shell</skos:prefLabel>
<skos:definition xml:lang="en">A device of the artillery which sometimes makes Tommy wish he had been born in a neutral country.</skos:definition>
<skos:inScheme rdf:resource="#OverTheTopDictionary"/>
<rdfs:isDefinedBy rdf:resource="http://rdf.muninn-project.org/ontologies/ott"/>
<rdf:type rdf:resource="http://dbpedia.org/resource/Irony"/>
<vs:term_status>Stable</vs:term_status>
</skos:Concept>
<skos:Concept rdf:ID="ShellHole">
<rdfs:label xml:lang="en">Shell Hole</rdfs:label>
<foaf:name>Shell Hole</foaf:name>
<skos:prefLabel xml:lang="en">Shell Hole</skos:prefLabel>
<skos:definition xml:lang="en">A hole in the ground caused by the explosion of a shell. Tommy&apos;s favorite resting-place while under fire.</skos:definition>
<skos:inScheme rdf:resource="#OverTheTopDictionary"/>
<rdfs:isDefinedBy rdf:resource="http://rdf.muninn-project.org/ontologies/ott"/>
<rdf:type rdf:resource="http://dbpedia.org/resource/Irony"/>
<vs:term_status>Stable</vs:term_status>
</skos:Concept>
<skos:Concept rdf:ID="Shovel">
<rdfs:label xml:lang="en">Shovel</rdfs:label>
<foaf:name>Shovel</foaf:name>
<skos:prefLabel xml:lang="en">Shovel</skos:prefLabel>
<skos:definition xml:lang="en">A tool closely related to the pick family. In France the &quot;shovel&quot; is mightier than the sword.</skos:definition>
<skos:inScheme rdf:resource="#OverTheTopDictionary"/>
<rdfs:isDefinedBy rdf:resource="http://rdf.muninn-project.org/ontologies/ott"/>
<rdf:type rdf:resource="http://dbpedia.org/resource/Irony"/>
<vs:term_status>Stable</vs:term_status>
</skos:Concept>
<skos:Concept rdf:ID="Shrapnel">
<rdfs:label xml:lang="en">Shrapnel</rdfs:label>
<foaf:name>Shrapnel</foaf:name>
<skos:prefLabel xml:lang="en">Shrapnel</skos:prefLabel>
<skos:definition xml:lang="en">A shell which bursts in the air and scatters small pieces of metal over a large area. It is used to test the resisting power of steel helmets.</skos:definition>
<skos:inScheme rdf:resource="#OverTheTopDictionary"/>
<rdfs:isDefinedBy rdf:resource="http://rdf.muninn-project.org/ontologies/ott"/>
<rdf:type rdf:resource="http://dbpedia.org/resource/Irony"/>
<vs:term_status>Stable</vs:term_status>
</skos:Concept>
<skos:Concept rdf:ID="Sicker">
<rdfs:label xml:lang="en">Sicker</rdfs:label>
<foaf:name>Sicker</foaf:name>
<skos:prefLabel xml:lang="en">Sicker</skos:prefLabel>
<skos:definition xml:lang="en">Nickname for the sick report book. It is Tommy&apos;s ambition to get on this &quot;sicker&quot; without feeling sick.</skos:definition>
<skos:inScheme rdf:resource="#OverTheTopDictionary"/>
<rdfs:isDefinedBy rdf:resource="http://rdf.muninn-project.org/ontologies/ott"/>
<rdf:type rdf:resource="http://dbpedia.org/resource/Irony"/>
<rdf:type rdf:resource="http://dbpedia.org/resource/Slang"/>
<vs:term_status>Stable</vs:term_status>
</skos:Concept>
<skos:Concept rdf:ID="SideParade">
<rdfs:label xml:lang="en">Side Parade</rdfs:label>
<foaf:name>Side Parade</foaf:name>
<skos:prefLabel xml:lang="en">Side Parade</skos:prefLabel>
<skos:definition xml:lang="en">A formation at which the doctor informs sick, or would-be sick Tommies that they are not sick.</skos:definition>
<skos:inScheme rdf:resource="#OverTheTopDictionary"/>
<rdfs:isDefinedBy rdf:resource="http://rdf.muninn-project.org/ontologies/ott"/>
<rdf:type rdf:resource="http://dbpedia.org/resource/Irony"/>
<vs:term_status>Stable</vs:term_status>
</skos:Concept>
<skos:Concept rdf:ID="SixtyPounder">
<rdfs:label xml:lang="en">Sixty-pounder</rdfs:label>
<foaf:name>Sixty-pounder</foaf:name>
<skos:prefLabel xml:lang="en">Sixty-pounder</skos:prefLabel>
<skos:definition xml:lang="en">One of our shells which weighs sixty pounds (officially). When Tommy handles them, their unofficial weight is three hundred weight.</skos:definition>
<skos:inScheme rdf:resource="#OverTheTopDictionary"/>
<rdfs:isDefinedBy rdf:resource="http://rdf.muninn-project.org/ontologies/ott"/>
<rdf:type rdf:resource="http://dbpedia.org/resource/Irony"/>
<vs:term_status>Stable</vs:term_status>
</skos:Concept>
<skos:Concept rdf:ID="Slacker">
<rdfs:label xml:lang="en">Slacker</rdfs:label>
<foaf:name>Slacker</foaf:name>
<skos:prefLabel xml:lang="en">Slacker</skos:prefLabel>
<skos:definition xml:lang="en">An insect in England who is afraid to join the Army. There are three things in this world that Tommy hates: a slacker, a German; and a trench-rat; it&apos;s hard to tell which he hates worst.</skos:definition>
<skos:inScheme rdf:resource="#OverTheTopDictionary"/>
<rdf:type rdf:resource="http://dbpedia.org/resource/Slang"/>
<rdfs:isDefinedBy rdf:resource="http://rdf.muninn-project.org/ontologies/ott"/>
<rdf:type rdf:resource="http://dbpedia.org/resource/Irony"/>
<rdf:type rdf:resource="http://dbpedia.org/resource/Derogatory"/>
<vs:term_status>Stable</vs:term_status>
</skos:Concept>
<skos:Concept rdf:ID="SlagHeap">
<rdfs:label xml:lang="en">Slag Heap</rdfs:label>
<foaf:name>Slag Heap</foaf:name>
<skos:prefLabel xml:lang="en">Slag Heap</skos:prefLabel>
<skos:definition xml:lang="en">A pile of rubbish, tin cans, etc.</skos:definition>
<skos:inScheme rdf:resource="#OverTheTopDictionary"/>
<rdf:type rdf:resource="http://dbpedia.org/resource/Slang"/>
<rdfs:isDefinedBy rdf:resource="http://rdf.muninn-project.org/ontologies/ott"/>
<rdf:type rdf:resource="http://dbpedia.org/resource/Irony"/>
<vs:term_status>Stable</vs:term_status>
</skos:Concept>
<skos:Concept rdf:ID="SmokeBomb">
<rdfs:label xml:lang="en">Smoke Bomb</rdfs:label>
<foaf:name>Smoke Bomb</foaf:name>
<skos:prefLabel xml:lang="en">Smoke Bomb</skos:prefLabel>
<skos:definition xml:lang="en">A shell which, in exploding, emits a dense white smoke, hiding the operations of troops. When Tommy, in attacking a trench, gets into this smoke, he imagines himself a magnet and thinks all the machine guns and rifles are firing at him alone.</skos:definition>
<skos:inScheme rdf:resource="#OverTheTopDictionary"/>
<rdfs:isDefinedBy rdf:resource="http://rdf.muninn-project.org/ontologies/ott"/>
<rdf:type rdf:resource="http://dbpedia.org/resource/Irony"/>
<vs:term_status>Stable</vs:term_status>
</skos:Concept>
<skos:Concept rdf:ID="Sniper">
<rdfs:label xml:lang="en">Sniper</rdfs:label>
<foaf:name>Sniper</foaf:name>
<skos:prefLabel xml:lang="en">Sniper</skos:prefLabel>
<skos:definition xml:lang="en">A good shot whose main occupation is picking off unwary individuals of the enemy. In the long run a sniper usually gets &quot;sniped.&quot;</skos:definition>
<skos:inScheme rdf:resource="#OverTheTopDictionary"/>
<rdfs:isDefinedBy rdf:resource="http://rdf.muninn-project.org/ontologies/ott"/>
<rdf:type rdf:resource="http://dbpedia.org/resource/Irony"/>
<vs:term_status>Stable</vs:term_status>
</skos:Concept>
<skos:Concept rdf:ID="SnipeHole">
<rdfs:label xml:lang="en">Snipe Hole</rdfs:label>
<foaf:name>Snipe Hole</foaf:name>
<skos:prefLabel xml:lang="en">Snipe Hole</skos:prefLabel>
<skos:definition xml:lang="en">A hole in a steel plate through which snipers &quot;snipe.&quot; It is not fair for the enemy to shoot at these holes, but they do, and often hit them, or at least the man behind them.</skos:definition>
<skos:inScheme rdf:resource="#OverTheTopDictionary"/>
<rdfs:isDefinedBy rdf:resource="http://rdf.muninn-project.org/ontologies/ott"/>
<rdf:type rdf:resource="http://dbpedia.org/resource/Irony"/>
<vs:term_status>Stable</vs:term_status>
</skos:Concept>
<skos:Concept rdf:ID="SoldiersFriend">
<rdfs:label xml:lang="en">Soldiers&apos; Friend</rdfs:label>
<foaf:name>Soldiers&apos; Friend</foaf:name>
<skos:prefLabel xml:lang="en">Soldiers&apos; Friend</skos:prefLabel>
<skos:definition xml:lang="en">Metal polish costing three ha&apos; pence which Tommy uses to polish his buttons. Tommy wonders why it is called &quot;Soldiers&apos; Friend.&quot;</skos:definition>
<skos:inScheme rdf:resource="#OverTheTopDictionary"/>
<rdfs:isDefinedBy rdf:resource="http://rdf.muninn-project.org/ontologies/ott"/>
<rdf:type rdf:resource="http://dbpedia.org/resource/Irony"/>
<rdf:type rdf:resource="http://dbpedia.org/resource/Slang"/>
<vs:term_status>Stable</vs:term_status>
</skos:Concept>
<skos:Concept rdf:ID="SomewhereinFrance">
<rdfs:label xml:lang="en">Somewhere in France</rdfs:label>
<foaf:name>Somewhere in France</foaf:name>
<skos:prefLabel xml:lang="en">Somewhere in France</skos:prefLabel>
<skos:definition xml:lang="en">A certain spot in France where Tommy has to live in mud, hunt for &quot;cooties,&quot; and duck shells and bullets. Tommy&apos;s official address.</skos:definition>
<skos:inScheme rdf:resource="#OverTheTopDictionary"/>
<rdfs:isDefinedBy rdf:resource="http://rdf.muninn-project.org/ontologies/ott"/>
<rdf:type rdf:resource="http://dbpedia.org/resource/Irony"/>
<vs:term_status>Stable</vs:term_status>
</skos:Concept>
<skos:Concept rdf:ID="Spy">
<rdfs:label xml:lang="en">Spy</rdfs:label>
<foaf:name>Spy</foaf:name>
<skos:prefLabel xml:lang="en">Spy</skos:prefLabel>
<skos:definition xml:lang="en">A suspicious person whom no one suspects until he is caught. Then all say they knew he was a spy but had no chance to report it to the proper authorities.</skos:definition>
<skos:inScheme rdf:resource="#OverTheTopDictionary"/>
<rdfs:isDefinedBy rdf:resource="http://rdf.muninn-project.org/ontologies/ott"/>
<rdf:type rdf:resource="http://dbpedia.org/resource/Irony"/>
<vs:term_status>Stable</vs:term_status>
</skos:Concept>
<skos:Concept rdf:ID="Spud">
<rdfs:label xml:lang="en">Spud</rdfs:label>
<foaf:name>Spud</foaf:name>
<skos:prefLabel xml:lang="en">Spud</skos:prefLabel>
<skos:definition xml:lang="en">Tommy&apos;s name for the solitary potato which gets into the stew. It&apos;s a great mystery how that lonely little spud got into such bad company.</skos:definition>
<skos:inScheme rdf:resource="#OverTheTopDictionary"/>
<rdfs:isDefinedBy rdf:resource="http://rdf.muninn-project.org/ontologies/ott"/>
<rdf:type rdf:resource="http://dbpedia.org/resource/Irony"/>
<rdf:type rdf:resource="http://dbpedia.org/resource/Slang"/>
<vs:term_status>Stable</vs:term_status>
</skos:Concept>
<skos:Concept rdf:ID="StandTo">
<rdfs:label xml:lang="en">Stand To</rdfs:label>
<foaf:name>Stand To</foaf:name>
<skos:prefLabel xml:lang="en">Stand To</skos:prefLabel>
<skos:definition xml:lang="en">Order to mount the fire step. Given just as it begins to grow dark.</skos:definition>
<skos:inScheme rdf:resource="#OverTheTopDictionary"/>
<rdfs:isDefinedBy rdf:resource="http://rdf.muninn-project.org/ontologies/ott"/>
<rdf:type rdf:resource="http://dbpedia.org/resource/Slang"/>
<rdf:type rdf:resource="http://dbpedia.org/resource/Irony"/>
<vs:term_status>Stable</vs:term_status>
</skos:Concept>
<skos:Concept rdf:ID="StandDown">
<rdfs:label xml:lang="en">Stand Down</rdfs:label>
<foaf:name>Stand Down</foaf:name>
<skos:prefLabel xml:lang="en">Stand Down</skos:prefLabel>
<skos:definition xml:lang="en">Order given in the trenches at break of dawn to let the men know their night watch is ended. It has a pleasant sound in Tommy&apos;s ears.</skos:definition>
<skos:inScheme rdf:resource="#OverTheTopDictionary"/>
<rdf:type rdf:resource="http://dbpedia.org/resource/Slang"/>
<rdfs:isDefinedBy rdf:resource="http://rdf.muninn-project.org/ontologies/ott"/>
<rdf:type rdf:resource="http://dbpedia.org/resource/Irony"/>
<vs:term_status>Stable</vs:term_status>
</skos:Concept>
<skos:Concept rdf:ID="SteelHelmet">
<rdfs:label xml:lang="en">Steel Helmet</rdfs:label>
<foaf:name>Steel Helmet</foaf:name>
<skos:prefLabel xml:lang="en">Steel Helmet</skos:prefLabel>
<skos:definition xml:lang="en">A round hat made out of steel which is supposed to be shrapnel proof. It is until a piece of shell goes through it, then Tommy loses interest as to whether it is shrapnel proof or not. He calls it a &quot;tin hat.&quot;</skos:definition>
<skos:inScheme rdf:resource="#OverTheTopDictionary"/>
<rdfs:isDefinedBy rdf:resource="http://rdf.muninn-project.org/ontologies/ott"/>
<rdf:type rdf:resource="http://dbpedia.org/resource/Irony"/>
<vs:term_status>Stable</vs:term_status>
</skos:Concept>
<skos:Concept rdf:ID="Stew">
<rdfs:label xml:lang="en">Stew</rdfs:label>
<foaf:name>Stew</foaf:name>
<skos:prefLabel xml:lang="en">Stew</skos:prefLabel>
<skos:definition xml:lang="en">A concoction of the cook&apos;s which contains bully beef, Maconochie rations, water, a few lumps of fresh meat, and a potato. Occasionally a little salt falls into it by mistake. Tommy is supposed to eat this mess -- he does -- worse luck!</skos:definition>
<skos:inScheme rdf:resource="#OverTheTopDictionary"/>
<rdfs:isDefinedBy rdf:resource="http://rdf.muninn-project.org/ontologies/ott"/>
<rdf:type rdf:resource="http://dbpedia.org/resource/Irony"/>
<vs:term_status>Stable</vs:term_status>
</skos:Concept>
<skos:Concept rdf:ID="Strafeing">
<rdfs:label xml:lang="en">Strafeing</rdfs:label>
<foaf:name>Strafeing</foaf:name>
<skos:prefLabel xml:lang="en">Strafeing</skos:prefLabel>
<skos:definition xml:lang="en">Tommy&apos;s chief sport -- shelling the Germans. Taken from Fritz&apos;s own dictionary.</skos:definition>
<skos:inScheme rdf:resource="#OverTheTopDictionary"/>
<rdfs:isDefinedBy rdf:resource="http://rdf.muninn-project.org/ontologies/ott"/>
<rdf:type rdf:resource="http://dbpedia.org/resource/Irony"/>
<vs:term_status>Stable</vs:term_status>
</skos:Concept>
<skos:Concept rdf:ID="Stretcher">
<rdfs:label xml:lang="en">Stretcher</rdfs:label>
<foaf:name>Stretcher</foaf:name>
<skos:prefLabel xml:lang="en">Stretcher</skos:prefLabel>
<skos:definition xml:lang="en">A contrivance on which dead and wounded are carried. The only time Tommy gets a free ride in the trenches is while on a stretcher. As a rule he does not appreciate this means of transportation.</skos:definition>
<skos:inScheme rdf:resource="#OverTheTopDictionary"/>
<rdfs:isDefinedBy rdf:resource="http://rdf.muninn-project.org/ontologies/ott"/>
<rdf:type rdf:resource="http://dbpedia.org/resource/Irony"/>
<vs:term_status>Stable</vs:term_status>
</skos:Concept>
<skos:Concept rdf:ID="SuicideClub">
<rdfs:label xml:lang="en">Suicide Club</rdfs:label>
<foaf:name>Suicide Club</foaf:name>
<skos:prefLabel xml:lang="en">Suicide Club</skos:prefLabel>
<skos:definition xml:lang="en">Nickname for bombers and machine gunners. (No misnomer.)</skos:definition>
<skos:inScheme rdf:resource="#OverTheTopDictionary"/>
<rdfs:isDefinedBy rdf:resource="http://rdf.muninn-project.org/ontologies/ott"/>
<rdf:type rdf:resource="http://dbpedia.org/resource/Irony"/>
<vs:term_status>Stable</vs:term_status>
</skos:Concept>
<skos:Concept rdf:ID="Supper">
<rdfs:label xml:lang="en">Supper</rdfs:label>
<foaf:name>Supper</foaf:name>
<skos:prefLabel xml:lang="en">Supper</skos:prefLabel>
<skos:definition xml:lang="en">Tommy&apos;s fourth meal, generally eaten just before &quot;lights out.&quot; It is composed of the remains of the day&apos;s rations. There are a lot of Tommies who never eat supper. There is a reason.</skos:definition>
<skos:inScheme rdf:resource="#OverTheTopDictionary"/>
<rdfs:isDefinedBy rdf:resource="http://rdf.muninn-project.org/ontologies/ott"/>
<rdf:type rdf:resource="http://dbpedia.org/resource/Irony"/>
<vs:term_status>Stable</vs:term_status>
</skos:Concept>
<skos:Concept rdf:ID="Shellwound">
<rdfs:label xml:lang="en">Shell wound</rdfs:label>
<muninn:acronym xml:lang="en">S.W.</muninn:acronym>
<foaf:name>Shell wound</foaf:name>
<skos:prefLabel xml:lang="en">Shell wound</skos:prefLabel>
<skos:definition xml:lang="en">What the doctor marks on your hospital chart when a shell has removed your leg.</skos:definition>
<skos:inScheme rdf:resource="#OverTheTopDictionary"/>
<rdfs:isDefinedBy rdf:resource="http://rdf.muninn-project.org/ontologies/ott"/>
<rdf:type rdf:resource="http://dbpedia.org/resource/Irony"/>
<vs:term_status>Stable</vs:term_status>
</skos:Concept>
<skos:Concept rdf:ID="Swamping">
<rdfs:label xml:lang="en">Swamping</rdfs:label>
<foaf:name>Swamping</foaf:name>
<skos:prefLabel xml:lang="en">Swamping</skos:prefLabel>
<skos:definition xml:lang="en">Putting on airs; showing off. Generally accredited to Yankees.</skos:definition>
<skos:inScheme rdf:resource="#OverTheTopDictionary"/>
<rdfs:isDefinedBy rdf:resource="http://rdf.muninn-project.org/ontologies/ott"/>
<rdf:type rdf:resource="http://dbpedia.org/resource/Irony"/>
<rdf:type rdf:resource="http://dbpedia.org/resource/Slang"/>
<vs:term_status>Stable</vs:term_status>
</skos:Concept>
<skos:Concept rdf:ID="Swingingthelead">
<rdfs:label xml:lang="en">Swinging the lead</rdfs:label>
<foaf:name>Swinging the lead</foaf:name>
<skos:prefLabel xml:lang="en">Swinging the lead</skos:prefLabel>
<skos:definition xml:lang="en">Throwing the bull.</skos:definition>
<skos:inScheme rdf:resource="#OverTheTopDictionary"/>
<rdfs:isDefinedBy rdf:resource="http://rdf.muninn-project.org/ontologies/ott"/>
<rdf:type rdf:resource="http://dbpedia.org/resource/Irony"/>
<vs:term_status>Stable</vs:term_status>
</skos:Concept>
<skos:Concept rdf:ID="Sweatingonleave">
<rdfs:label xml:lang="en">Sweating on leave</rdfs:label>
<foaf:name>Sweating on leave</foaf:name>
<skos:prefLabel xml:lang="en">Sweating on leave</skos:prefLabel>
<skos:definition xml:lang="en">Impatiently waiting for your name to appear in orders for leave. If Tommy sweats very long he generally catches cold and when leave comes he is too sick to go.</skos:definition>
<skos:inScheme rdf:resource="#OverTheTopDictionary"/>
<rdfs:isDefinedBy rdf:resource="http://rdf.muninn-project.org/ontologies/ott"/>
<rdf:type rdf:resource="http://dbpedia.org/resource/Irony"/>
<rdf:type rdf:resource="http://dbpedia.org/resource/Slang"/>
<vs:term_status>Stable</vs:term_status>
</skos:Concept>
<skos:Concept rdf:ID="Takingover">
<rdfs:label xml:lang="en">Taking over</rdfs:label>
<foaf:name>Taking over</foaf:name>
<skos:prefLabel xml:lang="en">Taking over</skos:prefLabel>
<skos:definition xml:lang="en">Going into a trench. Tommy &quot;takes over,&quot; is &quot;taken out&quot; and sometimes is &quot;put under.&quot;</skos:definition>
<skos:inScheme rdf:resource="#OverTheTopDictionary"/>
<rdfs:isDefinedBy rdf:resource="http://rdf.muninn-project.org/ontologies/ott"/>
<rdf:type rdf:resource="http://dbpedia.org/resource/Irony"/>
<vs:term_status>Stable</vs:term_status>
</skos:Concept>
<skos:Concept rdf:ID="Taube">
<rdfs:label xml:lang="en">Taube</rdfs:label>
<foaf:name>Taube</foaf:name>
<skos:prefLabel xml:lang="en">Taube</skos:prefLabel>
<skos:definition xml:lang="en">A type of German aeroplane whose special ambition is beating the altitude record. It occasionally loses its way and flies over the British lines and then stops flying.</skos:definition>
<skos:inScheme rdf:resource="#OverTheTopDictionary"/>
<rdfs:isDefinedBy rdf:resource="http://rdf.muninn-project.org/ontologies/ott"/>
<rdf:type rdf:resource="http://dbpedia.org/resource/Irony"/>
<vs:term_status>Stable</vs:term_status>
</skos:Concept>
<skos:Concept rdf:ID="Tea">
<rdfs:label xml:lang="en">Tea</rdfs:label>
<foaf:name>Tea</foaf:name>
<skos:prefLabel xml:lang="en">Tea</skos:prefLabel>
<skos:definition xml:lang="en">A dark brown drug, which Tommy has to have at certain periods of the day. Battles have been known to have been stopped to enable Tommy to get his tea, or &quot;char&quot; as it is commonly called.</skos:definition>
<rdf:type rdf:resource="http://dbpedia.org/resource/Slang"/>
<skos:inScheme rdf:resource="#OverTheTopDictionary"/>
<rdfs:isDefinedBy rdf:resource="http://rdf.muninn-project.org/ontologies/ott"/>
<rdf:type rdf:resource="http://dbpedia.org/resource/Irony"/>
<vs:term_status>Stable</vs:term_status>
</skos:Concept>
<skos:Concept rdf:ID="TearShell">
<rdfs:label xml:lang="en">Tear Shell</rdfs:label>
<foaf:name>Tear Shell</foaf:name>
<skos:prefLabel xml:lang="en">Tear Shell</skos:prefLabel>
<skos:definition xml:lang="en">Trench name for the German lachrymose chemical shell which makes the eyes smart. The only time Tommy is outwardly sentimental.</skos:definition>
<skos:inScheme rdf:resource="#OverTheTopDictionary"/>
<rdfs:isDefinedBy rdf:resource="http://rdf.muninn-project.org/ontologies/ott"/>
<rdf:type rdf:resource="http://dbpedia.org/resource/Irony"/>
<rdf:type rdf:resource="http://dbpedia.org/resource/Slang"/>
<vs:term_status>Stable</vs:term_status>
</skos:Concept>
<skos:Concept rdf:ID="Telephone">
<rdfs:label xml:lang="en">Telephone</rdfs:label>
<foaf:name>Telephone</foaf:name>
<skos:prefLabel xml:lang="en">Telephone</skos:prefLabel>
<skos:definition xml:lang="en">A little instrument with a wire attached to it. An artillery observer whispers something into this instrument and immediately one of your batteries behind the line opens up and drops a few shells into your front trench. This keeps up until the observer whispers, &quot;Your range is too short.&quot; Then the shells drop nearer the German lines.</skos:definition>
<skos:inScheme rdf:resource="#OverTheTopDictionary"/>
<rdfs:isDefinedBy rdf:resource="http://rdf.muninn-project.org/ontologies/ott"/>
<rdf:type rdf:resource="http://dbpedia.org/resource/Irony"/>
<vs:term_status>Stable</vs:term_status>
</skos:Concept>
<skos:Concept rdf:ID="Terrier">
<rdfs:label xml:lang="en">Terrier</rdfs:label>
<foaf:name>Terrier</foaf:name>
<skos:prefLabel xml:lang="en">Terrier</skos:prefLabel>
<skos:definition xml:lang="en">Tommy&apos;s nickname for a Territorial or &quot;Saturday-night soldier.&quot; A regular despises a Territorial while a Territorial looks down on &quot;Kitchener&apos;s Mob.&quot; Kitchener&apos;s Mob has the utmost contempt for both of them.</skos:definition>
<skos:inScheme rdf:resource="#OverTheTopDictionary"/>
<rdf:type rdf:resource="http://dbpedia.org/resource/Slang"/>
<rdfs:isDefinedBy rdf:resource="http://rdf.muninn-project.org/ontologies/ott"/>
<rdf:type rdf:resource="http://dbpedia.org/resource/Irony"/>
<vs:term_status>Stable</vs:term_status>
</skos:Concept>
<skos:Concept rdf:ID="Territorial">
<rdfs:label xml:lang="en">Territorial</rdfs:label>
<foaf:name>Territorial</foaf:name>
<skos:prefLabel xml:lang="en">Territorial</skos:prefLabel>
<skos:definition xml:lang="en">A peace-time soldier with the same status as the American militiaman. Before the war they were called &quot;Saturday-Night Soldiers,&quot; but they soon proved themselves &quot;every-night soldiers.&quot;</skos:definition>
<skos:inScheme rdf:resource="#OverTheTopDictionary"/>
<rdfs:isDefinedBy rdf:resource="http://rdf.muninn-project.org/ontologies/ott"/>
<rdf:type rdf:resource="http://dbpedia.org/resource/Irony"/>
<vs:term_status>Stable</vs:term_status>
</skos:Concept>
<skos:Concept rdf:ID="TheOldMan">
<rdfs:label xml:lang="en">The Old Man</rdfs:label>
<foaf:name>The Old Man</foaf:name>
<skos:prefLabel xml:lang="en">The Old Man</skos:prefLabel>
<skos:definition xml:lang="en">Captain of a company. He is called &quot;the old man,&quot; because generally his age is about twenty-eight.</skos:definition>
<rdf:type rdf:resource="http://dbpedia.org/resource/Slang"/>
<rdf:type rdf:resource="http://dbpedia.org/resource/Nickname"/>
<skos:inScheme rdf:resource="#OverTheTopDictionary"/>
<rdfs:isDefinedBy rdf:resource="http://rdf.muninn-project.org/ontologies/ott"/>
<rdf:type rdf:resource="http://dbpedia.org/resource/Irony"/>
<vs:term_status>Stable</vs:term_status>
</skos:Concept>
<skos:Concept rdf:ID="TheBestoLuck">
<rdfs:label xml:lang="en">The Best o&apos; Luck</rdfs:label>
<foaf:name>The Best o&apos; Luck</foaf:name>
<rdf:type rdf:resource="http://dbpedia.org/resource/Slang"/>
<skos:prefLabel xml:lang="en">The Best o&apos; Luck</skos:prefLabel>
<skos:definition xml:lang="en">The Jonah phrase of the trenches. Every time Tommy goes over the top or on a trench raid his mates wish him the best o&apos; luck. It means that if you are lucky enough to come back, you generally have an arm or leg missing.</skos:definition>
<skos:inScheme rdf:resource="#OverTheTopDictionary"/>
<rdfs:isDefinedBy rdf:resource="http://rdf.muninn-project.org/ontologies/ott"/>
<rdf:type rdf:resource="http://dbpedia.org/resource/Irony"/>
<vs:term_status>Stable</vs:term_status>
</skos:Concept>
<skos:Concept rdf:ID="Thumbsup">
<rdfs:label xml:lang="en">Thumbs up</rdfs:label>
<foaf:name>Thumbs up</foaf:name>
<skos:prefLabel xml:lang="en">Thumbs up</skos:prefLabel>
<skos:definition xml:lang="en">Tommy&apos;s expression which means &quot;everything is fine with me.&quot; Very seldom used during an intense bombardment.</skos:definition>
<skos:inScheme rdf:resource="#OverTheTopDictionary"/>
<rdfs:isDefinedBy rdf:resource="http://rdf.muninn-project.org/ontologies/ott"/>
<rdf:type rdf:resource="http://dbpedia.org/resource/Slang"/>
<rdf:type rdf:resource="http://dbpedia.org/resource/Irony"/>
<vs:term_status>Stable</vs:term_status>
</skos:Concept>
<skos:Concept rdf:ID="Timeex">
<rdfs:label xml:lang="en">Time ex</rdfs:label>
<foaf:name>Time ex</foaf:name>
<skos:prefLabel xml:lang="en">Time ex</skos:prefLabel>
<skos:definition xml:lang="en">Expiration of term of enlistment. The only time Tommy is a civilian in the trenches; but about ten minutes after he is a soldier for duration of war.</skos:definition>
<skos:inScheme rdf:resource="#OverTheTopDictionary"/>
<rdf:type rdf:resource="http://dbpedia.org/resource/Slang"/>
<rdfs:isDefinedBy rdf:resource="http://rdf.muninn-project.org/ontologies/ott"/>
<rdf:type rdf:resource="http://dbpedia.org/resource/Irony"/>
<vs:term_status>Stable</vs:term_status>
</skos:Concept>
<skos:Concept rdf:ID="TinHat">
<rdfs:label xml:lang="en">Tin Hat</rdfs:label>
<foaf:name>Tin Hat</foaf:name>
<skos:prefLabel xml:lang="en">Tin Hat</skos:prefLabel>
<skos:definition xml:lang="en">Tommy&apos;s name for his steel helmet which is made out of a metal about as hard as mush. The only advantage is that it is heavy and greatly adds to the weight of Tommy&apos;s equipment. Its most popular use is for carrying eggs.</skos:definition>
<skos:inScheme rdf:resource="#OverTheTopDictionary"/>
<rdfs:isDefinedBy rdf:resource="http://rdf.muninn-project.org/ontologies/ott"/>
<rdf:type rdf:resource="http://dbpedia.org/resource/Irony"/>
<vs:term_status>Stable</vs:term_status>
</skos:Concept>
<skos:Concept rdf:ID="Trinitrotoluene">
<rdfs:label xml:lang="en">Trinitrotoluene</rdfs:label>
<muninn:acronym xml:lang="en">T.N.T.</muninn:acronym>
<foaf:name>Trinitrotoluene</foaf:name>
<skos:prefLabel xml:lang="en">Trinitrotoluene</skos:prefLabel>
<skos:definition xml:lang="en">A high explosive which the Army Ordnance Corps prescribes for Fritz. Fritz prefers a No. 9 pill.</skos:definition>
<skos:inScheme rdf:resource="#OverTheTopDictionary"/>
<rdfs:isDefinedBy rdf:resource="http://rdf.muninn-project.org/ontologies/ott"/>
<rdf:type rdf:resource="http://dbpedia.org/resource/Irony"/>
<vs:term_status>Stable</vs:term_status>
</skos:Concept>
<skos:Concept rdf:ID="TommyAtkins">
<rdfs:label xml:lang="en">Tommy Atkins</rdfs:label>
<foaf:name>Tommy Atkins</foaf:name>
<skos:prefLabel xml:lang="en">Tommy Atkins</skos:prefLabel>
<skos:definition xml:lang="en">The name England gives to an English soldier, even if his name is Willie Jones.</skos:definition>
<skos:inScheme rdf:resource="#OverTheTopDictionary"/>
<rdf:type rdf:resource="http://dbpedia.org/resource/Slang"/>
<rdf:type rdf:resource="http://dbpedia.org/resource/Nickname"/>
<rdfs:isDefinedBy rdf:resource="http://rdf.muninn-project.org/ontologies/ott"/>
<rdf:type rdf:resource="http://dbpedia.org/resource/Irony"/>
<vs:term_status>Stable</vs:term_status>
</skos:Concept>
<skos:Concept rdf:ID="TommysCooker">
<rdfs:label xml:lang="en">Tommy&apos;s Cooker</rdfs:label>
<foaf:name>Tommy&apos;s Cooker</foaf:name>
<skos:prefLabel xml:lang="en">Tommy&apos;s Cooker</skos:prefLabel>
<rdf:type rdf:resource="http://dbpedia.org/resource/Slang"/>
<skos:definition xml:lang="en">A spirit stove widely advertised as &quot;A suitable gift to the men in the trenches.&quot; Many are sent out to Tommy and most of them are thrown away.</skos:definition>
<skos:inScheme rdf:resource="#OverTheTopDictionary"/>
<rdfs:isDefinedBy rdf:resource="http://rdf.muninn-project.org/ontologies/ott"/>
<rdf:type rdf:resource="http://dbpedia.org/resource/Irony"/>
<vs:term_status>Stable</vs:term_status>
</skos:Concept>
<skos:Concept rdf:ID="Tonite">
<rdfs:label xml:lang="en">Tonite</rdfs:label>
<foaf:name>Tonite</foaf:name>
<skos:prefLabel xml:lang="en">Tonite</skos:prefLabel>
<skos:definition xml:lang="en">The explosive contained in a rifle grenade. It looks like a harmless reel of cotton before it explodes, -- after it explodes the spectator is missing.</skos:definition>
<skos:inScheme rdf:resource="#OverTheTopDictionary"/>
<rdfs:isDefinedBy rdf:resource="http://rdf.muninn-project.org/ontologies/ott"/>
<rdf:type rdf:resource="http://dbpedia.org/resource/Irony"/>
<vs:term_status>Stable</vs:term_status>
</skos:Concept>
<skos:Concept rdf:ID="TootsSweet">
<rdfs:label xml:lang="en">Toots Sweet</rdfs:label>
<foaf:name>Toots Sweet</foaf:name>
<skos:prefLabel xml:lang="en">Toots Sweet</skos:prefLabel>
<skos:definition xml:lang="en">Tommy&apos;s Preach for &quot;hurry up,&quot; &quot;look smart.&quot; Generally used in a French estaminet when Tommy only has a couple of minutes in which to drink his beer.</skos:definition>
<skos:inScheme rdf:resource="#OverTheTopDictionary"/>
<rdfs:isDefinedBy rdf:resource="http://rdf.muninn-project.org/ontologies/ott"/>
<rdf:type rdf:resource="http://dbpedia.org/resource/Slang"/>
<rdf:type rdf:resource="http://dbpedia.org/resource/Irony"/>
<vs:term_status>Stable</vs:term_status>
</skos:Concept>
<skos:Concept rdf:ID="TopHatsatHome">
<rdfs:label xml:lang="en">Top Hats at Home</rdfs:label>
<foaf:name>Top Hats at Home</foaf:name>
<skos:prefLabel xml:lang="en">Top Hats at Home</skos:prefLabel>
<skos:definition xml:lang="en">Tommy&apos;s name for Parliament when his application for leave has been turned down or when no strawberry jam arrives with the rations.</skos:definition>
<skos:inScheme rdf:resource="#OverTheTopDictionary"/>
<rdfs:isDefinedBy rdf:resource="http://rdf.muninn-project.org/ontologies/ott"/>
<rdf:type rdf:resource="http://dbpedia.org/resource/Slang"/>
<rdf:type rdf:resource="http://dbpedia.org/resource/Irony"/>
<vs:term_status>Stable</vs:term_status>
</skos:Concept>
<skos:Concept rdf:ID="TownMajor">
<rdfs:label xml:lang="en">Town Major</rdfs:label>
<foaf:name>Town Major</foaf:name>
<skos:prefLabel xml:lang="en">Town Major</skos:prefLabel>
<skos:definition xml:lang="en">An officer stationed in a. French town or village who is supposed to look after billets, upkeep of roads, and act as interpreter.</skos:definition>
<skos:inScheme rdf:resource="#OverTheTopDictionary"/>
<rdfs:isDefinedBy rdf:resource="http://rdf.muninn-project.org/ontologies/ott"/>
<rdf:type rdf:resource="http://dbpedia.org/resource/Irony"/>
<vs:term_status>Stable</vs:term_status>
</skos:Concept>
<skos:Concept rdf:ID="Transport">
<rdfs:label xml:lang="en">Transport</rdfs:label>
<foaf:name>Transport</foaf:name>
<skos:prefLabel xml:lang="en">Transport</skos:prefLabel>
<skos:definition xml:lang="en">An aggregation of mules, limbers, and rough riders, whose duty is to keep the men in the trenches supplied with rations and supplies. Sometimes a shell drops within two miles of them and Tommy doesn&apos;t get his rations, etc.</skos:definition>
<skos:inScheme rdf:resource="#OverTheTopDictionary"/>
<rdfs:isDefinedBy rdf:resource="http://rdf.muninn-project.org/ontologies/ott"/>
<rdf:type rdf:resource="http://dbpedia.org/resource/Irony"/>
<vs:term_status>Stable</vs:term_status>
</skos:Concept>
<skos:Concept rdf:ID="Traverse">
<rdfs:label xml:lang="en">Traverse</rdfs:label>
<foaf:name>Traverse</foaf:name>
<skos:prefLabel xml:lang="en">Traverse</skos:prefLabel>
<skos:definition xml:lang="en">Sandbags piled in a trench so that the trench cannot be traversed by Tommy. Sometimes it prevents enfilading fire by the enemy.</skos:definition>
<skos:inScheme rdf:resource="#OverTheTopDictionary"/>
<rdfs:isDefinedBy rdf:resource="http://rdf.muninn-project.org/ontologies/ott"/>
<rdf:type rdf:resource="http://dbpedia.org/resource/Irony"/>
<vs:term_status>Stable</vs:term_status>
</skos:Concept>
<skos:Concept rdf:ID="Trench">
<rdfs:label xml:lang="en">Trench</rdfs:label>
<foaf:name>Trench</foaf:name>
<skos:prefLabel xml:lang="en">Trench</skos:prefLabel>
<skos:definition xml:lang="en">A ditch full of water, rats, and soldiers. During his visit to France, Tommy uses these ditches as residences. Now and again he sticks his head &quot;over the top&quot; to take a look at the surrounding scenery. If he is lucky he lives to tell his mates what he saw.</skos:definition>
<skos:inScheme rdf:resource="#OverTheTopDictionary"/>
<rdfs:isDefinedBy rdf:resource="http://rdf.muninn-project.org/ontologies/ott"/>
<rdf:type rdf:resource="http://dbpedia.org/resource/Irony"/>
<vs:term_status>Stable</vs:term_status>
</skos:Concept>
<skos:Concept rdf:ID="TrenchFeet">
<rdfs:label xml:lang="en">Trench Feet</rdfs:label>
<foaf:name>Trench Feet</foaf:name>
<skos:prefLabel xml:lang="en">Trench Feet</skos:prefLabel>
<skos:definition xml:lang="en">A disease of the feet contracted in the trenches from exposure to extreme cold and wet. Tommy&apos;s greatest ambition is to contract this disease because it means &quot;Blighty&quot; for him.</skos:definition>
<skos:inScheme rdf:resource="#OverTheTopDictionary"/>
<rdfs:isDefinedBy rdf:resource="http://rdf.muninn-project.org/ontologies/ott"/>
<rdf:type rdf:resource="http://dbpedia.org/resource/Irony"/>
<vs:term_status>Stable</vs:term_status>
</skos:Concept>
<skos:Concept rdf:ID="TrenchFever">
<rdfs:label xml:lang="en">Trench Fever</rdfs:label>
<foaf:name>Trench Fever</foaf:name>
<skos:prefLabel xml:lang="en">Trench Fever</skos:prefLabel>
<skos:definition xml:lang="en">A malady contracted in the trenches; the symptoms are high temperature, bodily pains, and homesickness. Mostly homesickness. A bad case lands Tommy in &quot;Blighty,&quot; a slight case lands him back in the trenches, where he tries to get it worse than ever.</skos:definition>
<skos:inScheme rdf:resource="#OverTheTopDictionary"/>
<rdfs:isDefinedBy rdf:resource="http://rdf.muninn-project.org/ontologies/ott"/>
<rdf:type rdf:resource="http://dbpedia.org/resource/Irony"/>
<vs:term_status>Stable</vs:term_status>
</skos:Concept>
<skos:Concept rdf:ID="Trenchitis">
<rdfs:label xml:lang="en">Trenchitis</rdfs:label>
<foaf:name>Trenchitis</foaf:name>
<skos:prefLabel xml:lang="en">Trenchitis</skos:prefLabel>
<skos:definition xml:lang="en">A combination of &quot;fedupness&quot; and homesickness, experienced by Tommy in the trenches, especially when he receives a letter from a friend in Blighty who is making a fortune working in a munition plant.</skos:definition>
<skos:inScheme rdf:resource="#OverTheTopDictionary"/>
<rdfs:isDefinedBy rdf:resource="http://rdf.muninn-project.org/ontologies/ott"/>
<rdf:type rdf:resource="http://dbpedia.org/resource/Irony"/>
<vs:term_status>Stable</vs:term_status>
</skos:Concept>
<skos:Concept rdf:ID="TrenchMortar">
<rdfs:label xml:lang="en">Trench Mortar</rdfs:label>
<foaf:name>Trench Mortar</foaf:name>
<skos:prefLabel xml:lang="en">Trench Mortar</skos:prefLabel>
<skos:definition xml:lang="en">A gun like a stove pipe which throws shells at the German trenches. Tommy detests these mortars because when they take positions near to him in the trenches, he knows that it is only a matter of minutes before a German Shell with his name and number on it will be knocking at his door.</skos:definition>
<skos:inScheme rdf:resource="#OverTheTopDictionary"/>
<rdfs:isDefinedBy rdf:resource="http://rdf.muninn-project.org/ontologies/ott"/>
<rdf:type rdf:resource="http://dbpedia.org/resource/Irony"/>
<vs:term_status>Stable</vs:term_status>
</skos:Concept>
<skos:Concept rdf:ID="TrenchPudding">
<rdfs:label xml:lang="en">Trench Pudding</rdfs:label>
<foaf:name>Trench Pudding</foaf:name>
<skos:prefLabel xml:lang="en">Trench Pudding</skos:prefLabel>
<skos:definition xml:lang="en">A delectable mess of broken biscuits, condensed milk, jam, and mud. Slightly flavored with smoke. Tommy prepares, cooks, and eats this. Next day he has &quot;trench fever.&quot;</skos:definition>
<skos:inScheme rdf:resource="#OverTheTopDictionary"/>
<rdfs:isDefinedBy rdf:resource="http://rdf.muninn-project.org/ontologies/ott"/>
<rdf:type rdf:resource="http://dbpedia.org/resource/Slang"/>
<rdf:type rdf:resource="http://dbpedia.org/resource/Irony"/>
<vs:term_status>Stable</vs:term_status>
</skos:Concept>
<skos:Concept rdf:ID="TrenchRaid">
<rdfs:label xml:lang="en">Trench Raid</rdfs:label>
<foaf:name>Trench Raid</foaf:name>
<skos:prefLabel xml:lang="en">Trench Raid</skos:prefLabel>
<skos:definition xml:lang="en">Several men detailed to go over the top at night and shake hands with the Germans, and, if possible, persuade some of them to be prisoners. At times the raiders would themselves get raided because Fritz refused to shake and adopted nasty methods.</skos:definition>
<skos:inScheme rdf:resource="#OverTheTopDictionary"/>
<rdfs:isDefinedBy rdf:resource="http://rdf.muninn-project.org/ontologies/ott"/>
<rdf:type rdf:resource="http://dbpedia.org/resource/Irony"/>
<vs:term_status>Stable</vs:term_status>
</skos:Concept>
<skos:Concept rdf:ID="Turpenite">
<rdfs:label xml:lang="en">Turpenite</rdfs:label>
<foaf:name>Turpenite</foaf:name>
<skos:prefLabel xml:lang="en">Turpenite</skos:prefLabel>
<skos:definition xml:lang="en">A deadly chemical shell invented by an enthusiastic war correspondent suffering from brain storm. Companies and batteries were supposed to die standing up from its effects, but they refused to do this.</skos:definition>
<skos:inScheme rdf:resource="#OverTheTopDictionary"/>
<rdfs:isDefinedBy rdf:resource="http://rdf.muninn-project.org/ontologies/ott"/>
<rdf:type rdf:resource="http://dbpedia.org/resource/Irony"/>
<vs:term_status>Stable</vs:term_status>
</skos:Concept>
<skos:Concept rdf:ID="Twelveinone">
<rdfs:label xml:lang="en">Twelve in one</rdfs:label>
<foaf:name>Twelve in one</foaf:name>
<skos:prefLabel xml:lang="en">Twelve in one</skos:prefLabel>
<skos:definition xml:lang="en">Means that twelve men are to share one loaf of bread. When the slicing takes place the war in the dugout makes the European argument look like thirty cents.</skos:definition>
<skos:inScheme rdf:resource="#OverTheTopDictionary"/>
<rdfs:isDefinedBy rdf:resource="http://rdf.muninn-project.org/ontologies/ott"/>
<rdf:type rdf:resource="http://dbpedia.org/resource/Slang"/>
<rdf:type rdf:resource="http://dbpedia.org/resource/Irony"/>
<vs:term_status>Stable</vs:term_status>
</skos:Concept>
<skos:Concept rdf:ID="Upagainstthewall">
<rdfs:label xml:lang="en">Up against the wall</rdfs:label>
<foaf:name>Up against the wall</foaf:name>
<skos:prefLabel xml:lang="en">Up against the wall</skos:prefLabel>
<skos:definition xml:lang="en">Tommy&apos;s term for a man who is to be shot by a firing squad.</skos:definition>
<skos:inScheme rdf:resource="#OverTheTopDictionary"/>
<rdf:type rdf:resource="http://dbpedia.org/resource/Slang"/>
<rdfs:isDefinedBy rdf:resource="http://rdf.muninn-project.org/ontologies/ott"/>
<rdf:type rdf:resource="http://dbpedia.org/resource/Irony"/>
<vs:term_status>Stable</vs:term_status>
</skos:Concept>
<skos:Concept rdf:ID="Uptheline">
<rdfs:label xml:lang="en">Up the line</rdfs:label>
<foaf:name>Up the line</foaf:name>
<skos:prefLabel xml:lang="en">Up the line</skos:prefLabel>
<skos:definition xml:lang="en">Term generally used in rest billets when Tommy talks about the fire trench or fighting line. When orders are issued to go &quot;up the line&quot; Tommy immediately goes &quot;up in the air.&quot;</skos:definition>
<skos:inScheme rdf:resource="#OverTheTopDictionary"/>
<rdfs:isDefinedBy rdf:resource="http://rdf.muninn-project.org/ontologies/ott"/>
<rdf:type rdf:resource="http://dbpedia.org/resource/Irony"/>
<vs:term_status>Stable</vs:term_status>
</skos:Concept>
<skos:Concept rdf:ID="VictoriaCross">
<rdfs:label xml:lang="en">Victoria Cross</rdfs:label>
<muninn:acronym xml:lang="en">V.C.</muninn:acronym>
<foaf:name>Victoria Cross</foaf:name>
<skos:prefLabel xml:lang="en">Victoria Cross</skos:prefLabel>
<skos:definition xml:lang="en">Victoria Cross, or &quot;Very careless&quot; as Tommy calls it. It is a bronze medal won by Tommy for being very careless with his life.</skos:definition>
<skos:inScheme rdf:resource="#OverTheTopDictionary"/>
<rdfs:isDefinedBy rdf:resource="http://rdf.muninn-project.org/ontologies/ott"/>
<rdf:type rdf:resource="http://dbpedia.org/resource/Irony"/>
<vs:term_status>Stable</vs:term_status>
</skos:Concept>
<skos:Concept rdf:ID="VickersGun">
<rdfs:label xml:lang="en">Vickers Gun</rdfs:label>
<foaf:name>Vickers Gun</foaf:name>
<skos:prefLabel xml:lang="en">Vickers Gun</skos:prefLabel>
<skos:definition xml:lang="en">A machine gun improved on by a fellow named Vickers. His intentions were good but his improvements, according to Tommy, were &quot;rotten.&quot;</skos:definition>
<skos:inScheme rdf:resource="#OverTheTopDictionary"/>
<rdfs:isDefinedBy rdf:resource="http://rdf.muninn-project.org/ontologies/ott"/>
<rdf:type rdf:resource="http://dbpedia.org/resource/Irony"/>
<vs:term_status>Stable</vs:term_status>
</skos:Concept>
<skos:Concept rdf:ID="Waders">
<rdfs:label xml:lang="en">Waders</rdfs:label>
<foaf:name>Waders</foaf:name>
<skos:prefLabel xml:lang="en">Waders</skos:prefLabel>
<skos:definition xml:lang="en">Rubber hip boots, used when the water in the trenches is up to Tommy&apos;s neck.</skos:definition>
<skos:inScheme rdf:resource="#OverTheTopDictionary"/>
<rdfs:isDefinedBy rdf:resource="http://rdf.muninn-project.org/ontologies/ott"/>
<rdf:type rdf:resource="http://dbpedia.org/resource/Irony"/>
<vs:term_status>Stable</vs:term_status>
</skos:Concept>
<skos:Concept rdf:ID="WaitingMan">
<rdfs:label xml:lang="en">Waiting Man</rdfs:label>
<foaf:name>Waiting Man</foaf:name>
<skos:prefLabel xml:lang="en">Waiting Man</skos:prefLabel>
<skos:definition xml:lang="en">The cleanest man at guard mounting. He does not have to walk post; is supposed to wait on the guard.</skos:definition>
<skos:inScheme rdf:resource="#OverTheTopDictionary"/>
<rdf:type rdf:resource="http://dbpedia.org/resource/Slang"/>
<rdfs:isDefinedBy rdf:resource="http://rdf.muninn-project.org/ontologies/ott"/>
<rdf:type rdf:resource="http://dbpedia.org/resource/Irony"/>
<vs:term_status>Stable</vs:term_status>
</skos:Concept>
<skos:Concept rdf:ID="Washout">
<rdfs:label xml:lang="en">Washout</rdfs:label>
<foaf:name>Washout</foaf:name>
<skos:prefLabel xml:lang="en">Washout</skos:prefLabel>
<skos:definition xml:lang="en">Tommy&apos;s idea of something that is worth nothing.</skos:definition>
<skos:inScheme rdf:resource="#OverTheTopDictionary"/>
<rdfs:isDefinedBy rdf:resource="http://rdf.muninn-project.org/ontologies/ott"/>
<rdf:type rdf:resource="http://dbpedia.org/resource/Slang"/>
<rdf:type rdf:resource="http://dbpedia.org/resource/Irony"/>
<vs:term_status>Stable</vs:term_status>
</skos:Concept>
<skos:Concept rdf:ID="WaterBottle">
<rdfs:label xml:lang="en">Water Bottle</rdfs:label>
<foaf:name>Water Bottle</foaf:name>
<skos:prefLabel xml:lang="en">Water Bottle</skos:prefLabel>
<skos:definition xml:lang="en">A metal bottle for carrying water (when not used for rum, beer, or wine).</skos:definition>
<skos:inScheme rdf:resource="#OverTheTopDictionary"/>
<rdfs:isDefinedBy rdf:resource="http://rdf.muninn-project.org/ontologies/ott"/>
<rdf:type rdf:resource="http://dbpedia.org/resource/Irony"/>
<vs:term_status>Stable</vs:term_status>
</skos:Concept>
<skos:Concept rdf:ID="Waterproof">
<rdfs:label xml:lang="en">Waterproof</rdfs:label>
<foaf:name>Waterproof</foaf:name>
<skos:prefLabel xml:lang="en">Waterproof</skos:prefLabel>
<skos:definition xml:lang="en">A rubber sheet issued to Tommy to keep him dry. It does when the sun is out.</skos:definition>
<skos:inScheme rdf:resource="#OverTheTopDictionary"/>
<rdfs:isDefinedBy rdf:resource="http://rdf.muninn-project.org/ontologies/ott"/>
<rdf:type rdf:resource="http://dbpedia.org/resource/Irony"/>
<vs:term_status>Stable</vs:term_status>
</skos:Concept>
<skos:Concept rdf:ID="Wave">
<rdfs:label xml:lang="en">Wave</rdfs:label>
<foaf:name>Wave</foaf:name>
<skos:prefLabel xml:lang="en">Wave</skos:prefLabel>
<skos:definition xml:lang="en">A line of troops which goes &quot;over the top&quot; in a charge. The waves are numbered according to their turn in going over, viz., &quot;First Wave,&quot; &quot;Second Wave,&quot; etc. Tommy would sooner go over with the &quot; Tenth Wave.&quot;</skos:definition>
<skos:inScheme rdf:resource="#OverTheTopDictionary"/>
<rdfs:isDefinedBy rdf:resource="http://rdf.muninn-project.org/ontologies/ott"/>
<rdf:type rdf:resource="http://dbpedia.org/resource/Irony"/>
<vs:term_status>Stable</vs:term_status>
</skos:Concept>
<skos:Concept rdf:ID="WetCanteen">
<rdfs:label xml:lang="en">Wet Canteen</rdfs:label>
<foaf:name>Wet Canteen</foaf:name>
<skos:prefLabel xml:lang="en">Wet Canteen</skos:prefLabel>
<skos:definition xml:lang="en">A military saloon or pub where Tommy can get a &quot;wet,&quot; Most campaigns and battles are planned and fought in these places.</skos:definition>
<skos:inScheme rdf:resource="#OverTheTopDictionary"/>
<rdfs:isDefinedBy rdf:resource="http://rdf.muninn-project.org/ontologies/ott"/>
<rdf:type rdf:resource="http://dbpedia.org/resource/Irony"/>
<vs:term_status>Stable</vs:term_status>
</skos:Concept>
<skos:Concept rdf:ID="WhizzBang">
<rdfs:label xml:lang="en">Whizz Bang</rdfs:label>
<foaf:name>Whizz Bang</foaf:name>
<skos:prefLabel xml:lang="en">Whizz Bang</skos:prefLabel>
<skos:definition xml:lang="en">A small German shell which whizzes through the air and explodes with a &quot;bang.&quot; Their bark is worse than their bite.</skos:definition>
<skos:inScheme rdf:resource="#OverTheTopDictionary"/>
<rdfs:isDefinedBy rdf:resource="http://rdf.muninn-project.org/ontologies/ott"/>
<rdf:type rdf:resource="http://dbpedia.org/resource/Irony"/>
<rdf:type rdf:resource="http://dbpedia.org/resource/Slang"/>
<vs:term_status>Stable</vs:term_status>
</skos:Concept>
<skos:Concept rdf:ID="Windup">
<rdfs:label xml:lang="en">Wind up</rdfs:label>
<foaf:name>Wind up</foaf:name>
<skos:prefLabel xml:lang="en">Wind up</skos:prefLabel>
<skos:definition xml:lang="en">Term generally applied to the Germans when they send up several star shells at once because they are nervous and expect an attack or night raid on their trenches.</skos:definition>
<skos:inScheme rdf:resource="#OverTheTopDictionary"/>
<rdfs:isDefinedBy rdf:resource="http://rdf.muninn-project.org/ontologies/ott"/>
<rdf:type rdf:resource="http://dbpedia.org/resource/Irony"/>
<vs:term_status>Stable</vs:term_status>
</skos:Concept>
<skos:Concept rdf:ID="Windy">
<rdfs:label xml:lang="en">Windy</rdfs:label>
<foaf:name>Windy</foaf:name>
<skos:prefLabel xml:lang="en">Windy</skos:prefLabel>
<skos:definition xml:lang="en">Tommy&apos;s name for a nervous soldier, coward.</skos:definition>
<skos:inScheme rdf:resource="#OverTheTopDictionary"/>
<rdfs:isDefinedBy rdf:resource="http://rdf.muninn-project.org/ontologies/ott"/>
<rdf:type rdf:resource="http://dbpedia.org/resource/Irony"/>
<vs:term_status>Stable</vs:term_status>
</skos:Concept>
<skos:Concept rdf:ID="Wipers">
<rdfs:label xml:lang="en">Wipers</rdfs:label>
<foaf:name>Wipers</foaf:name>
<skos:prefLabel xml:lang="en">Wipers</skos:prefLabel>
<skos:definition xml:lang="en">Tommy&apos;s name for Ypres, sometimes he calls it &quot;Yeeps.&quot; A place up the line which Tommy likes to duck. It is even &quot;hot&quot; in the winter time at &quot;Wipers.&quot;</skos:definition>
<skos:inScheme rdf:resource="#OverTheTopDictionary"/>
<rdfs:isDefinedBy rdf:resource="http://rdf.muninn-project.org/ontologies/ott"/>
<rdf:type rdf:resource="http://dbpedia.org/resource/Irony"/>
<rdf:type rdf:resource="http://dbpedia.org/resource/Slang"/>
<owl:sameAs rdf:resource="http://dbpedia.org/resource/Battle_of_Ypres"/>
<vs:term_status>Stable</vs:term_status>
</skos:Concept>
<skos:Concept rdf:ID="WireCutters">
<rdfs:label xml:lang="en">Wire Cutters</rdfs:label>
<foaf:name>Wire Cutters</foaf:name>
<skos:prefLabel xml:lang="en">Wire Cutters</skos:prefLabel>
<skos:definition xml:lang="en">An instrument for cutting barbed wire, but mostly used for driving nails.</skos:definition>
<skos:inScheme rdf:resource="#OverTheTopDictionary"/>
<rdfs:isDefinedBy rdf:resource="http://rdf.muninn-project.org/ontologies/ott"/>
<rdf:type rdf:resource="http://dbpedia.org/resource/Irony"/>
<vs:term_status>Stable</vs:term_status>
</skos:Concept>
<skos:Concept rdf:ID="WiringParty">
<rdfs:label xml:lang="en">Wiring Party</rdfs:label>
<foaf:name>Wiring Party</foaf:name>
<skos:prefLabel xml:lang="en">Wiring Party</skos:prefLabel>
<skos:definition xml:lang="en">Another social affair for which Tommy receives invitations. It consists of going &quot;over the top &quot; at night and stretching barbed wire between stakes. A German machine gun generally takes the place of an orchestra.</skos:definition>
<skos:inScheme rdf:resource="#OverTheTopDictionary"/>
<rdfs:isDefinedBy rdf:resource="http://rdf.muninn-project.org/ontologies/ott"/>
<rdf:type rdf:resource="http://dbpedia.org/resource/Irony"/>
<vs:term_status>Stable</vs:term_status>
</skos:Concept>
<skos:Concept rdf:ID="Woodbine">
<rdfs:label xml:lang="en">Woodbine</rdfs:label>
<foaf:name>Woodbine</foaf:name>
<skos:prefLabel xml:lang="en">Woodbine</skos:prefLabel>
<skos:definition xml:lang="en">A cigarette made of paper and old hay. Tommy swears by a Woodbine.</skos:definition>
<skos:inScheme rdf:resource="#OverTheTopDictionary"/>
<rdfs:isDefinedBy rdf:resource="http://rdf.muninn-project.org/ontologies/ott"/>
<rdf:type rdf:resource="http://dbpedia.org/resource/Slang"/>
<rdf:type rdf:resource="http://dbpedia.org/resource/Irony"/>
<vs:term_status>Stable</vs:term_status>
</skos:Concept>
<skos:Concept rdf:ID="WoodenCross">
<rdfs:label xml:lang="en">Wooden Cross</rdfs:label>
<foaf:name>Wooden Cross</foaf:name>
<skos:prefLabel xml:lang="en">Wooden Cross</skos:prefLabel>
<skos:definition xml:lang="en">Two pieces of wood in the form of a cross placed at the head of a Tommy&apos;s grave. Inscribed on it are his rank, name, number, and regiment. Also date of death and last but not least, the letters R. I. P.</skos:definition>
<skos:inScheme rdf:resource="#OverTheTopDictionary"/>
<rdfs:isDefinedBy rdf:resource="http://rdf.muninn-project.org/ontologies/ott"/>
<rdf:type rdf:resource="http://dbpedia.org/resource/Irony"/>
<vs:term_status>Stable</vs:term_status>
</skos:Concept>
<skos:Concept rdf:ID="WorkingParty">
<rdfs:label xml:lang="en">Working Party</rdfs:label>
<foaf:name>Working Party</foaf:name>
<skos:prefLabel xml:lang="en">Working Party</skos:prefLabel>
<skos:definition xml:lang="en">A sort of compulsory invitation affair for which Tommy often is honored with an invitation. It consists of digging, filling sandbags, and ducking shells and bullets.</skos:definition>
<skos:inScheme rdf:resource="#OverTheTopDictionary"/>
<rdfs:isDefinedBy rdf:resource="http://rdf.muninn-project.org/ontologies/ott"/>
<rdf:type rdf:resource="http://dbpedia.org/resource/Irony"/>
<vs:term_status>Stable</vs:term_status>
</skos:Concept>
<skos:Concept rdf:ID="Zeppelin">
<rdfs:label xml:lang="en">Zeppelin</rdfs:label>
<foaf:name>Zeppelin</foaf:name>
<skos:prefLabel xml:lang="en">Zeppelin</skos:prefLabel>
<skos:definition xml:lang="en">A bag full of gas invented by a count full of gas. It is a dirigible airship used by the Germans for killing babies and dropping bombs in open fields. You never see them over the trenches, it is safer to bombard civilians in cities. They use Iron Crosses for ballast.</skos:definition>
<skos:inScheme rdf:resource="#OverTheTopDictionary"/>
<rdfs:isDefinedBy rdf:resource="http://rdf.muninn-project.org/ontologies/ott"/>
<rdf:type rdf:resource="http://dbpedia.org/resource/Irony"/>
<vs:term_status>Stable</vs:term_status>
</skos:Concept>

</rdf:RDF>

 